@prefix rdf: <http://www.w3.org/1999/02/22-rdf-syntax-ns#> .
@prefix dct: <http://purl.org/dc/terms/> .
@prefix xsd: <http://www.w3.org/2001/XMLSchema#> .
@prefix aspfacet:  <http://cv.iptc.org/newscodes/asportfacet/> .
@prefix aspfacetvalue:  <http://cv.iptc.org/newscodes/asportfacetvalue/> .
@prefix ikos:  <http://cv.iptc.org/newscodes/ikos/> .
@prefix skos:  <http://www.w3.org/2004/02/skos/core#> .

<http://cv.iptc.org/newscodes/asportfacetvalue/> 
	rdf:type skos:ConceptScheme ; 
  ikos:prefSchemeAlias "aspfacetvalue" ;
  ikos:authority "http://www.iptc.org" ;
  dct:rightsHolder "IPTC, International Press Telecommunications Council - https://iptc.org" ;
  ikos:licenceLink "http://creativecommons.org/licenses/by/4.0/" ;
  ikos:dateReleased "2019-11-25T12:00:00+00:00"^^xsd:dateTime ;
  dct:dateSubmitted "2019-11-25T12:00:00+00:00"^^xsd:dateTime ;
  skos:prefLabel "Value of a Sport Facet"@en-GB ;
  skos:definition "A value which may be used with specific facet(s) of the Sport Facets NewsCodes - http://cv.iptc.org/newscodes/asportfacet/"@en-GB ;
	skos:HasTopConcept		aspfacetvalue:14.1 ;
	skos:HasTopConcept		aspfacetvalue:470 ;
	skos:HasTopConcept		aspfacetvalue:49er ;
	skos:HasTopConcept		aspfacetvalue:505 ;
	skos:HasTopConcept		aspfacetvalue:8-ball ;
	skos:HasTopConcept		aspfacetvalue:9-ball ;
	skos:HasTopConcept		aspfacetvalue:accuracy ;
	skos:HasTopConcept		aspfacetvalue:aerials ;
	skos:HasTopConcept		aspfacetvalue:air-pistol ;
	skos:HasTopConcept		aspfacetvalue:air-rifle ;
	skos:HasTopConcept		aspfacetvalue:around-the-world ;
	skos:HasTopConcept		aspfacetvalue:artistic-skiing ;
	skos:HasTopConcept		aspfacetvalue:backstroke ;
	skos:HasTopConcept		aspfacetvalue:ball ;
	skos:HasTopConcept		aspfacetvalue:bare-hand ;
	skos:HasTopConcept		aspfacetvalue:beam ;
	skos:HasTopConcept		aspfacetvalue:bi-crossing ;
	skos:HasTopConcept		aspfacetvalue:breaststroke ;
	skos:HasTopConcept		aspfacetvalue:butterfly ;
	skos:HasTopConcept		aspfacetvalue:canoe-sailing ;
	skos:HasTopConcept		aspfacetvalue:chistera-ancha ;
	skos:HasTopConcept		aspfacetvalue:chistera-corta ;
	skos:HasTopConcept		aspfacetvalue:classic ;
	skos:HasTopConcept		aspfacetvalue:clean-and-jerk ;
	skos:HasTopConcept		aspfacetvalue:clubs ;
	skos:HasTopConcept		aspfacetvalue:combined-alpineskiing ;
	skos:HasTopConcept		aspfacetvalue:combined-nordicskiing ;
	skos:HasTopConcept		aspfacetvalue:combined-waterskiing ;
	skos:HasTopConcept		aspfacetvalue:coxless ;
	skos:HasTopConcept		aspfacetvalue:cross-country-equestrian ;
	skos:HasTopConcept		aspfacetvalue:cross-country-race ;
	skos:HasTopConcept		aspfacetvalue:cyclo-cross ;
	skos:HasTopConcept		aspfacetvalue:DDC ;
	skos:HasTopConcept		aspfacetvalue:discathon ;
	skos:HasTopConcept		aspfacetvalue:disc-golf ;
	skos:HasTopConcept		aspfacetvalue:distance ;
	skos:HasTopConcept		aspfacetvalue:double-trap ;
	skos:HasTopConcept		aspfacetvalue:downhill ;
	skos:HasTopConcept		aspfacetvalue:dressage ;
	skos:HasTopConcept		aspfacetvalue:endurance-equestrian ;
	skos:HasTopConcept		aspfacetvalue:endurance-motorcycling ;
	skos:HasTopConcept		aspfacetvalue:endurance-motorracing ;
	skos:HasTopConcept		aspfacetvalue:enduro ;
	skos:HasTopConcept		aspfacetvalue:epee ;
	skos:HasTopConcept		aspfacetvalue:europe ;
	skos:HasTopConcept		aspfacetvalue:eventing ;
	skos:HasTopConcept		aspfacetvalue:F3000 ;
	skos:HasTopConcept		aspfacetvalue:finn ;
	skos:HasTopConcept		aspfacetvalue:flatland ;
	skos:HasTopConcept		aspfacetvalue:flat-racing ;
	skos:HasTopConcept		aspfacetvalue:floorexercise ;
	skos:HasTopConcept		aspfacetvalue:flying-dutchman ;
	skos:HasTopConcept		aspfacetvalue:foil ;
	skos:HasTopConcept		aspfacetvalue:folkrace ;
	skos:HasTopConcept		aspfacetvalue:formulaone ;
	skos:HasTopConcept		aspfacetvalue:freestyle-flyingdisc ;
	skos:HasTopConcept		aspfacetvalue:freestyle-swimming ;
	skos:HasTopConcept		aspfacetvalue:fronton ;
	skos:HasTopConcept		aspfacetvalue:futsal ;
	skos:HasTopConcept		aspfacetvalue:giantslalom-alpineskiing ;
	skos:HasTopConcept		aspfacetvalue:giantslalom-snowboarding ;
	skos:HasTopConcept		aspfacetvalue:grandprix ;
	skos:HasTopConcept		aspfacetvalue:grasstrack ;
	skos:HasTopConcept		aspfacetvalue:guts ;
	skos:HasTopConcept		aspfacetvalue:harnessracing ;
	skos:HasTopConcept		aspfacetvalue:hoop ;
	skos:HasTopConcept		aspfacetvalue:horizontalbar ;
	skos:HasTopConcept		aspfacetvalue:horse-driving ;
	skos:HasTopConcept		aspfacetvalue:ice-dance ;
	skos:HasTopConcept		aspfacetvalue:beach-football ;
	skos:HasTopConcept		aspfacetvalue:indoor-soccer ;
	skos:HasTopConcept		aspfacetvalue:indyracing ;
	skos:HasTopConcept		aspfacetvalue:jump ;
	skos:HasTopConcept		aspfacetvalue:jumping ;
	skos:HasTopConcept		aspfacetvalue:kart-racing ;
	skos:HasTopConcept		aspfacetvalue:keirin ;
	skos:HasTopConcept		aspfacetvalue:lake ;
	skos:HasTopConcept		aspfacetvalue:land ;
	skos:HasTopConcept		aspfacetvalue:laser ;
	skos:HasTopConcept		aspfacetvalue:left-wall ;
	skos:HasTopConcept		aspfacetvalue:lightweight ;
	skos:HasTopConcept		aspfacetvalue:madison-race ;
	skos:HasTopConcept		aspfacetvalue:marathon ;
	skos:HasTopConcept		aspfacetvalue:massstart ;
	skos:HasTopConcept		aspfacetvalue:medley ;
	skos:HasTopConcept		aspfacetvalue:men ;
	skos:HasTopConcept		aspfacetvalue:mistral ;
	skos:HasTopConcept		aspfacetvalue:mixed ;
	skos:HasTopConcept		aspfacetvalue:moguls ;
	skos:HasTopConcept		aspfacetvalue:monohull ;
	skos:HasTopConcept		aspfacetvalue:moto-ball ;
	skos:HasTopConcept		aspfacetvalue:moto-cross ;
	skos:HasTopConcept		aspfacetvalue:motoGP ;
	skos:HasTopConcept		aspfacetvalue:MTA ;
	skos:HasTopConcept		aspfacetvalue:multihulls ;
	skos:HasTopConcept		aspfacetvalue:ocean ;
	skos:HasTopConcept		aspfacetvalue:ovaltrack ;
	skos:HasTopConcept		aspfacetvalue:overall ;
	skos:HasTopConcept		aspfacetvalue:pairs ;
	skos:HasTopConcept		aspfacetvalue:pala-ancha ;
	skos:HasTopConcept		aspfacetvalue:pala-corta ;
	skos:HasTopConcept		aspfacetvalue:parallelbars ;
	skos:HasTopConcept		aspfacetvalue:parallelslalom-alpineskiing ;
	skos:HasTopConcept		aspfacetvalue:parallelslalom-snowboarding ;
	skos:HasTopConcept		aspfacetvalue:park ;
	skos:HasTopConcept		aspfacetvalue:pasaka ;
	skos:HasTopConcept		aspfacetvalue:pistol ;
	skos:HasTopConcept		aspfacetvalue:points-race ;
	skos:HasTopConcept		aspfacetvalue:pommelhorse ;
	skos:HasTopConcept		aspfacetvalue:pontoniering ;
	skos:HasTopConcept		aspfacetvalue:powerlifting ;
	skos:HasTopConcept		aspfacetvalue:pursuit ;
	skos:HasTopConcept		aspfacetvalue:rallycross ;
	skos:HasTopConcept		aspfacetvalue:rallying ;
	skos:HasTopConcept		aspfacetvalue:rapid-fire-pistol ;
	skos:HasTopConcept		aspfacetvalue:rebot ;
	skos:HasTopConcept		aspfacetvalue:reining ;
	skos:HasTopConcept		aspfacetvalue:relay ;
	skos:HasTopConcept		aspfacetvalue:ribbon ;
	skos:HasTopConcept		aspfacetvalue:rifle-3-positions ;
	skos:HasTopConcept		aspfacetvalue:rifle-prone ;
	skos:HasTopConcept		aspfacetvalue:rings ;
	skos:HasTopConcept		aspfacetvalue:river ;
	skos:HasTopConcept		aspfacetvalue:road-race ;
	skos:HasTopConcept		aspfacetvalue:rope ;
	skos:HasTopConcept		aspfacetvalue:running-target ;
	skos:HasTopConcept		aspfacetvalue:sabre ;
	skos:HasTopConcept		aspfacetvalue:SCF ;
	skos:HasTopConcept		aspfacetvalue:sculls ;
	skos:HasTopConcept		aspfacetvalue:shortcourse ;
	skos:HasTopConcept		aspfacetvalue:side-cars ;
	skos:HasTopConcept		aspfacetvalue:singles ;
	skos:HasTopConcept		aspfacetvalue:skating-freestyle ;
	skos:HasTopConcept		aspfacetvalue:skeet ;
	skos:HasTopConcept		aspfacetvalue:skiathlon ;
	skos:HasTopConcept		aspfacetvalue:ski-cross ;
	skos:HasTopConcept		aspfacetvalue:slalom-alpineskiing ;
	skos:HasTopConcept		aspfacetvalue:slalom-canoekayaking ;
	skos:HasTopConcept		aspfacetvalue:slalom-snowboarding ;
	skos:HasTopConcept		aspfacetvalue:slalom-waterskiing ;
	skos:HasTopConcept		aspfacetvalue:sled ;
	skos:HasTopConcept		aspfacetvalue:snatch ;
	skos:HasTopConcept		aspfacetvalue:snooker ;
	skos:HasTopConcept		aspfacetvalue:big-air-snowboarding ;
	skos:HasTopConcept		aspfacetvalue:snowboard-cross ;
	skos:HasTopConcept		aspfacetvalue:halfpipe-snowboarding ;
	skos:HasTopConcept		aspfacetvalue:soling ;
	skos:HasTopConcept		aspfacetvalue:speedway ;
	skos:HasTopConcept		aspfacetvalue:sprint ;
	skos:HasTopConcept		aspfacetvalue:staged ;
	skos:HasTopConcept		aspfacetvalue:star ;
	skos:HasTopConcept		aspfacetvalue:steeplechase ;
	skos:HasTopConcept		aspfacetvalue:street ;
	skos:HasTopConcept		aspfacetvalue:supercross ;
	skos:HasTopConcept		aspfacetvalue:superg ;
	skos:HasTopConcept		aspfacetvalue:teamsprint-cycling ;
	skos:HasTopConcept		aspfacetvalue:teamsprint-nordicskiing ;
	skos:HasTopConcept		aspfacetvalue:time-trial ;
	skos:HasTopConcept		aspfacetvalue:tornado ;
	skos:HasTopConcept		aspfacetvalue:track ;
	skos:HasTopConcept		aspfacetvalue:trap ;
	skos:HasTopConcept		aspfacetvalue:TRC ;
	skos:HasTopConcept		aspfacetvalue:trial ;
	skos:HasTopConcept		aspfacetvalue:trick ;
	skos:HasTopConcept		aspfacetvalue:trinquet ;
	skos:HasTopConcept		aspfacetvalue:trotting ;
	skos:HasTopConcept		aspfacetvalue:ultimate ;
	skos:HasTopConcept		aspfacetvalue:unevenbars ;
	skos:HasTopConcept		aspfacetvalue:vault ;
	skos:HasTopConcept		aspfacetvalue:vaulting ;
	skos:HasTopConcept		aspfacetvalue:vertramp ;
	skos:HasTopConcept		aspfacetvalue:vtt-cross ;
	skos:HasTopConcept		aspfacetvalue:vtt-downhill ;
	skos:HasTopConcept		aspfacetvalue:women ;
	skos:HasTopConcept		aspfacetvalue:xare ;
	skos:HasTopConcept		aspfacetvalue:yngling .

aspfacetvalue:14.1
	rdf:type skos:Concept ;
	skos:prefLabel	"14.1"@en-GB ;
	skos:definition	"A player nominates the ball he is attempting to pot and into which pocket. He collects points for each successful hit. He continues until he makes a mistake. Before hitting the 15th ball, the 14 reds are set up again in the triangle."@en-GB ;
	skos:inScheme <http://cv.iptc.org/newscodes/asportfacetvalue/>  ;
	ikos:created "2017-07-04T12:00:00+00:00"^^xsd:dateTime ;
	dct:created "2017-07-04T12:00:00+00:00"^^xsd:dateTime ;
	ikos:modified "2017-07-04T12:00:00+00:00"^^xsd:dateTime ;
	dct:modified "2017-07-04T12:00:00+00:00"^^xsd:dateTime  ;
	ikos:isObjectOf aspfacet:billiardtype .

aspfacetvalue:470
	rdf:type skos:Concept ;
	skos:prefLabel	"470"@en-GB ;
	skos:definition	"Boat Category: two man dinghy (7.10m/sq mainsail) Olympic sport "@en-GB ;
	skos:inScheme <http://cv.iptc.org/newscodes/asportfacetvalue/>  ;
	ikos:created "2017-07-04T12:00:00+00:00"^^xsd:dateTime ;
	dct:created "2017-07-04T12:00:00+00:00"^^xsd:dateTime ;
	ikos:modified "2017-07-04T12:00:00+00:00"^^xsd:dateTime ;
	dct:modified "2017-07-04T12:00:00+00:00"^^xsd:dateTime  ;
	ikos:isObjectOf aspfacet:sailingtype .

aspfacetvalue:49er
	rdf:type skos:Concept ;
	skos:prefLabel	"49er"@en-GB ;
	skos:definition	"Boat Category: two man dinghy (8.23m/sq mainsail) Olympic sport"@en-GB ;
	skos:inScheme <http://cv.iptc.org/newscodes/asportfacetvalue/>  ;
	ikos:created "2017-07-04T12:00:00+00:00"^^xsd:dateTime ;
	dct:created "2017-07-04T12:00:00+00:00"^^xsd:dateTime ;
	ikos:modified "2017-07-04T12:00:00+00:00"^^xsd:dateTime ;
	dct:modified "2017-07-04T12:00:00+00:00"^^xsd:dateTime  ;
	ikos:isObjectOf aspfacet:sailingtype .

aspfacetvalue:505
	rdf:type skos:Concept ;
	skos:prefLabel	"505"@en-GB ;
	skos:definition	"Boat Category: two man dinghy"@en-GB ;
	skos:inScheme <http://cv.iptc.org/newscodes/asportfacetvalue/>  ;
	ikos:created "2017-07-04T12:00:00+00:00"^^xsd:dateTime ;
	dct:created "2017-07-04T12:00:00+00:00"^^xsd:dateTime ;
	ikos:modified "2017-07-04T12:00:00+00:00"^^xsd:dateTime ;
	dct:modified "2017-07-04T12:00:00+00:00"^^xsd:dateTime  ;
	ikos:isObjectOf aspfacet:sailingtype .

aspfacetvalue:8-ball
	rdf:type skos:Concept ;
	skos:prefLabel	"8-ball"@en-GB ;
	skos:definition	"A game using 15 balls and a white. The first player aims to pot the balls numbered 1-7 (solids) with the second player potting balls 9-15 (stripes). After that the first player to pot the black wins."@en-GB ;
	skos:inScheme <http://cv.iptc.org/newscodes/asportfacetvalue/>  ;
	ikos:created "2017-07-04T12:00:00+00:00"^^xsd:dateTime ;
	dct:created "2017-07-04T12:00:00+00:00"^^xsd:dateTime ;
	ikos:modified "2017-07-04T12:00:00+00:00"^^xsd:dateTime ;
	dct:modified "2017-07-04T12:00:00+00:00"^^xsd:dateTime  ;
	ikos:isObjectOf aspfacet:billiardtype .

aspfacetvalue:9-ball
	rdf:type skos:Concept ;
	skos:prefLabel	"9-ball"@en-GB ;
	skos:definition	"A game played with nine balls numbered 1-9, and a white. On each turn the player must hit the lowest numbered ball."@en-GB ;
	skos:inScheme <http://cv.iptc.org/newscodes/asportfacetvalue/>  ;
	ikos:created "2017-07-04T12:00:00+00:00"^^xsd:dateTime ;
	dct:created "2017-07-04T12:00:00+00:00"^^xsd:dateTime ;
	ikos:modified "2017-07-04T12:00:00+00:00"^^xsd:dateTime ;
	dct:modified "2017-07-04T12:00:00+00:00"^^xsd:dateTime  ;
	ikos:isObjectOf aspfacet:billiardtype .

aspfacetvalue:accuracy
	rdf:type skos:Concept ;
	skos:prefLabel	"accuracy"@en-GB ;
	skos:definition	"Each player has 28 throws from various distances and angles to throw the disc through a goal 1.5 x 1.5 meters."@en-GB ;
	skos:inScheme <http://cv.iptc.org/newscodes/asportfacetvalue/>  ;
	ikos:created "2017-07-04T12:00:00+00:00"^^xsd:dateTime ;
	dct:created "2017-07-04T12:00:00+00:00"^^xsd:dateTime ;
	ikos:modified "2017-07-04T12:00:00+00:00"^^xsd:dateTime ;
	dct:modified "2017-07-04T12:00:00+00:00"^^xsd:dateTime  ;
	ikos:isObjectOf aspfacet:flyingdisctype .

aspfacetvalue:aerials
	rdf:type skos:Concept ;
	skos:prefLabel	"aerials"@en-GB ;
	skos:definition	"Competitors perform a series of aerial twists and turns from a prepared jump."@en-GB ;
	skos:inScheme <http://cv.iptc.org/newscodes/asportfacetvalue/>  ;
	ikos:created "2017-07-04T12:00:00+00:00"^^xsd:dateTime ;
	dct:created "2017-07-04T12:00:00+00:00"^^xsd:dateTime ;
	ikos:modified "2017-07-04T12:00:00+00:00"^^xsd:dateTime ;
	dct:modified "2017-07-04T12:00:00+00:00"^^xsd:dateTime  ;
	ikos:isObjectOf aspfacet:freestyleskiingtype .

aspfacetvalue:air-pistol
	rdf:type skos:Concept ;
	skos:prefLabel	"air pistol"@en-GB ;
	skos:definition	"Shooting event shot with 4.5 mm (or .177) caliber air guns at a distance of 10 metres (11 yards)"@en-GB ;
	skos:inScheme <http://cv.iptc.org/newscodes/asportfacetvalue/>  ;
	ikos:created "2017-07-04T12:00:00+00:00"^^xsd:dateTime ;
	dct:created "2017-07-04T12:00:00+00:00"^^xsd:dateTime ;
	ikos:modified "2017-07-04T12:00:00+00:00"^^xsd:dateTime ;
	dct:modified "2017-07-04T12:00:00+00:00"^^xsd:dateTime  ;
	ikos:isObjectOf aspfacet:shootingtype .

aspfacetvalue:air-rifle
	rdf:type skos:Concept ;
	skos:prefLabel	"air rifle"@en-GB ;
	skos:definition	"Shooting event shot over a distance of 10 metres (10.94 yards) from a standing position with a 4.5 mm (0.177 in) calibre air rifle with a maximum weight of 5.5 kg (12.13 lb)."@en-GB ;
	skos:inScheme <http://cv.iptc.org/newscodes/asportfacetvalue/>  ;
	ikos:created "2017-07-04T12:00:00+00:00"^^xsd:dateTime ;
	dct:created "2017-07-04T12:00:00+00:00"^^xsd:dateTime ;
	ikos:modified "2017-07-04T12:00:00+00:00"^^xsd:dateTime ;
	dct:modified "2017-07-04T12:00:00+00:00"^^xsd:dateTime  ;
	ikos:isObjectOf aspfacet:shootingtype .

aspfacetvalue:around-the-world
	rdf:type skos:Concept ;
	skos:prefLabel	"around the world"@en-GB ;
	skos:definition	"Race category: open seas racing"@en-GB ;
	skos:inScheme <http://cv.iptc.org/newscodes/asportfacetvalue/>  ;
	ikos:created "2017-07-04T12:00:00+00:00"^^xsd:dateTime ;
	dct:created "2017-07-04T12:00:00+00:00"^^xsd:dateTime ;
	ikos:modified "2017-07-04T12:00:00+00:00"^^xsd:dateTime ;
	dct:modified "2017-07-04T12:00:00+00:00"^^xsd:dateTime  ;
	ikos:isObjectOf aspfacet:sailingtype .

aspfacetvalue:artistic-skiing
	rdf:type skos:Concept ;
	skos:prefLabel	"artistic skiing"@en-GB ;
	skos:definition	"Competitors perform a series of artistic moves (jumps and twists) all set to music. The use of ski poles is permitted."@en-GB ;
	skos:inScheme <http://cv.iptc.org/newscodes/asportfacetvalue/>  ;
	ikos:created "2017-07-04T12:00:00+00:00"^^xsd:dateTime ;
	dct:created "2017-07-04T12:00:00+00:00"^^xsd:dateTime ;
	ikos:modified "2017-07-04T12:00:00+00:00"^^xsd:dateTime ;
	dct:modified "2017-07-04T12:00:00+00:00"^^xsd:dateTime  ;
	ikos:isObjectOf aspfacet:freestyleskiingtype .

aspfacetvalue:backstroke
	rdf:type skos:Concept ;
	skos:prefLabel	"backstroke"@en-GB ;
	skos:definition	"Swimming style, on the back, legs move in flapping motion whilst arms propel the swimmer forward."@en-GB ;
	skos:inScheme <http://cv.iptc.org/newscodes/asportfacetvalue/>  ;
	ikos:created "2017-07-04T12:00:00+00:00"^^xsd:dateTime ;
	dct:created "2017-07-04T12:00:00+00:00"^^xsd:dateTime ;
	ikos:modified "2017-07-04T12:00:00+00:00"^^xsd:dateTime ;
	dct:modified "2017-07-04T12:00:00+00:00"^^xsd:dateTime  ;
	ikos:isObjectOf aspfacet:swimmingtype .

aspfacetvalue:ball
	rdf:type skos:Concept ;
	skos:prefLabel	"ball"@en-GB ;
	skos:definition	"Rhythmic gymnastics event using rubber or plastic ball that is 18 to 20 cm in diameter and having a minimum weight of 400g"@en-GB ;
	skos:inScheme <http://cv.iptc.org/newscodes/asportfacetvalue/>  ;
	ikos:created "2017-07-04T12:00:00+00:00"^^xsd:dateTime ;
	dct:created "2017-07-04T12:00:00+00:00"^^xsd:dateTime ;
	ikos:modified "2017-07-04T12:00:00+00:00"^^xsd:dateTime ;
	dct:modified "2017-07-04T12:00:00+00:00"^^xsd:dateTime  ;
	ikos:isObjectOf aspfacet:rhythmgymtype .

aspfacetvalue:bare-hand
	rdf:type skos:Concept ;
	skos:prefLabel	"bare hand"@en-GB ;
	skos:definition	"The *Main Nue* (bare hand) is the ancestor of all Basque sports. "@en-GB ;
	skos:inScheme <http://cv.iptc.org/newscodes/asportfacetvalue/>  ;
	ikos:created "2017-07-04T12:00:00+00:00"^^xsd:dateTime ;
	dct:created "2017-07-04T12:00:00+00:00"^^xsd:dateTime ;
	ikos:modified "2017-07-04T12:00:00+00:00"^^xsd:dateTime ;
	dct:modified "2017-07-04T12:00:00+00:00"^^xsd:dateTime  ;
	ikos:isObjectOf aspfacet:jaialaitype .

aspfacetvalue:beam
	rdf:type skos:Concept ;
	skos:prefLabel	"beam"@en-GB ;
	skos:definition	"Artistic gymnastics event where gymnasts perform leaps and flips from a balance beam that is 10 cm wide."@en-GB ;
	skos:inScheme <http://cv.iptc.org/newscodes/asportfacetvalue/>  ;
	ikos:created "2017-07-04T12:00:00+00:00"^^xsd:dateTime ;
	dct:created "2017-07-04T12:00:00+00:00"^^xsd:dateTime ;
	ikos:modified "2017-07-04T12:00:00+00:00"^^xsd:dateTime ;
	dct:modified "2017-07-04T12:00:00+00:00"^^xsd:dateTime  ;
	ikos:isObjectOf aspfacet:artisticgymtype .

aspfacetvalue:bi-crossing
	rdf:type skos:Concept ;
	skos:prefLabel	"bi-crossing"@en-GB ;
	skos:definition	"Cycling race where competitors have to cover a circuit with obstacles as quickly as possible."@en-GB ;
	skos:inScheme <http://cv.iptc.org/newscodes/asportfacetvalue/>  ;
	ikos:created "2017-07-04T12:00:00+00:00"^^xsd:dateTime ;
	dct:created "2017-07-04T12:00:00+00:00"^^xsd:dateTime ;
	ikos:modified "2017-07-04T12:00:00+00:00"^^xsd:dateTime ;
	dct:modified "2017-07-04T12:00:00+00:00"^^xsd:dateTime  ;
	ikos:isObjectOf aspfacet:cyclingtype .

aspfacetvalue:breaststroke
	rdf:type skos:Concept ;
	skos:prefLabel	"breaststroke"@en-GB ;
	skos:definition	"Swimming style, on the front, effecting forward and outward push movements with the arms and backward and outward pushes with the legs."@en-GB ;
	skos:inScheme <http://cv.iptc.org/newscodes/asportfacetvalue/>  ;
	ikos:created "2017-07-04T12:00:00+00:00"^^xsd:dateTime ;
	dct:created "2017-07-04T12:00:00+00:00"^^xsd:dateTime ;
	ikos:modified "2017-07-04T12:00:00+00:00"^^xsd:dateTime ;
	dct:modified "2017-07-04T12:00:00+00:00"^^xsd:dateTime  ;
	ikos:isObjectOf aspfacet:swimmingtype .

aspfacetvalue:butterfly
	rdf:type skos:Concept ;
	skos:prefLabel	"butterfly"@en-GB ;
	skos:definition	"Swimming style, swum on the front with the shoulders remaining parallel to the water both arms moving in simultaneous windmill fashion, the legs remain together and are moved in a flapping motion."@en-GB ;
	skos:inScheme <http://cv.iptc.org/newscodes/asportfacetvalue/>  ;
	ikos:created "2017-07-04T12:00:00+00:00"^^xsd:dateTime ;
	dct:created "2017-07-04T12:00:00+00:00"^^xsd:dateTime ;
	ikos:modified "2017-07-04T12:00:00+00:00"^^xsd:dateTime ;
	dct:modified "2017-07-04T12:00:00+00:00"^^xsd:dateTime  ;
	ikos:isObjectOf aspfacet:swimmingtype .

aspfacetvalue:canoe-sailing
	rdf:type skos:Concept ;
	skos:prefLabel	"canoe sailing"@en-GB ;
	skos:definition	"A race involving a canoe equipped with a sail."@en-GB ;
	skos:inScheme <http://cv.iptc.org/newscodes/asportfacetvalue/>  ;
	ikos:created "2017-07-04T12:00:00+00:00"^^xsd:dateTime ;
	dct:created "2017-07-04T12:00:00+00:00"^^xsd:dateTime ;
	ikos:modified "2017-07-04T12:00:00+00:00"^^xsd:dateTime ;
	dct:modified "2017-07-04T12:00:00+00:00"^^xsd:dateTime  ;
	ikos:isObjectOf aspfacet:canoekayaktype .

aspfacetvalue:chistera-ancha
	rdf:type skos:Concept ;
	skos:prefLabel	"chistera ancha"@en-GB ;
	skos:definition	"The *chistera-ancha* also called the *cesta punta* is the game played in a *ja√Ø alai* with 1 or 2 players in each team. The players use a long curved basket called the *chistera* (68 cm long and 13 cm wide). "@en-GB ;
	skos:inScheme <http://cv.iptc.org/newscodes/asportfacetvalue/>  ;
	ikos:created "2017-07-04T12:00:00+00:00"^^xsd:dateTime ;
	dct:created "2017-07-04T12:00:00+00:00"^^xsd:dateTime ;
	ikos:modified "2017-07-04T12:00:00+00:00"^^xsd:dateTime ;
	dct:modified "2017-07-04T12:00:00+00:00"^^xsd:dateTime  ;
	ikos:isObjectOf aspfacet:jaialaitype .

aspfacetvalue:chistera-corta
	rdf:type skos:Concept ;
	skos:prefLabel	"chistera corta"@en-GB ;
	skos:definition	"The *chistera-corta* is the game played in a fronton *place libre* with left hand wall and 3 players in each team. The players use a long curved basket called the *chistera* (56 cm long and 12 cm wide). "@en-GB ;
	skos:inScheme <http://cv.iptc.org/newscodes/asportfacetvalue/>  ;
	ikos:created "2017-07-04T12:00:00+00:00"^^xsd:dateTime ;
	dct:created "2017-07-04T12:00:00+00:00"^^xsd:dateTime ;
	ikos:modified "2017-07-04T12:00:00+00:00"^^xsd:dateTime ;
	dct:modified "2017-07-04T12:00:00+00:00"^^xsd:dateTime  ;
	ikos:isObjectOf aspfacet:jaialaitype .

aspfacetvalue:classic
	rdf:type skos:Concept ;
	skos:prefLabel	"classic"@en-GB ;
	skos:definition	"The basic method of propulsion over undulating terrain, by using a striding action, with extra momentum provided by pushing with the poles diagonally opposite to the skis."@en-GB ;
	skos:note	"Moved from *nordicskiingtype* to *crosscountryskiingtype* in August 2019"@en-GB ;
	skos:inScheme <http://cv.iptc.org/newscodes/asportfacetvalue/>  ;
	ikos:created "2017-07-04T12:00:00+00:00"^^xsd:dateTime ;
	dct:created "2017-07-04T12:00:00+00:00"^^xsd:dateTime ;
	ikos:modified "2017-07-04T12:00:00+00:00"^^xsd:dateTime ;
	dct:modified "2017-07-04T12:00:00+00:00"^^xsd:dateTime  ;
	ikos:isObjectOf aspfacet:crosscountryskiingtype .

aspfacetvalue:clean-and-jerk
	rdf:type skos:Concept ;
	skos:prefLabel	"clean and jerk"@en-GB ;
	skos:definition	"The bar is first lifted to the shoulders and then jerk it above the head and keep it there while maintaining straight legs"@en-GB ;
	skos:inScheme <http://cv.iptc.org/newscodes/asportfacetvalue/>  ;
	ikos:created "2017-07-04T12:00:00+00:00"^^xsd:dateTime ;
	dct:created "2017-07-04T12:00:00+00:00"^^xsd:dateTime ;
	ikos:modified "2017-07-04T12:00:00+00:00"^^xsd:dateTime ;
	dct:modified "2017-07-04T12:00:00+00:00"^^xsd:dateTime  ;
	ikos:isObjectOf aspfacet:weightliftingtype .

aspfacetvalue:clubs
	rdf:type skos:Concept ;
	skos:prefLabel	"clubs"@en-GB ;
	skos:definition	"Rhythmic gymnastics event where clubs are passed and tossed"@en-GB ;
	skos:inScheme <http://cv.iptc.org/newscodes/asportfacetvalue/>  ;
	ikos:created "2017-07-04T12:00:00+00:00"^^xsd:dateTime ;
	dct:created "2017-07-04T12:00:00+00:00"^^xsd:dateTime ;
	ikos:modified "2017-07-04T12:00:00+00:00"^^xsd:dateTime ;
	dct:modified "2017-07-04T12:00:00+00:00"^^xsd:dateTime  ;
	ikos:isObjectOf aspfacet:rhythmgymtype .

aspfacetvalue:combined-alpineskiing
	rdf:type skos:Concept ;
	skos:prefLabel	"combined"@en-GB ;
	skos:definition	"Race, usually competed over two days that combines a downhill leg and a slalom leg rewarding the most complete skiers. Combined fastest time wins."@en-GB ;
	skos:inScheme <http://cv.iptc.org/newscodes/asportfacetvalue/>  ;
	ikos:created "2017-07-04T12:00:00+00:00"^^xsd:dateTime ;
	dct:created "2017-07-04T12:00:00+00:00"^^xsd:dateTime ;
	ikos:modified "2017-07-04T12:00:00+00:00"^^xsd:dateTime ;
	dct:modified "2017-07-04T12:00:00+00:00"^^xsd:dateTime  ;
	ikos:isObjectOf aspfacet:alpineskiingtype .

aspfacetvalue:combined-nordicskiing
	rdf:type skos:Concept ;
	skos:prefLabel	"combined"@en-GB ;
	skos:definition	"Competition combining cross-country skiing and ski jumping"@en-GB ;
	skos:note	"Moved from *nordicskiingtype* to *crosscountryskiingtype* in August 2019"@en-GB ;
	skos:inScheme <http://cv.iptc.org/newscodes/asportfacetvalue/>  ;
	ikos:created "2017-07-04T12:00:00+00:00"^^xsd:dateTime ;
	dct:created "2017-07-04T12:00:00+00:00"^^xsd:dateTime ;
	ikos:modified "2017-07-04T12:00:00+00:00"^^xsd:dateTime ;
	dct:modified "2017-07-04T12:00:00+00:00"^^xsd:dateTime  ;
	ikos:isObjectOf aspfacet:crosscountryskiingtype .

aspfacetvalue:combined-waterskiing
	rdf:type skos:Concept ;
	skos:prefLabel	"combined"@en-GB ;
	skos:definition	"A combined event made up of the slalom, jump and trick"@en-GB ;
	skos:inScheme <http://cv.iptc.org/newscodes/asportfacetvalue/>  ;
	ikos:created "2017-07-04T12:00:00+00:00"^^xsd:dateTime ;
	dct:created "2017-07-04T12:00:00+00:00"^^xsd:dateTime ;
	ikos:modified "2017-07-04T12:00:00+00:00"^^xsd:dateTime ;
	dct:modified "2017-07-04T12:00:00+00:00"^^xsd:dateTime  ;
	ikos:isObjectOf aspfacet:waterskiingtype .

aspfacetvalue:coxless
	rdf:type skos:Concept ;
	skos:prefLabel	"coxless"@en-GB ;
	skos:definition	"one oar each and without a team mate to give directions"@en-GB ;
	skos:inScheme <http://cv.iptc.org/newscodes/asportfacetvalue/>  ;
	ikos:created "2017-07-04T12:00:00+00:00"^^xsd:dateTime ;
	dct:created "2017-07-04T12:00:00+00:00"^^xsd:dateTime ;
	ikos:modified "2017-07-04T12:00:00+00:00"^^xsd:dateTime ;
	dct:modified "2017-07-04T12:00:00+00:00"^^xsd:dateTime  ;
	ikos:isObjectOf aspfacet:rowingtype .

aspfacetvalue:cross-country-equestrian
	rdf:type skos:Concept ;
	skos:prefLabel	"cross country"@en-GB ;
	skos:definition	"Equestrian event held on a designated circuit in the countryside featuring artificial and natural obstacles."@en-GB ;
	skos:inScheme <http://cv.iptc.org/newscodes/asportfacetvalue/>  ;
	ikos:created "2017-07-04T12:00:00+00:00"^^xsd:dateTime ;
	dct:created "2017-07-04T12:00:00+00:00"^^xsd:dateTime ;
	ikos:modified "2017-07-04T12:00:00+00:00"^^xsd:dateTime ;
	dct:modified "2017-07-04T12:00:00+00:00"^^xsd:dateTime  ;
	ikos:isObjectOf aspfacet:equestriantype .

aspfacetvalue:cross-country-race
	rdf:type skos:Concept ;
	skos:prefLabel	"cross-country"@en-GB ;
	skos:definition	"A race over natural terrain."@en-GB ;
	skos:inScheme <http://cv.iptc.org/newscodes/asportfacetvalue/>  ;
	ikos:created "2017-07-04T12:00:00+00:00"^^xsd:dateTime ;
	dct:created "2017-07-04T12:00:00+00:00"^^xsd:dateTime ;
	ikos:modified "2017-07-04T12:00:00+00:00"^^xsd:dateTime ;
	dct:modified "2017-07-04T12:00:00+00:00"^^xsd:dateTime  ;
	ikos:isObjectOf aspfacet:racetype .

aspfacetvalue:cyclo-cross
	rdf:type skos:Concept ;
	skos:prefLabel	"cyclo-cross"@en-GB ;
	skos:definition	"A cycling race staged on various surfaces - earth, grass, sand or tarmac."@en-GB ;
	skos:inScheme <http://cv.iptc.org/newscodes/asportfacetvalue/>  ;
	ikos:created "2017-07-04T12:00:00+00:00"^^xsd:dateTime ;
	dct:created "2017-07-04T12:00:00+00:00"^^xsd:dateTime ;
	ikos:modified "2017-07-04T12:00:00+00:00"^^xsd:dateTime ;
	dct:modified "2017-07-04T12:00:00+00:00"^^xsd:dateTime  ;
	ikos:isObjectOf aspfacet:cyclingtype .

aspfacetvalue:DDC
	rdf:type skos:Concept ;
	skos:prefLabel	"DDC"@en-GB ;
	skos:definition	"Abbreviation for Double Disc Court. Two players per team in a square 13x13 metre. The teams start with one disc per team and throw at each other. Discs are thrown back and forth until one or both hit the ground. "@en-GB ;
	skos:inScheme <http://cv.iptc.org/newscodes/asportfacetvalue/>  ;
	ikos:created "2017-07-04T12:00:00+00:00"^^xsd:dateTime ;
	dct:created "2017-07-04T12:00:00+00:00"^^xsd:dateTime ;
	ikos:modified "2017-07-04T12:00:00+00:00"^^xsd:dateTime ;
	dct:modified "2017-07-04T12:00:00+00:00"^^xsd:dateTime  ;
	ikos:isObjectOf aspfacet:flyingdisctype .

aspfacetvalue:discathon
	rdf:type skos:Concept ;
	skos:prefLabel	"discathon"@en-GB ;
	skos:definition	"The object is to throw and run a park course of about 1 kilometre. Four players compete in each heat. They have two discs each. They may also carry a third disc in reserve. Where one thrown disc stops the second disc must be thrown. "@en-GB ;
	skos:inScheme <http://cv.iptc.org/newscodes/asportfacetvalue/>  ;
	ikos:created "2017-07-04T12:00:00+00:00"^^xsd:dateTime ;
	dct:created "2017-07-04T12:00:00+00:00"^^xsd:dateTime ;
	ikos:modified "2017-07-04T12:00:00+00:00"^^xsd:dateTime ;
	dct:modified "2017-07-04T12:00:00+00:00"^^xsd:dateTime  ;
	ikos:isObjectOf aspfacet:flyingdisctype .

aspfacetvalue:disc-golf
	rdf:type skos:Concept ;
	skos:prefLabel	"disc golf"@en-GB ;
	skos:definition	"Much like golf but played with discs instead of balls and clubs. Instead of a hole in the ground there is a metal basket with light metal chains to throw the disc at. Players often carry discs specialized for long throws, right or left bends. "@en-GB ;
	skos:inScheme <http://cv.iptc.org/newscodes/asportfacetvalue/>  ;
	ikos:created "2017-07-04T12:00:00+00:00"^^xsd:dateTime ;
	dct:created "2017-07-04T12:00:00+00:00"^^xsd:dateTime ;
	ikos:modified "2017-07-04T12:00:00+00:00"^^xsd:dateTime ;
	dct:modified "2017-07-04T12:00:00+00:00"^^xsd:dateTime  ;
	ikos:isObjectOf aspfacet:flyingdisctype .

aspfacetvalue:distance
	rdf:type skos:Concept ;
	skos:prefLabel	"distance"@en-GB ;
	skos:definition	"The object is to throw the disc as far as possible. Each player get five throws per turn. Throws are made downwind."@en-GB ;
	skos:inScheme <http://cv.iptc.org/newscodes/asportfacetvalue/>  ;
	ikos:created "2017-07-04T12:00:00+00:00"^^xsd:dateTime ;
	dct:created "2017-07-04T12:00:00+00:00"^^xsd:dateTime ;
	ikos:modified "2017-07-04T12:00:00+00:00"^^xsd:dateTime ;
	dct:modified "2017-07-04T12:00:00+00:00"^^xsd:dateTime  ;
	ikos:isObjectOf aspfacet:flyingdisctype .

aspfacetvalue:double-trap
	rdf:type skos:Concept ;
	skos:prefLabel	"double trap"@en-GB ;
	skos:definition	"Shooting event with two moving targets launched at the same time "@en-GB ;
	skos:inScheme <http://cv.iptc.org/newscodes/asportfacetvalue/>  ;
	ikos:created "2017-07-04T12:00:00+00:00"^^xsd:dateTime ;
	dct:created "2017-07-04T12:00:00+00:00"^^xsd:dateTime ;
	ikos:modified "2017-07-04T12:00:00+00:00"^^xsd:dateTime ;
	dct:modified "2017-07-04T12:00:00+00:00"^^xsd:dateTime  ;
	ikos:isObjectOf aspfacet:shootingtype .

aspfacetvalue:downhill
	rdf:type skos:Concept ;
	skos:prefLabel	"downhill"@en-GB ;
	skos:definition	"Alpine skiing high speed race between widely set gates."@en-GB ;
	skos:inScheme <http://cv.iptc.org/newscodes/asportfacetvalue/>  ;
	ikos:created "2017-07-04T12:00:00+00:00"^^xsd:dateTime ;
	dct:created "2017-07-04T12:00:00+00:00"^^xsd:dateTime ;
	ikos:modified "2017-07-04T12:00:00+00:00"^^xsd:dateTime ;
	dct:modified "2017-07-04T12:00:00+00:00"^^xsd:dateTime  ;
	ikos:isObjectOf aspfacet:alpineskiingtype .

aspfacetvalue:dressage
	rdf:type skos:Concept ;
	skos:prefLabel	"dressage"@en-GB ;
	skos:definition	"A rider is judged on a series of moves at three different paces - walk, trot and gallop."@en-GB ;
	skos:inScheme <http://cv.iptc.org/newscodes/asportfacetvalue/>  ;
	ikos:created "2017-07-04T12:00:00+00:00"^^xsd:dateTime ;
	dct:created "2017-07-04T12:00:00+00:00"^^xsd:dateTime ;
	ikos:modified "2017-07-04T12:00:00+00:00"^^xsd:dateTime ;
	dct:modified "2017-07-04T12:00:00+00:00"^^xsd:dateTime  ;
	ikos:isObjectOf aspfacet:equestriantype .

aspfacetvalue:endurance-equestrian
	rdf:type skos:Concept ;
	skos:prefLabel	"endurance"@en-GB ;
	skos:definition	"Equestrian sport consisting of controlled long-distance races."@en-GB ;
	skos:inScheme <http://cv.iptc.org/newscodes/asportfacetvalue/>  ;
	ikos:created "2017-07-04T12:00:00+00:00"^^xsd:dateTime ;
	dct:created "2017-07-04T12:00:00+00:00"^^xsd:dateTime ;
	ikos:modified "2017-07-04T12:00:00+00:00"^^xsd:dateTime ;
	dct:modified "2017-07-04T12:00:00+00:00"^^xsd:dateTime  ;
	ikos:isObjectOf aspfacet:equestriantype .

aspfacetvalue:endurance-motorcycling
	rdf:type skos:Concept ;
	skos:prefLabel	"endurance"@en-GB ;
	skos:definition	"Motorcycle road race where consistency and endurance is the object."@en-GB ;
	skos:inScheme <http://cv.iptc.org/newscodes/asportfacetvalue/>  ;
	ikos:created "2017-07-04T12:00:00+00:00"^^xsd:dateTime ;
	dct:created "2017-07-04T12:00:00+00:00"^^xsd:dateTime ;
	ikos:modified "2017-07-04T12:00:00+00:00"^^xsd:dateTime ;
	dct:modified "2017-07-04T12:00:00+00:00"^^xsd:dateTime  ;
	ikos:isObjectOf aspfacet:motorcyclingtype .

aspfacetvalue:endurance-motorracing
	rdf:type skos:Concept ;
	skos:prefLabel	"endurance"@en-GB ;
	skos:definition	"Endurance races for a driver and co-pilot using specially built cars."@en-GB ;
	skos:inScheme <http://cv.iptc.org/newscodes/asportfacetvalue/>  ;
	ikos:created "2017-07-04T12:00:00+00:00"^^xsd:dateTime ;
	dct:created "2017-07-04T12:00:00+00:00"^^xsd:dateTime ;
	ikos:modified "2017-07-04T12:00:00+00:00"^^xsd:dateTime ;
	dct:modified "2017-07-04T12:00:00+00:00"^^xsd:dateTime  ;
	ikos:isObjectOf aspfacet:motorcarracingtype .

aspfacetvalue:enduro
	rdf:type skos:Concept ;
	skos:prefLabel	"enduro"@en-GB ;
	skos:definition	"Motrocycle race of speed, endurance and regularity over varied surfaces such as through forests and on dirt tracks."@en-GB ;
	skos:inScheme <http://cv.iptc.org/newscodes/asportfacetvalue/>  ;
	ikos:created "2017-07-04T12:00:00+00:00"^^xsd:dateTime ;
	dct:created "2017-07-04T12:00:00+00:00"^^xsd:dateTime ;
	ikos:modified "2017-07-04T12:00:00+00:00"^^xsd:dateTime ;
	dct:modified "2017-07-04T12:00:00+00:00"^^xsd:dateTime  ;
	ikos:isObjectOf aspfacet:motorcyclingtype .

aspfacetvalue:epee
	rdf:type skos:Concept ;
	skos:prefLabel	"epee"@en-GB ;
	skos:definition	"Category of fencing using a weapon with a triangular cross-section blade and a large bell guard."@en-GB ;
	skos:inScheme <http://cv.iptc.org/newscodes/asportfacetvalue/>  ;
	ikos:created "2017-07-04T12:00:00+00:00"^^xsd:dateTime ;
	dct:created "2017-07-04T12:00:00+00:00"^^xsd:dateTime ;
	ikos:modified "2017-07-04T12:00:00+00:00"^^xsd:dateTime ;
	dct:modified "2017-07-04T12:00:00+00:00"^^xsd:dateTime  ;
	ikos:isObjectOf aspfacet:fencingtype .

aspfacetvalue:europe
	rdf:type skos:Concept ;
	skos:prefLabel	"europe"@en-GB ;
	skos:definition	"Boat Category: one man dinghy (4.57m/sq mainsail) Olympic sport "@en-GB ;
	skos:inScheme <http://cv.iptc.org/newscodes/asportfacetvalue/>  ;
	ikos:created "2017-07-04T12:00:00+00:00"^^xsd:dateTime ;
	dct:created "2017-07-04T12:00:00+00:00"^^xsd:dateTime ;
	ikos:modified "2017-07-04T12:00:00+00:00"^^xsd:dateTime ;
	dct:modified "2017-07-04T12:00:00+00:00"^^xsd:dateTime  ;
	ikos:isObjectOf aspfacet:sailingtype .

aspfacetvalue:eventing
	rdf:type skos:Concept ;
	skos:prefLabel	"eventing"@en-GB ;
	skos:definition	"Equestrian event involving three disciplines - Dressage, cross-country and show jumping."@en-GB ;
	skos:inScheme <http://cv.iptc.org/newscodes/asportfacetvalue/>  ;
	ikos:created "2017-07-04T12:00:00+00:00"^^xsd:dateTime ;
	dct:created "2017-07-04T12:00:00+00:00"^^xsd:dateTime ;
	ikos:modified "2017-07-04T12:00:00+00:00"^^xsd:dateTime ;
	dct:modified "2017-07-04T12:00:00+00:00"^^xsd:dateTime  ;
	ikos:isObjectOf aspfacet:equestriantype .

aspfacetvalue:F3000
	rdf:type skos:Concept ;
	skos:prefLabel	"F3000"@en-GB ;
	skos:definition	"Using less powerful motors than the Formula One, designated construction teams race over varied circuits the world over in speed races for individual and team honours over a season. "@en-GB ;
	skos:inScheme <http://cv.iptc.org/newscodes/asportfacetvalue/>  ;
	ikos:created "2017-07-04T12:00:00+00:00"^^xsd:dateTime ;
	dct:created "2017-07-04T12:00:00+00:00"^^xsd:dateTime ;
	ikos:modified "2017-07-04T12:00:00+00:00"^^xsd:dateTime ;
	dct:modified "2017-07-04T12:00:00+00:00"^^xsd:dateTime  ;
	ikos:isObjectOf aspfacet:motorcarracingtype .

aspfacetvalue:finn
	rdf:type skos:Concept ;
	skos:prefLabel	"finn"@en-GB ;
	skos:definition	"Boat Category: one man dinghy (10m/sq mainsail) Olympic sport "@en-GB ;
	skos:inScheme <http://cv.iptc.org/newscodes/asportfacetvalue/>  ;
	ikos:created "2017-07-04T12:00:00+00:00"^^xsd:dateTime ;
	dct:created "2017-07-04T12:00:00+00:00"^^xsd:dateTime ;
	ikos:modified "2017-07-04T12:00:00+00:00"^^xsd:dateTime ;
	dct:modified "2017-07-04T12:00:00+00:00"^^xsd:dateTime  ;
	ikos:isObjectOf aspfacet:sailingtype .

aspfacetvalue:flatland
	rdf:type skos:Concept ;
	skos:prefLabel	"flatland"@en-GB ;
	skos:definition	"BMX on a smooth, flat surface. Tricks involve spinning and balancing in a variety of body and bicycle positions."@en-GB ;
	skos:inScheme <http://cv.iptc.org/newscodes/asportfacetvalue/>  ;
	ikos:created "2017-07-04T12:00:00+00:00"^^xsd:dateTime ;
	dct:created "2017-07-04T12:00:00+00:00"^^xsd:dateTime ;
	ikos:modified "2017-07-04T12:00:00+00:00"^^xsd:dateTime ;
	dct:modified "2017-07-04T12:00:00+00:00"^^xsd:dateTime  ;
	ikos:isObjectOf aspfacet:bmxfreestyletype .

aspfacetvalue:flat-racing
	rdf:type skos:Concept ;
	skos:prefLabel	"flat racing"@en-GB ;
	skos:definition	"Horse race run on a level racecourse."@en-GB ;
	skos:inScheme <http://cv.iptc.org/newscodes/asportfacetvalue/>  ;
	ikos:created "2017-07-04T12:00:00+00:00"^^xsd:dateTime ;
	dct:created "2017-07-04T12:00:00+00:00"^^xsd:dateTime ;
	ikos:modified "2017-07-04T12:00:00+00:00"^^xsd:dateTime ;
	dct:modified "2017-07-04T12:00:00+00:00"^^xsd:dateTime  ;
	ikos:isObjectOf aspfacet:horseracingtype .

aspfacetvalue:floorexercise
	rdf:type skos:Concept ;
	skos:prefLabel	"floor exercise"@en-GB ;
	skos:definition	"Artistic gymnastics event where floor exercises are performed on a 12m/sq matt."@en-GB ;
	skos:inScheme <http://cv.iptc.org/newscodes/asportfacetvalue/>  ;
	ikos:created "2017-07-04T12:00:00+00:00"^^xsd:dateTime ;
	dct:created "2017-07-04T12:00:00+00:00"^^xsd:dateTime ;
	ikos:modified "2017-07-04T12:00:00+00:00"^^xsd:dateTime ;
	dct:modified "2017-07-04T12:00:00+00:00"^^xsd:dateTime  ;
	ikos:isObjectOf aspfacet:artisticgymtype .

aspfacetvalue:flying-dutchman
	rdf:type skos:Concept ;
	skos:prefLabel	"flying dutchman"@en-GB ;
	skos:definition	"Boat Category: two man dinghy "@en-GB ;
	skos:inScheme <http://cv.iptc.org/newscodes/asportfacetvalue/>  ;
	ikos:created "2017-07-04T12:00:00+00:00"^^xsd:dateTime ;
	dct:created "2017-07-04T12:00:00+00:00"^^xsd:dateTime ;
	ikos:modified "2017-07-04T12:00:00+00:00"^^xsd:dateTime ;
	dct:modified "2017-07-04T12:00:00+00:00"^^xsd:dateTime  ;
	ikos:isObjectOf aspfacet:sailingtype .

aspfacetvalue:foil
	rdf:type skos:Concept ;
	skos:prefLabel	"foil"@en-GB ;
	skos:definition	"Category of fencing using a weapon with a rectangular cross-section blade and a small bell guard."@en-GB ;
	skos:inScheme <http://cv.iptc.org/newscodes/asportfacetvalue/>  ;
	ikos:created "2017-07-04T12:00:00+00:00"^^xsd:dateTime ;
	dct:created "2017-07-04T12:00:00+00:00"^^xsd:dateTime ;
	ikos:modified "2017-07-04T12:00:00+00:00"^^xsd:dateTime ;
	dct:modified "2017-07-04T12:00:00+00:00"^^xsd:dateTime  ;
	ikos:isObjectOf aspfacet:fencingtype .

aspfacetvalue:folkrace
	rdf:type skos:Concept ;
	skos:prefLabel	"folkrace"@en-GB ;
	skos:definition	""@en-GB ;
	skos:inScheme <http://cv.iptc.org/newscodes/asportfacetvalue/>  ;
	ikos:created "2019-11-25T12:00:00+00:00"^^xsd:dateTime ;
	dct:created "2019-11-25T12:00:00+00:00"^^xsd:dateTime ;
	ikos:modified "2019-11-25T12:00:00+00:00"^^xsd:dateTime ;
	dct:modified "2019-11-25T12:00:00+00:00"^^xsd:dateTime  ;
	ikos:isObjectOf aspfacet:motorcarracingtype .

aspfacetvalue:formulaone
	rdf:type skos:Concept ;
	skos:prefLabel	"formula one"@en-GB ;
	skos:definition	"Single cockpit car racing where 20 or so competitors race head to head over varied circuits around the world to win Grand Prix points in an individual and constructors championship "@en-GB ;
	skos:inScheme <http://cv.iptc.org/newscodes/asportfacetvalue/>  ;
	ikos:created "2017-07-04T12:00:00+00:00"^^xsd:dateTime ;
	dct:created "2017-07-04T12:00:00+00:00"^^xsd:dateTime ;
	ikos:modified "2017-07-04T12:00:00+00:00"^^xsd:dateTime ;
	dct:modified "2017-07-04T12:00:00+00:00"^^xsd:dateTime  ;
	ikos:isObjectOf aspfacet:motorcarracingtype .

aspfacetvalue:freestyle-flyingdisc
	rdf:type skos:Concept ;
	skos:prefLabel	"freestyle"@en-GB ;
	skos:definition	"A judged event where groups of two or three players perform as many tricks as possible. In competitions the judges can use either a ranking system or set scores on presentation, execution and difficulty. "@en-GB ;
	skos:inScheme <http://cv.iptc.org/newscodes/asportfacetvalue/>  ;
	ikos:created "2017-07-04T12:00:00+00:00"^^xsd:dateTime ;
	dct:created "2017-07-04T12:00:00+00:00"^^xsd:dateTime ;
	ikos:modified "2017-07-04T12:00:00+00:00"^^xsd:dateTime ;
	dct:modified "2017-07-04T12:00:00+00:00"^^xsd:dateTime  ;
	ikos:isObjectOf aspfacet:flyingdisctype .

aspfacetvalue:freestyle-swimming
	rdf:type skos:Concept ;
	skos:prefLabel	"freestyle"@en-GB ;
	skos:definition	"Any swimming style may be employed, though front crawl is universally employed."@en-GB ;
	skos:inScheme <http://cv.iptc.org/newscodes/asportfacetvalue/>  ;
	ikos:created "2017-07-04T12:00:00+00:00"^^xsd:dateTime ;
	dct:created "2017-07-04T12:00:00+00:00"^^xsd:dateTime ;
	ikos:modified "2017-07-04T12:00:00+00:00"^^xsd:dateTime ;
	dct:modified "2017-07-04T12:00:00+00:00"^^xsd:dateTime  ;
	ikos:isObjectOf aspfacet:swimmingtype .

aspfacetvalue:fronton
	rdf:type skos:Concept ;
	skos:prefLabel	"fronton"@en-GB ;
	skos:definition	"The *fronton* known as *Fronton Place Libre* consists of a rectangular outdoor court plus a large pink shaped wall at one end. The two sides and the other end are left opened. "@en-GB ;
	skos:inScheme <http://cv.iptc.org/newscodes/asportfacetvalue/>  ;
	ikos:created "2017-07-04T12:00:00+00:00"^^xsd:dateTime ;
	dct:created "2017-07-04T12:00:00+00:00"^^xsd:dateTime ;
	ikos:modified "2017-07-04T12:00:00+00:00"^^xsd:dateTime ;
	dct:modified "2017-07-04T12:00:00+00:00"^^xsd:dateTime  ;
	ikos:isObjectOf aspfacet:jaialaitype .

aspfacetvalue:futsal
	rdf:type skos:Concept ;
	skos:prefLabel	"futsal"@en-GB ;
	skos:definition	""@en-GB ;
	skos:inScheme <http://cv.iptc.org/newscodes/asportfacetvalue/>  ;
	ikos:created "2019-11-25T12:00:00+00:00"^^xsd:dateTime ;
	dct:created "2019-11-25T12:00:00+00:00"^^xsd:dateTime ;
	ikos:modified "2019-11-25T12:00:00+00:00"^^xsd:dateTime ;
	dct:modified "2019-11-25T12:00:00+00:00"^^xsd:dateTime  ;
	ikos:isObjectOf aspfacet:soccertype .

aspfacetvalue:giantslalom-alpineskiing
	rdf:type skos:Concept ;
	skos:prefLabel	"giant slalom"@en-GB ;
	skos:definition	"Timed race between poles or gates. Total time in two heats. "@en-GB ;
	skos:inScheme <http://cv.iptc.org/newscodes/asportfacetvalue/>  ;
	ikos:created "2017-07-04T12:00:00+00:00"^^xsd:dateTime ;
	dct:created "2017-07-04T12:00:00+00:00"^^xsd:dateTime ;
	ikos:modified "2017-07-04T12:00:00+00:00"^^xsd:dateTime ;
	dct:modified "2017-07-04T12:00:00+00:00"^^xsd:dateTime  ;
	ikos:isObjectOf aspfacet:alpineskiingtype .

aspfacetvalue:giantslalom-snowboarding
	rdf:type skos:Concept ;
	skos:prefLabel	"giant slalom"@en-GB ;
	skos:definition	"Race between poles or gates, longer and wider than slalom."@en-GB ;
	skos:inScheme <http://cv.iptc.org/newscodes/asportfacetvalue/>  ;
	ikos:created "2017-07-04T12:00:00+00:00"^^xsd:dateTime ;
	dct:created "2017-07-04T12:00:00+00:00"^^xsd:dateTime ;
	ikos:modified "2017-07-04T12:00:00+00:00"^^xsd:dateTime ;
	dct:modified "2017-07-04T12:00:00+00:00"^^xsd:dateTime  ;
	ikos:isObjectOf aspfacet:snowboardingtype .

aspfacetvalue:grandprix
	rdf:type skos:Concept ;
	skos:prefLabel	"grand prix"@en-GB ;
	skos:definition	"A race with Grand Prix motorcycles"@en-GB ;
	skos:inScheme <http://cv.iptc.org/newscodes/asportfacetvalue/>  ;
	ikos:created "2017-07-04T12:00:00+00:00"^^xsd:dateTime ;
	dct:created "2017-07-04T12:00:00+00:00"^^xsd:dateTime ;
	ikos:modified "2017-07-04T12:00:00+00:00"^^xsd:dateTime ;
	dct:modified "2017-07-04T12:00:00+00:00"^^xsd:dateTime  ;
	ikos:isObjectOf aspfacet:motorcyclingtype .

aspfacetvalue:grasstrack
	rdf:type skos:Concept ;
	skos:prefLabel	"grass track"@en-GB ;
	skos:definition	"Horse race competed on turf."@en-GB ;
	skos:inScheme <http://cv.iptc.org/newscodes/asportfacetvalue/>  ;
	ikos:created "2017-07-04T12:00:00+00:00"^^xsd:dateTime ;
	dct:created "2017-07-04T12:00:00+00:00"^^xsd:dateTime ;
	ikos:modified "2017-07-04T12:00:00+00:00"^^xsd:dateTime ;
	dct:modified "2017-07-04T12:00:00+00:00"^^xsd:dateTime  ;
	ikos:isObjectOf aspfacet:horseracingtype .

aspfacetvalue:guts
	rdf:type skos:Concept ;
	skos:prefLabel	"guts"@en-GB ;
	skos:definition	"Team game where two teams of 5 players each face each other. Teams take turns to throw the disc towards the other team. Points are scored if the opposing team does not catch the disc. "@en-GB ;
	skos:inScheme <http://cv.iptc.org/newscodes/asportfacetvalue/>  ;
	ikos:created "2017-07-04T12:00:00+00:00"^^xsd:dateTime ;
	dct:created "2017-07-04T12:00:00+00:00"^^xsd:dateTime ;
	ikos:modified "2017-07-04T12:00:00+00:00"^^xsd:dateTime ;
	dct:modified "2017-07-04T12:00:00+00:00"^^xsd:dateTime  ;
	ikos:isObjectOf aspfacet:flyingdisctype .

aspfacetvalue:harnessracing
	rdf:type skos:Concept ;
	skos:prefLabel	"harness racing"@en-GB ;
	skos:definition	"Horses hitched to a jockeyed buggy race round a flat course. Can be performed at a trotting gait or a pacing gait. "@en-GB ;
	skos:inScheme <http://cv.iptc.org/newscodes/asportfacetvalue/>  ;
	ikos:created "2017-07-04T12:00:00+00:00"^^xsd:dateTime ;
	dct:created "2017-07-04T12:00:00+00:00"^^xsd:dateTime ;
	ikos:modified "2017-07-04T12:00:00+00:00"^^xsd:dateTime ;
	dct:modified "2017-07-04T12:00:00+00:00"^^xsd:dateTime  ;
	ikos:isObjectOf aspfacet:horseracingtype .

aspfacetvalue:hoop
	rdf:type skos:Concept ;
	skos:prefLabel	"hoop"@en-GB ;
	skos:definition	"Rhythmic gymnastics event where a hoop is rolled and thrown"@en-GB ;
	skos:inScheme <http://cv.iptc.org/newscodes/asportfacetvalue/>  ;
	ikos:created "2017-07-04T12:00:00+00:00"^^xsd:dateTime ;
	dct:created "2017-07-04T12:00:00+00:00"^^xsd:dateTime ;
	ikos:modified "2017-07-04T12:00:00+00:00"^^xsd:dateTime ;
	dct:modified "2017-07-04T12:00:00+00:00"^^xsd:dateTime  ;
	ikos:isObjectOf aspfacet:rhythmgymtype .

aspfacetvalue:horizontalbar
	rdf:type skos:Concept ;
	skos:prefLabel	"horizontal bar"@en-GB ;
	skos:definition	"Artistic gymnastics event where gymnasts turn, spin and perform pirouettes around the horizontal bar."@en-GB ;
	skos:inScheme <http://cv.iptc.org/newscodes/asportfacetvalue/>  ;
	ikos:created "2017-07-04T12:00:00+00:00"^^xsd:dateTime ;
	dct:created "2017-07-04T12:00:00+00:00"^^xsd:dateTime ;
	ikos:modified "2017-07-04T12:00:00+00:00"^^xsd:dateTime ;
	dct:modified "2017-07-04T12:00:00+00:00"^^xsd:dateTime  ;
	ikos:isObjectOf aspfacet:artisticgymtype .

aspfacetvalue:horse-driving
	rdf:type skos:Concept ;
	skos:prefLabel	"horse driving"@en-GB ;
	skos:definition	"Equestrian events involving horses being driven in harness, single vehicle around a course."@en-GB ;
	skos:inScheme <http://cv.iptc.org/newscodes/asportfacetvalue/>  ;
	ikos:created "2017-07-04T12:00:00+00:00"^^xsd:dateTime ;
	dct:created "2017-07-04T12:00:00+00:00"^^xsd:dateTime ;
	ikos:modified "2017-07-04T12:00:00+00:00"^^xsd:dateTime ;
	dct:modified "2017-07-04T12:00:00+00:00"^^xsd:dateTime  ;
	ikos:isObjectOf aspfacet:equestriantype .

aspfacetvalue:ice-dance
	rdf:type skos:Concept ;
	skos:prefLabel	"ice dance"@en-GB ;
	skos:definition	"Skating event that takes place over three days with, in order, two compulsory dances, the original dance (2min 30sec) and the free dance (4min)"@en-GB ;
	skos:inScheme <http://cv.iptc.org/newscodes/asportfacetvalue/>  ;
	ikos:created "2017-07-04T12:00:00+00:00"^^xsd:dateTime ;
	dct:created "2017-07-04T12:00:00+00:00"^^xsd:dateTime ;
	ikos:modified "2017-07-04T12:00:00+00:00"^^xsd:dateTime ;
	dct:modified "2017-07-04T12:00:00+00:00"^^xsd:dateTime  ;
	ikos:isObjectOf aspfacet:figureskatingtype .

aspfacetvalue:beach-football
	rdf:type skos:Concept ;
	skos:prefLabel	"beach football"@en-GB ;
	skos:definition	"A form of association football played on a soft-sand surface and a smaller pitch which allows for numerous goal attempts"@en-GB ;
	skos:inScheme <http://cv.iptc.org/newscodes/asportfacetvalue/>  ;
	ikos:created "2019-11-25T12:00:00+00:00"^^xsd:dateTime ;
	dct:created "2019-11-25T12:00:00+00:00"^^xsd:dateTime ;
	ikos:modified "2019-11-25T12:00:00+00:00"^^xsd:dateTime ;
	dct:modified "2019-11-25T12:00:00+00:00"^^xsd:dateTime  ;
	ikos:isObjectOf aspfacet:soccertype .

aspfacetvalue:indoor-soccer
	rdf:type skos:Concept ;
	skos:prefLabel	"indoor soccer"@en-GB ;
	skos:definition	""@en-GB ;
	skos:inScheme <http://cv.iptc.org/newscodes/asportfacetvalue/>  ;
	ikos:created "2019-11-25T12:00:00+00:00"^^xsd:dateTime ;
	dct:created "2019-11-25T12:00:00+00:00"^^xsd:dateTime ;
	ikos:modified "2019-11-25T12:00:00+00:00"^^xsd:dateTime ;
	dct:modified "2019-11-25T12:00:00+00:00"^^xsd:dateTime  ;
	ikos:isObjectOf aspfacet:soccertype .

aspfacetvalue:indyracing
	rdf:type skos:Concept ;
	skos:prefLabel	"indy racing"@en-GB ;
	skos:definition	"North American top range professional league speed racing over circuits. "@en-GB ;
	skos:inScheme <http://cv.iptc.org/newscodes/asportfacetvalue/>  ;
	ikos:created "2017-07-04T12:00:00+00:00"^^xsd:dateTime ;
	dct:created "2017-07-04T12:00:00+00:00"^^xsd:dateTime ;
	ikos:modified "2017-07-04T12:00:00+00:00"^^xsd:dateTime ;
	dct:modified "2017-07-04T12:00:00+00:00"^^xsd:dateTime  ;
	ikos:isObjectOf aspfacet:motorcarracingtype .

aspfacetvalue:jump
	rdf:type skos:Concept ;
	skos:prefLabel	"jump"@en-GB ;
	skos:definition	"Skiers perform as long a jump as possible from a ramp in the water"@en-GB ;
	skos:inScheme <http://cv.iptc.org/newscodes/asportfacetvalue/>  ;
	ikos:created "2017-07-04T12:00:00+00:00"^^xsd:dateTime ;
	dct:created "2017-07-04T12:00:00+00:00"^^xsd:dateTime ;
	ikos:modified "2017-07-04T12:00:00+00:00"^^xsd:dateTime ;
	dct:modified "2017-07-04T12:00:00+00:00"^^xsd:dateTime  ;
	ikos:isObjectOf aspfacet:waterskiingtype .

aspfacetvalue:jumping
	rdf:type skos:Concept ;
	skos:prefLabel	"jumping"@en-GB ;
	skos:definition	"A rider and horse attempt to jump a series of obstacles in an enclosed arena against the clock."@en-GB ;
	skos:inScheme <http://cv.iptc.org/newscodes/asportfacetvalue/>  ;
	ikos:created "2017-07-04T12:00:00+00:00"^^xsd:dateTime ;
	dct:created "2017-07-04T12:00:00+00:00"^^xsd:dateTime ;
	ikos:modified "2017-07-04T12:00:00+00:00"^^xsd:dateTime ;
	dct:modified "2017-07-04T12:00:00+00:00"^^xsd:dateTime  ;
	ikos:isObjectOf aspfacet:equestriantype .

aspfacetvalue:kart-racing
	rdf:type skos:Concept ;
	skos:prefLabel	"kart racing"@en-GB ;
	skos:definition	""@en-GB ;
	skos:inScheme <http://cv.iptc.org/newscodes/asportfacetvalue/>  ;
	ikos:created "2019-11-25T12:00:00+00:00"^^xsd:dateTime ;
	dct:created "2019-11-25T12:00:00+00:00"^^xsd:dateTime ;
	ikos:modified "2019-11-25T12:00:00+00:00"^^xsd:dateTime ;
	dct:modified "2019-11-25T12:00:00+00:00"^^xsd:dateTime  ;
	ikos:isObjectOf aspfacet:motorcarracingtype .

aspfacetvalue:keirin
	rdf:type skos:Concept ;
	skos:prefLabel	"keirin"@en-GB ;
	skos:definition	"Sprint between six cyclists where a pacemaker on a moped gradually increases the pace over the first 1400m. When the pacemaker leaves the track the race develops into a sprint finish over the final 6-700m."@en-GB ;
	skos:inScheme <http://cv.iptc.org/newscodes/asportfacetvalue/>  ;
	ikos:created "2017-07-04T12:00:00+00:00"^^xsd:dateTime ;
	dct:created "2017-07-04T12:00:00+00:00"^^xsd:dateTime ;
	ikos:modified "2017-07-04T12:00:00+00:00"^^xsd:dateTime ;
	dct:modified "2017-07-04T12:00:00+00:00"^^xsd:dateTime  ;
	ikos:isObjectOf aspfacet:cyclingtype .

aspfacetvalue:lake
	rdf:type skos:Concept ;
	skos:prefLabel	"lake"@en-GB ;
	skos:definition	"Windsurfing races on a lake."@en-GB ;
	skos:inScheme <http://cv.iptc.org/newscodes/asportfacetvalue/>  ;
	ikos:created "2017-07-04T12:00:00+00:00"^^xsd:dateTime ;
	dct:created "2017-07-04T12:00:00+00:00"^^xsd:dateTime ;
	ikos:modified "2017-07-04T12:00:00+00:00"^^xsd:dateTime ;
	dct:modified "2017-07-04T12:00:00+00:00"^^xsd:dateTime  ;
	ikos:isObjectOf aspfacet:windsurfingtype .

aspfacetvalue:land
	rdf:type skos:Concept ;
	skos:prefLabel	"land "@en-GB ;
	skos:definition	"Windsurfing races competed on land with a board equipped with wheels."@en-GB ;
	skos:inScheme <http://cv.iptc.org/newscodes/asportfacetvalue/>  ;
	ikos:created "2017-07-04T12:00:00+00:00"^^xsd:dateTime ;
	dct:created "2017-07-04T12:00:00+00:00"^^xsd:dateTime ;
	ikos:modified "2017-07-04T12:00:00+00:00"^^xsd:dateTime ;
	dct:modified "2017-07-04T12:00:00+00:00"^^xsd:dateTime  ;
	ikos:isObjectOf aspfacet:windsurfingtype .

aspfacetvalue:laser
	rdf:type skos:Concept ;
	skos:prefLabel	"laser"@en-GB ;
	skos:definition	"Boat Category: one man dinghy (4.6m/sq mainsail) Olympic sport "@en-GB ;
	skos:inScheme <http://cv.iptc.org/newscodes/asportfacetvalue/>  ;
	ikos:created "2017-07-04T12:00:00+00:00"^^xsd:dateTime ;
	dct:created "2017-07-04T12:00:00+00:00"^^xsd:dateTime ;
	ikos:modified "2017-07-04T12:00:00+00:00"^^xsd:dateTime ;
	dct:modified "2017-07-04T12:00:00+00:00"^^xsd:dateTime  ;
	ikos:isObjectOf aspfacet:sailingtype .

aspfacetvalue:left-wall
	rdf:type skos:Concept ;
	skos:prefLabel	"left wall"@en-GB ;
	skos:definition	"A *fronton with left hand wall* is an indoor fronton with a 36 meters long court where Pala or Main Nue are played. Three walls are used in the game: the front, the back and the left hand wall. "@en-GB ;
	skos:inScheme <http://cv.iptc.org/newscodes/asportfacetvalue/>  ;
	ikos:created "2017-07-04T12:00:00+00:00"^^xsd:dateTime ;
	dct:created "2017-07-04T12:00:00+00:00"^^xsd:dateTime ;
	ikos:modified "2017-07-04T12:00:00+00:00"^^xsd:dateTime ;
	dct:modified "2017-07-04T12:00:00+00:00"^^xsd:dateTime  ;
	ikos:isObjectOf aspfacet:jaialaitype .

aspfacetvalue:lightweight
	rdf:type skos:Concept ;
	skos:prefLabel	"lightweight"@en-GB ;
	skos:definition	"Where a weight category is imposed on competitors"@en-GB ;
	skos:inScheme <http://cv.iptc.org/newscodes/asportfacetvalue/>  ;
	ikos:created "2017-07-04T12:00:00+00:00"^^xsd:dateTime ;
	dct:created "2017-07-04T12:00:00+00:00"^^xsd:dateTime ;
	ikos:modified "2017-07-04T12:00:00+00:00"^^xsd:dateTime ;
	dct:modified "2017-07-04T12:00:00+00:00"^^xsd:dateTime  ;
	ikos:isObjectOf aspfacet:rowingtype .

aspfacetvalue:madison-race
	rdf:type skos:Concept ;
	skos:prefLabel	"madison race"@en-GB ;
	skos:definition	"A points race by teams comprising two cyclists in relay-format."@en-GB ;
	skos:inScheme <http://cv.iptc.org/newscodes/asportfacetvalue/>  ;
	ikos:created "2017-07-04T12:00:00+00:00"^^xsd:dateTime ;
	dct:created "2017-07-04T12:00:00+00:00"^^xsd:dateTime ;
	ikos:modified "2017-07-04T12:00:00+00:00"^^xsd:dateTime ;
	dct:modified "2017-07-04T12:00:00+00:00"^^xsd:dateTime  ;
	ikos:isObjectOf aspfacet:cyclingtype .

aspfacetvalue:marathon
	rdf:type skos:Concept ;
	skos:prefLabel	"marathon"@en-GB ;
	skos:definition	"Long distance open water swimming. "@en-GB ;
	skos:inScheme <http://cv.iptc.org/newscodes/asportfacetvalue/>  ;
	ikos:created "2017-07-04T12:00:00+00:00"^^xsd:dateTime ;
	dct:created "2017-07-04T12:00:00+00:00"^^xsd:dateTime ;
	ikos:modified "2017-07-04T12:00:00+00:00"^^xsd:dateTime ;
	dct:modified "2017-07-04T12:00:00+00:00"^^xsd:dateTime  ;
	ikos:isObjectOf aspfacet:swimmingtype .

aspfacetvalue:massstart
	rdf:type skos:Concept ;
	skos:prefLabel	"mass start"@en-GB ;
	skos:definition	"Event where all competitors start at once."@en-GB ;
	skos:inScheme <http://cv.iptc.org/newscodes/asportfacetvalue/>  ;
	ikos:created "2017-07-04T12:00:00+00:00"^^xsd:dateTime ;
	dct:created "2017-07-04T12:00:00+00:00"^^xsd:dateTime ;
	ikos:modified "2017-07-04T12:00:00+00:00"^^xsd:dateTime ;
	dct:modified "2017-07-04T12:00:00+00:00"^^xsd:dateTime  ;
	ikos:isObjectOf aspfacet:racetype .

aspfacetvalue:medley
	rdf:type skos:Concept ;
	skos:prefLabel	"medley"@en-GB ;
	skos:definition	"A combination of four different swimming styles in one race."@en-GB ;
	skos:inScheme <http://cv.iptc.org/newscodes/asportfacetvalue/>  ;
	ikos:created "2017-07-04T12:00:00+00:00"^^xsd:dateTime ;
	dct:created "2017-07-04T12:00:00+00:00"^^xsd:dateTime ;
	ikos:modified "2017-07-04T12:00:00+00:00"^^xsd:dateTime ;
	dct:modified "2017-07-04T12:00:00+00:00"^^xsd:dateTime  ;
	ikos:isObjectOf aspfacet:swimmingtype .

aspfacetvalue:men
	rdf:type skos:Concept ;
	skos:prefLabel	"men "@en-GB ;
	skos:definition	"Single male human person"@en-GB ;
	skos:inScheme <http://cv.iptc.org/newscodes/asportfacetvalue/>  ;
	ikos:created "2017-07-04T12:00:00+00:00"^^xsd:dateTime ;
	dct:created "2017-07-04T12:00:00+00:00"^^xsd:dateTime ;
	ikos:modified "2017-07-04T12:00:00+00:00"^^xsd:dateTime ;
	dct:modified "2017-07-04T12:00:00+00:00"^^xsd:dateTime  ;
	ikos:isObjectOf aspfacet:gender .

aspfacetvalue:mistral
	rdf:type skos:Concept ;
	skos:prefLabel	"mistral"@en-GB ;
	skos:definition	"Olympic boat class. A staged race using boats of the mistral type, which are 4.24 metres (13ft 11in) long and 1.3 metres (4ft 3in) wide. The number of races and the length of the courses varies. "@en-GB ;
	skos:inScheme <http://cv.iptc.org/newscodes/asportfacetvalue/>  ;
	ikos:created "2017-07-04T12:00:00+00:00"^^xsd:dateTime ;
	dct:created "2017-07-04T12:00:00+00:00"^^xsd:dateTime ;
	ikos:modified "2017-07-04T12:00:00+00:00"^^xsd:dateTime ;
	dct:modified "2017-07-04T12:00:00+00:00"^^xsd:dateTime  ;
	ikos:isObjectOf aspfacet:sailingtype .

aspfacetvalue:mixed
	rdf:type skos:Concept ;
	skos:prefLabel	"mixed "@en-GB ;
	skos:definition	"Mixed team of male and female human persons "@en-GB ;
	skos:inScheme <http://cv.iptc.org/newscodes/asportfacetvalue/>  ;
	ikos:created "2017-07-04T12:00:00+00:00"^^xsd:dateTime ;
	dct:created "2017-07-04T12:00:00+00:00"^^xsd:dateTime ;
	ikos:modified "2017-07-04T12:00:00+00:00"^^xsd:dateTime ;
	dct:modified "2017-07-04T12:00:00+00:00"^^xsd:dateTime  ;
	ikos:isObjectOf aspfacet:gender .

aspfacetvalue:moguls
	rdf:type skos:Concept ;
	skos:prefLabel	"moguls"@en-GB ;
	skos:definition	"Contestants attack a heavily moguled slope, performing technically challenging turns and jumps, while maintaining the most direct line from the top to the bottom of the hill."@en-GB ;
	skos:inScheme <http://cv.iptc.org/newscodes/asportfacetvalue/>  ;
	ikos:created "2017-07-04T12:00:00+00:00"^^xsd:dateTime ;
	dct:created "2017-07-04T12:00:00+00:00"^^xsd:dateTime ;
	ikos:modified "2017-07-04T12:00:00+00:00"^^xsd:dateTime ;
	dct:modified "2017-07-04T12:00:00+00:00"^^xsd:dateTime  ;
	ikos:isObjectOf aspfacet:freestyleskiingtype .

aspfacetvalue:monohull
	rdf:type skos:Concept ;
	skos:prefLabel	"monohull"@en-GB ;
	skos:definition	"Single hull craft"@en-GB ;
	skos:inScheme <http://cv.iptc.org/newscodes/asportfacetvalue/>  ;
	ikos:created "2017-07-04T12:00:00+00:00"^^xsd:dateTime ;
	dct:created "2017-07-04T12:00:00+00:00"^^xsd:dateTime ;
	ikos:modified "2017-07-04T12:00:00+00:00"^^xsd:dateTime ;
	dct:modified "2017-07-04T12:00:00+00:00"^^xsd:dateTime  ;
	ikos:isObjectOf aspfacet:sailingtype .

aspfacetvalue:moto-ball
	rdf:type skos:Concept ;
	skos:prefLabel	"moto-ball"@en-GB ;
	skos:definition	"Team sport where drivers play a ball."@en-GB ;
	skos:inScheme <http://cv.iptc.org/newscodes/asportfacetvalue/>  ;
	ikos:created "2017-07-04T12:00:00+00:00"^^xsd:dateTime ;
	dct:created "2017-07-04T12:00:00+00:00"^^xsd:dateTime ;
	ikos:modified "2017-07-04T12:00:00+00:00"^^xsd:dateTime ;
	dct:modified "2017-07-04T12:00:00+00:00"^^xsd:dateTime  ;
	ikos:isObjectOf aspfacet:motorcyclingtype .

aspfacetvalue:moto-cross
	rdf:type skos:Concept ;
	skos:prefLabel	"moto-cross"@en-GB ;
	skos:definition	"Race over dirt tracks featuring severe mounds."@en-GB ;
	skos:inScheme <http://cv.iptc.org/newscodes/asportfacetvalue/>  ;
	ikos:created "2017-07-04T12:00:00+00:00"^^xsd:dateTime ;
	dct:created "2017-07-04T12:00:00+00:00"^^xsd:dateTime ;
	ikos:modified "2017-07-04T12:00:00+00:00"^^xsd:dateTime ;
	dct:modified "2017-07-04T12:00:00+00:00"^^xsd:dateTime  ;
	ikos:isObjectOf aspfacet:motorcyclingtype .

aspfacetvalue:motoGP
	rdf:type skos:Concept ;
	skos:prefLabel	"motoGP"@en-GB ;
	skos:definition	"Races on Grand Prix motorcycles."@en-GB ;
	skos:inScheme <http://cv.iptc.org/newscodes/asportfacetvalue/>  ;
	ikos:created "2017-07-04T12:00:00+00:00"^^xsd:dateTime ;
	dct:created "2017-07-04T12:00:00+00:00"^^xsd:dateTime ;
	ikos:modified "2017-07-04T12:00:00+00:00"^^xsd:dateTime ;
	dct:modified "2017-07-04T12:00:00+00:00"^^xsd:dateTime  ;
	ikos:isObjectOf aspfacet:motorcyclingtype .

aspfacetvalue:MTA
	rdf:type skos:Concept ;
	skos:prefLabel	"MTA"@en-GB ;
	skos:definition	"In the MTA (Maximum Time Aloft) sub event the player throws a disc and then tries to catch the disc with one hand as late as possible before it hits the ground."@en-GB ;
	skos:inScheme <http://cv.iptc.org/newscodes/asportfacetvalue/>  ;
	ikos:created "2017-07-04T12:00:00+00:00"^^xsd:dateTime ;
	dct:created "2017-07-04T12:00:00+00:00"^^xsd:dateTime ;
	ikos:modified "2017-07-04T12:00:00+00:00"^^xsd:dateTime ;
	dct:modified "2017-07-04T12:00:00+00:00"^^xsd:dateTime  ;
	ikos:isObjectOf aspfacet:flyingdisctype .

aspfacetvalue:multihulls
	rdf:type skos:Concept ;
	skos:prefLabel	"multihulls"@en-GB ;
	skos:definition	"Multi hull craft"@en-GB ;
	skos:inScheme <http://cv.iptc.org/newscodes/asportfacetvalue/>  ;
	ikos:created "2017-07-04T12:00:00+00:00"^^xsd:dateTime ;
	dct:created "2017-07-04T12:00:00+00:00"^^xsd:dateTime ;
	ikos:modified "2017-07-04T12:00:00+00:00"^^xsd:dateTime ;
	dct:modified "2017-07-04T12:00:00+00:00"^^xsd:dateTime  ;
	ikos:isObjectOf aspfacet:sailingtype .

aspfacetvalue:ocean
	rdf:type skos:Concept ;
	skos:prefLabel	"ocean"@en-GB ;
	skos:definition	"Windsurfing races on the open seas."@en-GB ;
	skos:inScheme <http://cv.iptc.org/newscodes/asportfacetvalue/>  ;
	ikos:created "2017-07-04T12:00:00+00:00"^^xsd:dateTime ;
	dct:created "2017-07-04T12:00:00+00:00"^^xsd:dateTime ;
	ikos:modified "2017-07-04T12:00:00+00:00"^^xsd:dateTime ;
	dct:modified "2017-07-04T12:00:00+00:00"^^xsd:dateTime  ;
	ikos:isObjectOf aspfacet:windsurfingtype .

aspfacetvalue:ovaltrack
	rdf:type skos:Concept ;
	skos:prefLabel	"oval track"@en-GB ;
	skos:definition	"Dog race where dogs pursue an artificial rabbit around an oval track ."@en-GB ;
	skos:inScheme <http://cv.iptc.org/newscodes/asportfacetvalue/>  ;
	ikos:created "2017-07-04T12:00:00+00:00"^^xsd:dateTime ;
	dct:created "2017-07-04T12:00:00+00:00"^^xsd:dateTime ;
	ikos:modified "2017-07-04T12:00:00+00:00"^^xsd:dateTime ;
	dct:modified "2017-07-04T12:00:00+00:00"^^xsd:dateTime  ;
	ikos:isObjectOf aspfacet:dogracingtype .

aspfacetvalue:overall
	rdf:type skos:Concept ;
	skos:prefLabel	"overall"@en-GB ;
	skos:definition	"Not an event in itself but in most competitions with individual events the winner of the competition will be awarded to the player with the highest combined score in the events. "@en-GB ;
	skos:inScheme <http://cv.iptc.org/newscodes/asportfacetvalue/>  ;
	ikos:created "2017-07-04T12:00:00+00:00"^^xsd:dateTime ;
	dct:created "2017-07-04T12:00:00+00:00"^^xsd:dateTime ;
	ikos:modified "2017-07-04T12:00:00+00:00"^^xsd:dateTime ;
	dct:modified "2017-07-04T12:00:00+00:00"^^xsd:dateTime  ;
	ikos:isObjectOf aspfacet:flyingdisctype .

aspfacetvalue:pairs
	rdf:type skos:Concept ;
	skos:prefLabel	"pairs"@en-GB ;
	skos:definition	"Skating event where the pairs event comprises a short program which counts for 33.3% of the score, and the free skate which is worth 66.7%."@en-GB ;
	skos:inScheme <http://cv.iptc.org/newscodes/asportfacetvalue/>  ;
	ikos:created "2017-07-04T12:00:00+00:00"^^xsd:dateTime ;
	dct:created "2017-07-04T12:00:00+00:00"^^xsd:dateTime ;
	ikos:modified "2017-07-04T12:00:00+00:00"^^xsd:dateTime ;
	dct:modified "2017-07-04T12:00:00+00:00"^^xsd:dateTime  ;
	ikos:isObjectOf aspfacet:figureskatingtype .

aspfacetvalue:pala-ancha
	rdf:type skos:Concept ;
	skos:prefLabel	"pala-ancha"@en-GB ;
	skos:definition	"The *pala-ancha* is the game played in a fronton *place libre* with 2 players in each team. The players use a heavy wooden bat *the pala* (50 cm long and 20 cm wide). "@en-GB ;
	skos:inScheme <http://cv.iptc.org/newscodes/asportfacetvalue/>  ;
	ikos:created "2017-07-04T12:00:00+00:00"^^xsd:dateTime ;
	dct:created "2017-07-04T12:00:00+00:00"^^xsd:dateTime ;
	ikos:modified "2017-07-04T12:00:00+00:00"^^xsd:dateTime ;
	dct:modified "2017-07-04T12:00:00+00:00"^^xsd:dateTime  ;
	ikos:isObjectOf aspfacet:jaialaitype .

aspfacetvalue:pala-corta
	rdf:type skos:Concept ;
	skos:prefLabel	"pala-corta"@en-GB ;
	skos:definition	"The *pala-corta* is the game played in a fronton with left hand wall and 2 players in each team. The players use a heavy wooden bat the *pala-corta* (50 cm long and 10 cm wide)."@en-GB ;
	skos:inScheme <http://cv.iptc.org/newscodes/asportfacetvalue/>  ;
	ikos:created "2017-07-04T12:00:00+00:00"^^xsd:dateTime ;
	dct:created "2017-07-04T12:00:00+00:00"^^xsd:dateTime ;
	ikos:modified "2017-07-04T12:00:00+00:00"^^xsd:dateTime ;
	dct:modified "2017-07-04T12:00:00+00:00"^^xsd:dateTime  ;
	ikos:isObjectOf aspfacet:jaialaitype .

aspfacetvalue:parallelbars
	rdf:type skos:Concept ;
	skos:prefLabel	"parallel bars"@en-GB ;
	skos:definition	"Artistic gymnastics event where gymnasts swing and turn around the parallel bars."@en-GB ;
	skos:inScheme <http://cv.iptc.org/newscodes/asportfacetvalue/>  ;
	ikos:created "2017-07-04T12:00:00+00:00"^^xsd:dateTime ;
	dct:created "2017-07-04T12:00:00+00:00"^^xsd:dateTime ;
	ikos:modified "2017-07-04T12:00:00+00:00"^^xsd:dateTime ;
	dct:modified "2017-07-04T12:00:00+00:00"^^xsd:dateTime  ;
	ikos:isObjectOf aspfacet:artisticgymtype .

aspfacetvalue:parallelslalom-alpineskiing
	rdf:type skos:Concept ;
	skos:prefLabel	"parallel slalom"@en-GB ;
	skos:definition	"Race between narrow set poles or gates run by two persons in parallel."@en-GB ;
	skos:inScheme <http://cv.iptc.org/newscodes/asportfacetvalue/>  ;
	ikos:created "2017-07-04T12:00:00+00:00"^^xsd:dateTime ;
	dct:created "2017-07-04T12:00:00+00:00"^^xsd:dateTime ;
	ikos:modified "2017-07-04T12:00:00+00:00"^^xsd:dateTime ;
	dct:modified "2017-07-04T12:00:00+00:00"^^xsd:dateTime  ;
	ikos:isObjectOf aspfacet:alpineskiingtype .

aspfacetvalue:parallelslalom-snowboarding
	rdf:type skos:Concept ;
	skos:prefLabel	"parallel slalom"@en-GB ;
	skos:definition	"Race between narrow set poles or gates run by two persons in parallel"@en-GB ;
	skos:inScheme <http://cv.iptc.org/newscodes/asportfacetvalue/>  ;
	ikos:created "2017-07-04T12:00:00+00:00"^^xsd:dateTime ;
	dct:created "2017-07-04T12:00:00+00:00"^^xsd:dateTime ;
	ikos:modified "2017-07-04T12:00:00+00:00"^^xsd:dateTime ;
	dct:modified "2017-07-04T12:00:00+00:00"^^xsd:dateTime  ;
	ikos:isObjectOf aspfacet:snowboardingtype .

aspfacetvalue:park
	rdf:type skos:Concept ;
	skos:prefLabel	"park"@en-GB ;
	skos:definition	"BMX with an emphasis on riding bowl transitions or ramp jumps."@en-GB ;
	skos:inScheme <http://cv.iptc.org/newscodes/asportfacetvalue/>  ;
	ikos:created "2017-07-04T12:00:00+00:00"^^xsd:dateTime ;
	dct:created "2017-07-04T12:00:00+00:00"^^xsd:dateTime ;
	ikos:modified "2017-07-04T12:00:00+00:00"^^xsd:dateTime ;
	dct:modified "2017-07-04T12:00:00+00:00"^^xsd:dateTime  ;
	ikos:isObjectOf aspfacet:bmxfreestyletype .

aspfacetvalue:pasaka
	rdf:type skos:Concept ;
	skos:prefLabel	"pasaka"@en-GB ;
	skos:definition	"The *pasaka* is the name of the game played in a trinquet by teams of 2 players facing each other on each side of a net where the pelota is hit between opponents. "@en-GB ;
	skos:inScheme <http://cv.iptc.org/newscodes/asportfacetvalue/>  ;
	ikos:created "2017-07-04T12:00:00+00:00"^^xsd:dateTime ;
	dct:created "2017-07-04T12:00:00+00:00"^^xsd:dateTime ;
	ikos:modified "2017-07-04T12:00:00+00:00"^^xsd:dateTime ;
	dct:modified "2017-07-04T12:00:00+00:00"^^xsd:dateTime  ;
	ikos:isObjectOf aspfacet:jaialaitype .

aspfacetvalue:pistol
	rdf:type skos:Concept ;
	skos:prefLabel	"pistol"@en-GB ;
	skos:definition	"Shooting event shot with a .22-caliber sport pistol, all firing must be done with one hand, unsupported."@en-GB ;
	skos:inScheme <http://cv.iptc.org/newscodes/asportfacetvalue/>  ;
	ikos:created "2017-07-04T12:00:00+00:00"^^xsd:dateTime ;
	dct:created "2017-07-04T12:00:00+00:00"^^xsd:dateTime ;
	ikos:modified "2017-07-04T12:00:00+00:00"^^xsd:dateTime ;
	dct:modified "2017-07-04T12:00:00+00:00"^^xsd:dateTime  ;
	ikos:isObjectOf aspfacet:shootingtype .

aspfacetvalue:points-race
	rdf:type skos:Concept ;
	skos:prefLabel	"points race"@en-GB ;
	skos:definition	"Cyclists aim to complete the highest number of laps. Bonus points are picked up in intermediate sprints held every 2500m."@en-GB ;
	skos:inScheme <http://cv.iptc.org/newscodes/asportfacetvalue/>  ;
	ikos:created "2017-07-04T12:00:00+00:00"^^xsd:dateTime ;
	dct:created "2017-07-04T12:00:00+00:00"^^xsd:dateTime ;
	ikos:modified "2017-07-04T12:00:00+00:00"^^xsd:dateTime ;
	dct:modified "2017-07-04T12:00:00+00:00"^^xsd:dateTime  ;
	ikos:isObjectOf aspfacet:cyclingtype .

aspfacetvalue:pommelhorse
	rdf:type skos:Concept ;
	skos:prefLabel	"pommel horse"@en-GB ;
	skos:definition	"Artistic gymnastics event where gymnasts perform an uninterrupted swing motion over a handled horse using balance and strength."@en-GB ;
	skos:inScheme <http://cv.iptc.org/newscodes/asportfacetvalue/>  ;
	ikos:created "2017-07-04T12:00:00+00:00"^^xsd:dateTime ;
	dct:created "2017-07-04T12:00:00+00:00"^^xsd:dateTime ;
	ikos:modified "2017-07-04T12:00:00+00:00"^^xsd:dateTime ;
	dct:modified "2017-07-04T12:00:00+00:00"^^xsd:dateTime  ;
	ikos:isObjectOf aspfacet:artisticgymtype .

aspfacetvalue:pontoniering
	rdf:type skos:Concept ;
	skos:prefLabel	"pontoniering"@en-GB ;
	skos:definition	"Team sport, military tradition, similar to canoe regatta, in boat. "@en-GB ;
	skos:inScheme <http://cv.iptc.org/newscodes/asportfacetvalue/>  ;
	ikos:created "2017-07-04T12:00:00+00:00"^^xsd:dateTime ;
	dct:created "2017-07-04T12:00:00+00:00"^^xsd:dateTime ;
	ikos:modified "2017-07-04T12:00:00+00:00"^^xsd:dateTime ;
	dct:modified "2017-07-04T12:00:00+00:00"^^xsd:dateTime  ;
	ikos:isObjectOf aspfacet:canoekayaktype .

aspfacetvalue:powerlifting
	rdf:type skos:Concept ;
	skos:prefLabel	"powerlifting"@en-GB ;
	skos:definition	"A strength test where competitors lift as heavy a weight as possible"@en-GB ;
	skos:inScheme <http://cv.iptc.org/newscodes/asportfacetvalue/>  ;
	ikos:created "2017-07-04T12:00:00+00:00"^^xsd:dateTime ;
	dct:created "2017-07-04T12:00:00+00:00"^^xsd:dateTime ;
	ikos:modified "2017-07-04T12:00:00+00:00"^^xsd:dateTime ;
	dct:modified "2017-07-04T12:00:00+00:00"^^xsd:dateTime  ;
	ikos:isObjectOf aspfacet:weightliftingtype .

aspfacetvalue:pursuit
	rdf:type skos:Concept ;
	skos:prefLabel	"pursuit"@en-GB ;
	skos:definition	"A race where the competitors start in relation to some previous result. Best competitor start first and then the rest in pursuit at some interval later."@en-GB ;
	skos:inScheme <http://cv.iptc.org/newscodes/asportfacetvalue/>  ;
	ikos:created "2017-07-04T12:00:00+00:00"^^xsd:dateTime ;
	dct:created "2017-07-04T12:00:00+00:00"^^xsd:dateTime ;
	ikos:modified "2017-07-04T12:00:00+00:00"^^xsd:dateTime ;
	dct:modified "2017-07-04T12:00:00+00:00"^^xsd:dateTime  ;
	ikos:isObjectOf aspfacet:racetype .

aspfacetvalue:rallycross
	rdf:type skos:Concept ;
	skos:prefLabel	"rallycross"@en-GB ;
	skos:definition	"Motor car races over dirt tracks "@en-GB ;
	skos:inScheme <http://cv.iptc.org/newscodes/asportfacetvalue/>  ;
	ikos:created "2017-07-04T12:00:00+00:00"^^xsd:dateTime ;
	dct:created "2017-07-04T12:00:00+00:00"^^xsd:dateTime ;
	ikos:modified "2017-07-04T12:00:00+00:00"^^xsd:dateTime ;
	dct:modified "2017-07-04T12:00:00+00:00"^^xsd:dateTime  ;
	ikos:isObjectOf aspfacet:motorcarracingtype .

aspfacetvalue:rallying
	rdf:type skos:Concept ;
	skos:prefLabel	"rallying"@en-GB ;
	skos:definition	"Motor car stage races."@en-GB ;
	skos:inScheme <http://cv.iptc.org/newscodes/asportfacetvalue/>  ;
	ikos:created "2017-07-04T12:00:00+00:00"^^xsd:dateTime ;
	dct:created "2017-07-04T12:00:00+00:00"^^xsd:dateTime ;
	ikos:modified "2017-07-04T12:00:00+00:00"^^xsd:dateTime ;
	dct:modified "2017-07-04T12:00:00+00:00"^^xsd:dateTime  ;
	ikos:isObjectOf aspfacet:motorcarracingtype .

aspfacetvalue:rapid-fire-pistol
	rdf:type skos:Concept ;
	skos:prefLabel	"rapid fire pistol"@en-GB ;
	skos:definition	"Shooting event shot with a rapid fire pistol."@en-GB ;
	skos:inScheme <http://cv.iptc.org/newscodes/asportfacetvalue/>  ;
	ikos:created "2017-07-04T12:00:00+00:00"^^xsd:dateTime ;
	dct:created "2017-07-04T12:00:00+00:00"^^xsd:dateTime ;
	ikos:modified "2017-07-04T12:00:00+00:00"^^xsd:dateTime ;
	dct:modified "2017-07-04T12:00:00+00:00"^^xsd:dateTime  ;
	ikos:isObjectOf aspfacet:shootingtype .

aspfacetvalue:rebot
	rdf:type skos:Concept ;
	skos:prefLabel	"rebot"@en-GB ;
	skos:definition	"The *rebot* is the game played in a fronton *place libre* with 5 players in each team. They use a *chistera* (56 cm long and 12 cm large) or bare hands. "@en-GB ;
	skos:inScheme <http://cv.iptc.org/newscodes/asportfacetvalue/>  ;
	ikos:created "2017-07-04T12:00:00+00:00"^^xsd:dateTime ;
	dct:created "2017-07-04T12:00:00+00:00"^^xsd:dateTime ;
	ikos:modified "2017-07-04T12:00:00+00:00"^^xsd:dateTime ;
	dct:modified "2017-07-04T12:00:00+00:00"^^xsd:dateTime  ;
	ikos:isObjectOf aspfacet:jaialaitype .

aspfacetvalue:reining
	rdf:type skos:Concept ;
	skos:prefLabel	"reining"@en-GB ;
	skos:definition	"Competition  where the riders guide the horses through a precise pattern of circles, spins, and stops."@en-GB ;
	skos:inScheme <http://cv.iptc.org/newscodes/asportfacetvalue/>  ;
	ikos:created "2017-07-04T12:00:00+00:00"^^xsd:dateTime ;
	dct:created "2017-07-04T12:00:00+00:00"^^xsd:dateTime ;
	ikos:modified "2017-07-04T12:00:00+00:00"^^xsd:dateTime ;
	dct:modified "2017-07-04T12:00:00+00:00"^^xsd:dateTime  ;
	ikos:isObjectOf aspfacet:equestriantype .

aspfacetvalue:relay
	rdf:type skos:Concept ;
	skos:prefLabel	"relay"@en-GB ;
	skos:definition	"A race where the members of a team compete in parts of the race and the total time is counted."@en-GB ;
	skos:inScheme <http://cv.iptc.org/newscodes/asportfacetvalue/>  ;
	ikos:created "2017-07-04T12:00:00+00:00"^^xsd:dateTime ;
	dct:created "2017-07-04T12:00:00+00:00"^^xsd:dateTime ;
	ikos:modified "2017-07-04T12:00:00+00:00"^^xsd:dateTime ;
	dct:modified "2017-07-04T12:00:00+00:00"^^xsd:dateTime  ;
	ikos:isObjectOf aspfacet:racetype .

aspfacetvalue:ribbon
	rdf:type skos:Concept ;
	skos:prefLabel	"ribbon"@en-GB ;
	skos:definition	"Rhythmic gymnastics event where a ribbon is used for moves that include flicks, circles, snakes and spirals, and throws"@en-GB ;
	skos:inScheme <http://cv.iptc.org/newscodes/asportfacetvalue/>  ;
	ikos:created "2017-07-04T12:00:00+00:00"^^xsd:dateTime ;
	dct:created "2017-07-04T12:00:00+00:00"^^xsd:dateTime ;
	ikos:modified "2017-07-04T12:00:00+00:00"^^xsd:dateTime ;
	dct:modified "2017-07-04T12:00:00+00:00"^^xsd:dateTime  ;
	ikos:isObjectOf aspfacet:rhythmgymtype .

aspfacetvalue:rifle-3-positions
	rdf:type skos:Concept ;
	skos:prefLabel	"rifle 3 positions"@en-GB ;
	skos:definition	"Shooting event consisting of the kneeling, prone, and standing positions, fired in that order, with 3√ó40 shots for men and 3√ó20 shots for women. The caliber is .22 Long Rifle (5.6 mm)."@en-GB ;
	skos:inScheme <http://cv.iptc.org/newscodes/asportfacetvalue/>  ;
	ikos:created "2017-07-04T12:00:00+00:00"^^xsd:dateTime ;
	dct:created "2017-07-04T12:00:00+00:00"^^xsd:dateTime ;
	ikos:modified "2017-07-04T12:00:00+00:00"^^xsd:dateTime ;
	dct:modified "2017-07-04T12:00:00+00:00"^^xsd:dateTime  ;
	ikos:isObjectOf aspfacet:shootingtype .

aspfacetvalue:rifle-prone
	rdf:type skos:Concept ;
	skos:prefLabel	"rifle prone"@en-GB ;
	skos:definition	"Shooting event consisting of 60 shots from the prone position with a .22 Long Rifle (5.6 mm) caliber rifle."@en-GB ;
	skos:inScheme <http://cv.iptc.org/newscodes/asportfacetvalue/>  ;
	ikos:created "2017-07-04T12:00:00+00:00"^^xsd:dateTime ;
	dct:created "2017-07-04T12:00:00+00:00"^^xsd:dateTime ;
	ikos:modified "2017-07-04T12:00:00+00:00"^^xsd:dateTime ;
	dct:modified "2017-07-04T12:00:00+00:00"^^xsd:dateTime  ;
	ikos:isObjectOf aspfacet:shootingtype .

aspfacetvalue:rings
	rdf:type skos:Concept ;
	skos:prefLabel	"rings"@en-GB ;
	skos:definition	"Artistic gymnastics event where gymnasts perform feats of balance and strength from two suspended rings."@en-GB ;
	skos:inScheme <http://cv.iptc.org/newscodes/asportfacetvalue/>  ;
	ikos:created "2017-07-04T12:00:00+00:00"^^xsd:dateTime ;
	dct:created "2017-07-04T12:00:00+00:00"^^xsd:dateTime ;
	ikos:modified "2017-07-04T12:00:00+00:00"^^xsd:dateTime ;
	dct:modified "2017-07-04T12:00:00+00:00"^^xsd:dateTime  ;
	ikos:isObjectOf aspfacet:artisticgymtype .

aspfacetvalue:river
	rdf:type skos:Concept ;
	skos:prefLabel	"river"@en-GB ;
	skos:definition	"Windsurfing races on a river."@en-GB ;
	skos:inScheme <http://cv.iptc.org/newscodes/asportfacetvalue/>  ;
	ikos:created "2017-07-04T12:00:00+00:00"^^xsd:dateTime ;
	dct:created "2017-07-04T12:00:00+00:00"^^xsd:dateTime ;
	ikos:modified "2017-07-04T12:00:00+00:00"^^xsd:dateTime ;
	dct:modified "2017-07-04T12:00:00+00:00"^^xsd:dateTime  ;
	ikos:isObjectOf aspfacet:windsurfingtype .

aspfacetvalue:road-race
	rdf:type skos:Concept ;
	skos:prefLabel	"road race"@en-GB ;
	skos:definition	"Road race with all the competitor starting en masse."@en-GB ;
	skos:inScheme <http://cv.iptc.org/newscodes/asportfacetvalue/>  ;
	ikos:created "2017-07-04T12:00:00+00:00"^^xsd:dateTime ;
	dct:created "2017-07-04T12:00:00+00:00"^^xsd:dateTime ;
	ikos:modified "2017-07-04T12:00:00+00:00"^^xsd:dateTime ;
	dct:modified "2017-07-04T12:00:00+00:00"^^xsd:dateTime  ;
	ikos:isObjectOf aspfacet:cyclingtype .

aspfacetvalue:rope
	rdf:type skos:Concept ;
	skos:prefLabel	"rope"@en-GB ;
	skos:definition	"Rhythmic gymnastics event where a rope is used for moves that include leaps and skipping"@en-GB ;
	skos:inScheme <http://cv.iptc.org/newscodes/asportfacetvalue/>  ;
	ikos:created "2017-07-04T12:00:00+00:00"^^xsd:dateTime ;
	dct:created "2017-07-04T12:00:00+00:00"^^xsd:dateTime ;
	ikos:modified "2017-07-04T12:00:00+00:00"^^xsd:dateTime ;
	dct:modified "2017-07-04T12:00:00+00:00"^^xsd:dateTime  ;
	ikos:isObjectOf aspfacet:rhythmgymtype .

aspfacetvalue:running-target
	rdf:type skos:Concept ;
	skos:prefLabel	"running target"@en-GB ;
	skos:definition	"Shooting event where the target is pulled across a two meter wide aisle at the range of 10 metres from the firing point. The target is pulled at either of two speeds, slow or fast."@en-GB ;
	skos:inScheme <http://cv.iptc.org/newscodes/asportfacetvalue/>  ;
	ikos:created "2017-07-04T12:00:00+00:00"^^xsd:dateTime ;
	dct:created "2017-07-04T12:00:00+00:00"^^xsd:dateTime ;
	ikos:modified "2017-07-04T12:00:00+00:00"^^xsd:dateTime ;
	dct:modified "2017-07-04T12:00:00+00:00"^^xsd:dateTime  ;
	ikos:isObjectOf aspfacet:shootingtype .

aspfacetvalue:sabre
	rdf:type skos:Concept ;
	skos:prefLabel	"sabre"@en-GB ;
	skos:definition	"A fencing weapon with a flat blade and knuckle guard used with cutting or thrusting moves."@en-GB ;
	skos:inScheme <http://cv.iptc.org/newscodes/asportfacetvalue/>  ;
	ikos:created "2017-07-04T12:00:00+00:00"^^xsd:dateTime ;
	dct:created "2017-07-04T12:00:00+00:00"^^xsd:dateTime ;
	ikos:modified "2017-07-04T12:00:00+00:00"^^xsd:dateTime ;
	dct:modified "2017-07-04T12:00:00+00:00"^^xsd:dateTime  ;
	ikos:isObjectOf aspfacet:fencingtype .

aspfacetvalue:SCF
	rdf:type skos:Concept ;
	skos:prefLabel	"SCF"@en-GB ;
	skos:definition	"SCF (Self Caught Flights) combines by values the MTA (Maximum Time Aloft) and TRC (Throw Run Catch)."@en-GB ;
	skos:inScheme <http://cv.iptc.org/newscodes/asportfacetvalue/>  ;
	ikos:created "2017-07-04T12:00:00+00:00"^^xsd:dateTime ;
	dct:created "2017-07-04T12:00:00+00:00"^^xsd:dateTime ;
	ikos:modified "2017-07-04T12:00:00+00:00"^^xsd:dateTime ;
	dct:modified "2017-07-04T12:00:00+00:00"^^xsd:dateTime  ;
	ikos:isObjectOf aspfacet:flyingdisctype .

aspfacetvalue:sculls
	rdf:type skos:Concept ;
	skos:prefLabel	"sculls"@en-GB ;
	skos:definition	"Two oars each and without a team mate to give directions"@en-GB ;
	skos:inScheme <http://cv.iptc.org/newscodes/asportfacetvalue/>  ;
	ikos:created "2017-07-04T12:00:00+00:00"^^xsd:dateTime ;
	dct:created "2017-07-04T12:00:00+00:00"^^xsd:dateTime ;
	ikos:modified "2017-07-04T12:00:00+00:00"^^xsd:dateTime ;
	dct:modified "2017-07-04T12:00:00+00:00"^^xsd:dateTime  ;
	ikos:isObjectOf aspfacet:rowingtype .

aspfacetvalue:shortcourse
	rdf:type skos:Concept ;
	skos:prefLabel	"short course"@en-GB ;
	skos:definition	"Races competed in a 25m length pool. "@en-GB ;
	skos:inScheme <http://cv.iptc.org/newscodes/asportfacetvalue/>  ;
	ikos:created "2017-07-04T12:00:00+00:00"^^xsd:dateTime ;
	dct:created "2017-07-04T12:00:00+00:00"^^xsd:dateTime ;
	ikos:modified "2017-07-04T12:00:00+00:00"^^xsd:dateTime ;
	dct:modified "2017-07-04T12:00:00+00:00"^^xsd:dateTime  ;
	ikos:isObjectOf aspfacet:swimmingtype .

aspfacetvalue:side-cars
	rdf:type skos:Concept ;
	skos:prefLabel	"side-cars"@en-GB ;
	skos:definition	"Race using motorycles of different engine sizes with an attached side car featuring a passenger."@en-GB ;
	skos:inScheme <http://cv.iptc.org/newscodes/asportfacetvalue/>  ;
	ikos:created "2017-07-04T12:00:00+00:00"^^xsd:dateTime ;
	dct:created "2017-07-04T12:00:00+00:00"^^xsd:dateTime ;
	ikos:modified "2017-07-04T12:00:00+00:00"^^xsd:dateTime ;
	dct:modified "2017-07-04T12:00:00+00:00"^^xsd:dateTime  ;
	ikos:isObjectOf aspfacet:motorcyclingtype .

aspfacetvalue:singles
	rdf:type skos:Concept ;
	skos:prefLabel	"singles"@en-GB ;
	skos:definition	"Skating event where the individual events comprise a short program which counts for 33.3% of the score, and the free skate which is worth 66.7%."@en-GB ;
	skos:inScheme <http://cv.iptc.org/newscodes/asportfacetvalue/>  ;
	ikos:created "2017-07-04T12:00:00+00:00"^^xsd:dateTime ;
	dct:created "2017-07-04T12:00:00+00:00"^^xsd:dateTime ;
	ikos:modified "2017-07-04T12:00:00+00:00"^^xsd:dateTime ;
	dct:modified "2017-07-04T12:00:00+00:00"^^xsd:dateTime  ;
	ikos:isObjectOf aspfacet:figureskatingtype .

aspfacetvalue:skating-freestyle
	rdf:type skos:Concept ;
	skos:prefLabel	"skating/freestyle"@en-GB ;
	skos:definition	"Skirace were the skier is allowed to skate. There are no prepared tracks in the snow for the skis. Poles are normally longer, boots sturdier and skis shorter compared to classic skiing. "@en-GB ;
	skos:note	"Moved from *nordicskiingtype* to *crosscountryskiingtype* in August 2019"@en-GB ;
	skos:inScheme <http://cv.iptc.org/newscodes/asportfacetvalue/>  ;
	ikos:created "2017-07-04T12:00:00+00:00"^^xsd:dateTime ;
	dct:created "2017-07-04T12:00:00+00:00"^^xsd:dateTime ;
	ikos:modified "2017-07-04T12:00:00+00:00"^^xsd:dateTime ;
	dct:modified "2017-07-04T12:00:00+00:00"^^xsd:dateTime  ;
	ikos:isObjectOf aspfacet:crosscountryskiingtype .

aspfacetvalue:skeet
	rdf:type skos:Concept ;
	skos:prefLabel	"skeet"@en-GB ;
	skos:definition	"Shooting event with moving targets, competitor shoots from a series of positions "@en-GB ;
	skos:inScheme <http://cv.iptc.org/newscodes/asportfacetvalue/>  ;
	ikos:created "2017-07-04T12:00:00+00:00"^^xsd:dateTime ;
	dct:created "2017-07-04T12:00:00+00:00"^^xsd:dateTime ;
	ikos:modified "2017-07-04T12:00:00+00:00"^^xsd:dateTime ;
	dct:modified "2017-07-04T12:00:00+00:00"^^xsd:dateTime  ;
	ikos:isObjectOf aspfacet:shootingtype .

aspfacetvalue:skiathlon
	rdf:type skos:Concept ;
	skos:prefLabel	"skiathlon"@en-GB ;
	skos:definition	"Cross-country skiing race in two stages. The first stage is done in the classic technique. After the first stage, the racers change skis at a transition area, then continue racing on skating skis using the free technique."@en-GB ;
	skos:note	"Moved from *nordicskiingtype* to *crosscountryskiingtype* in August 2019"@en-GB ;
	skos:inScheme <http://cv.iptc.org/newscodes/asportfacetvalue/>  ;
	ikos:created "2017-07-04T12:00:00+00:00"^^xsd:dateTime ;
	dct:created "2017-07-04T12:00:00+00:00"^^xsd:dateTime ;
	ikos:modified "2017-07-04T12:00:00+00:00"^^xsd:dateTime ;
	dct:modified "2017-07-04T12:00:00+00:00"^^xsd:dateTime  ;
	ikos:isObjectOf aspfacet:crosscountryskiingtype .

aspfacetvalue:ski-cross
	rdf:type skos:Concept ;
	skos:prefLabel	"ski-cross"@en-GB ;
	skos:definition	"a multi-participant downhill ski race on irregular terrain"@en-GB ;
	skos:inScheme <http://cv.iptc.org/newscodes/asportfacetvalue/>  ;
	ikos:created "2019-11-22T12:00:00+00:00"^^xsd:dateTime ;
	dct:created "2019-11-22T12:00:00+00:00"^^xsd:dateTime ;
	ikos:modified "2019-11-22T12:00:00+00:00"^^xsd:dateTime ;
	dct:modified "2019-11-22T12:00:00+00:00"^^xsd:dateTime  ;
	ikos:isObjectOf aspfacet:freestyleskiingtype .

aspfacetvalue:slalom-alpineskiing
	rdf:type skos:Concept ;
	skos:prefLabel	"slalom"@en-GB ;
	skos:definition	"Timed race between narrow set poles or gates. Total time in two heats."@en-GB ;
	skos:inScheme <http://cv.iptc.org/newscodes/asportfacetvalue/>  ;
	ikos:created "2017-07-04T12:00:00+00:00"^^xsd:dateTime ;
	dct:created "2017-07-04T12:00:00+00:00"^^xsd:dateTime ;
	ikos:modified "2017-07-04T12:00:00+00:00"^^xsd:dateTime ;
	dct:modified "2017-07-04T12:00:00+00:00"^^xsd:dateTime  ;
	ikos:isObjectOf aspfacet:alpineskiingtype .

aspfacetvalue:slalom-canoekayaking
	rdf:type skos:Concept ;
	skos:prefLabel	"slalom"@en-GB ;
	skos:definition	"White water course set out with gates consisting of two poles suspended vertically over the water. Competitors must negotiate the gates or face penalties."@en-GB ;
	skos:inScheme <http://cv.iptc.org/newscodes/asportfacetvalue/>  ;
	ikos:created "2017-07-04T12:00:00+00:00"^^xsd:dateTime ;
	dct:created "2017-07-04T12:00:00+00:00"^^xsd:dateTime ;
	ikos:modified "2017-07-04T12:00:00+00:00"^^xsd:dateTime ;
	dct:modified "2017-07-04T12:00:00+00:00"^^xsd:dateTime  ;
	ikos:isObjectOf aspfacet:canoekayaktype .

aspfacetvalue:slalom-snowboarding
	rdf:type skos:Concept ;
	skos:prefLabel	"slalom"@en-GB ;
	skos:definition	"Race between narrow set poles or gates."@en-GB ;
	skos:inScheme <http://cv.iptc.org/newscodes/asportfacetvalue/>  ;
	ikos:created "2017-07-04T12:00:00+00:00"^^xsd:dateTime ;
	dct:created "2017-07-04T12:00:00+00:00"^^xsd:dateTime ;
	ikos:modified "2017-07-04T12:00:00+00:00"^^xsd:dateTime ;
	dct:modified "2017-07-04T12:00:00+00:00"^^xsd:dateTime  ;
	ikos:isObjectOf aspfacet:snowboardingtype .

aspfacetvalue:slalom-waterskiing
	rdf:type skos:Concept ;
	skos:prefLabel	"slalom"@en-GB ;
	skos:definition	"Speed event where contestants round a course marked out by buoys"@en-GB ;
	skos:inScheme <http://cv.iptc.org/newscodes/asportfacetvalue/>  ;
	ikos:created "2017-07-04T12:00:00+00:00"^^xsd:dateTime ;
	dct:created "2017-07-04T12:00:00+00:00"^^xsd:dateTime ;
	ikos:modified "2017-07-04T12:00:00+00:00"^^xsd:dateTime ;
	dct:modified "2017-07-04T12:00:00+00:00"^^xsd:dateTime  ;
	ikos:isObjectOf aspfacet:waterskiingtype .

aspfacetvalue:sled
	rdf:type skos:Concept ;
	skos:prefLabel	"sled"@en-GB ;
	skos:definition	"Dog race where dogs are harnessed to a sled."@en-GB ;
	skos:inScheme <http://cv.iptc.org/newscodes/asportfacetvalue/>  ;
	ikos:created "2017-07-04T12:00:00+00:00"^^xsd:dateTime ;
	dct:created "2017-07-04T12:00:00+00:00"^^xsd:dateTime ;
	ikos:modified "2017-07-04T12:00:00+00:00"^^xsd:dateTime ;
	dct:modified "2017-07-04T12:00:00+00:00"^^xsd:dateTime  ;
	ikos:isObjectOf aspfacet:dogracingtype .

aspfacetvalue:snatch
	rdf:type skos:Concept ;
	skos:prefLabel	"snatch"@en-GB ;
	skos:definition	"The bar must be lifted from floor to above the head in one movement"@en-GB ;
	skos:inScheme <http://cv.iptc.org/newscodes/asportfacetvalue/>  ;
	ikos:created "2017-07-04T12:00:00+00:00"^^xsd:dateTime ;
	dct:created "2017-07-04T12:00:00+00:00"^^xsd:dateTime ;
	ikos:modified "2017-07-04T12:00:00+00:00"^^xsd:dateTime ;
	dct:modified "2017-07-04T12:00:00+00:00"^^xsd:dateTime  ;
	ikos:isObjectOf aspfacet:weightliftingtype .

aspfacetvalue:snooker
	rdf:type skos:Concept ;
	skos:prefLabel	"snooker"@en-GB ;
	skos:definition	"Two players using a cue and a white ball to *sink* other coloured balls in a correct order on a baize table and to cause an opponent to miss-hit by positioning the white ball in an inappropriate place."@en-GB ;
	skos:inScheme <http://cv.iptc.org/newscodes/asportfacetvalue/>  ;
	ikos:created "2017-07-04T12:00:00+00:00"^^xsd:dateTime ;
	dct:created "2017-07-04T12:00:00+00:00"^^xsd:dateTime ;
	ikos:modified "2017-07-04T12:00:00+00:00"^^xsd:dateTime ;
	dct:modified "2017-07-04T12:00:00+00:00"^^xsd:dateTime  ;
	ikos:isObjectOf aspfacet:billiardtype .

aspfacetvalue:big-air-snowboarding
	rdf:type skos:Concept ;
	skos:prefLabel	"big-air (snowboarding)"@en-GB ;
	skos:definition	"a competition involving a jump ramp and tricks performed in the air"@en-GB ;
	skos:inScheme <http://cv.iptc.org/newscodes/asportfacetvalue/>  ;
	ikos:created "2019-11-22T12:00:00+00:00"^^xsd:dateTime ;
	dct:created "2019-11-22T12:00:00+00:00"^^xsd:dateTime ;
	ikos:modified "2019-11-22T12:00:00+00:00"^^xsd:dateTime ;
	dct:modified "2019-11-22T12:00:00+00:00"^^xsd:dateTime  ;
	ikos:isObjectOf aspfacet:snowboardingtype .

aspfacetvalue:snowboard-cross
	rdf:type skos:Concept ;
	skos:prefLabel	"snowboard-cross"@en-GB ;
	skos:definition	"a multi-participant downhill sbowboard race on irregular terrain"@en-GB ;
	skos:inScheme <http://cv.iptc.org/newscodes/asportfacetvalue/>  ;
	ikos:created "2019-11-22T12:00:00+00:00"^^xsd:dateTime ;
	dct:created "2019-11-22T12:00:00+00:00"^^xsd:dateTime ;
	ikos:modified "2019-11-22T12:00:00+00:00"^^xsd:dateTime ;
	dct:modified "2019-11-22T12:00:00+00:00"^^xsd:dateTime  ;
	ikos:isObjectOf aspfacet:snowboardingtype .

aspfacetvalue:halfpipe-snowboarding
	rdf:type skos:Concept ;
	skos:prefLabel	"halfpipe (snowboarding)"@en-GB ;
	skos:definition	"a competition involving a semi-circular course with snowboarders performing tricks while going from side to side"@en-GB ;
	skos:inScheme <http://cv.iptc.org/newscodes/asportfacetvalue/>  ;
	ikos:created "2019-11-22T12:00:00+00:00"^^xsd:dateTime ;
	dct:created "2019-11-22T12:00:00+00:00"^^xsd:dateTime ;
	ikos:modified "2019-11-22T12:00:00+00:00"^^xsd:dateTime ;
	dct:modified "2019-11-22T12:00:00+00:00"^^xsd:dateTime  ;
	ikos:isObjectOf aspfacet:snowboardingtype .

aspfacetvalue:soling
	rdf:type skos:Concept ;
	skos:prefLabel	"soling"@en-GB ;
	skos:definition	"Boat Category: three man keel boat"@en-GB ;
	skos:inScheme <http://cv.iptc.org/newscodes/asportfacetvalue/>  ;
	ikos:created "2017-07-04T12:00:00+00:00"^^xsd:dateTime ;
	dct:created "2017-07-04T12:00:00+00:00"^^xsd:dateTime ;
	ikos:modified "2017-07-04T12:00:00+00:00"^^xsd:dateTime ;
	dct:modified "2017-07-04T12:00:00+00:00"^^xsd:dateTime  ;
	ikos:isObjectOf aspfacet:sailingtype .

aspfacetvalue:speedway
	rdf:type skos:Concept ;
	skos:prefLabel	"speedway"@en-GB ;
	skos:definition	"Motorcycle race involving up to six riders competing over a flat oval track. Speedway motorcycles use only one gear and have no brakes."@en-GB ;
	skos:inScheme <http://cv.iptc.org/newscodes/asportfacetvalue/>  ;
	ikos:created "2017-07-04T12:00:00+00:00"^^xsd:dateTime ;
	dct:created "2017-07-04T12:00:00+00:00"^^xsd:dateTime ;
	ikos:modified "2017-07-04T12:00:00+00:00"^^xsd:dateTime ;
	dct:modified "2017-07-04T12:00:00+00:00"^^xsd:dateTime  ;
	ikos:isObjectOf aspfacet:motorcyclingtype .

aspfacetvalue:sprint
	rdf:type skos:Concept ;
	skos:prefLabel	"sprint"@en-GB ;
	skos:definition	"A race over a shorter distance than is traditional and that focuses on speed."@en-GB ;
	skos:inScheme <http://cv.iptc.org/newscodes/asportfacetvalue/>  ;
	ikos:created "2017-07-04T12:00:00+00:00"^^xsd:dateTime ;
	dct:created "2017-07-04T12:00:00+00:00"^^xsd:dateTime ;
	ikos:modified "2017-07-04T12:00:00+00:00"^^xsd:dateTime ;
	dct:modified "2017-07-04T12:00:00+00:00"^^xsd:dateTime  ;
	ikos:isObjectOf aspfacet:racetype .

aspfacetvalue:staged
	rdf:type skos:Concept ;
	skos:prefLabel	"staged"@en-GB ;
	skos:definition	"A race divided into different parts based on time or distance."@en-GB ;
	skos:inScheme <http://cv.iptc.org/newscodes/asportfacetvalue/>  ;
	ikos:created "2017-07-04T12:00:00+00:00"^^xsd:dateTime ;
	dct:created "2017-07-04T12:00:00+00:00"^^xsd:dateTime ;
	ikos:modified "2017-07-04T12:00:00+00:00"^^xsd:dateTime ;
	dct:modified "2017-07-04T12:00:00+00:00"^^xsd:dateTime  ;
	ikos:isObjectOf aspfacet:racetype .

aspfacetvalue:star
	rdf:type skos:Concept ;
	skos:prefLabel	"star"@en-GB ;
	skos:definition	"Boat Category: two man keel boat (7.10m/sq mainsail) Olympic sport "@en-GB ;
	skos:inScheme <http://cv.iptc.org/newscodes/asportfacetvalue/>  ;
	ikos:created "2017-07-04T12:00:00+00:00"^^xsd:dateTime ;
	dct:created "2017-07-04T12:00:00+00:00"^^xsd:dateTime ;
	ikos:modified "2017-07-04T12:00:00+00:00"^^xsd:dateTime ;
	dct:modified "2017-07-04T12:00:00+00:00"^^xsd:dateTime  ;
	ikos:isObjectOf aspfacet:sailingtype .

aspfacetvalue:steeplechase
	rdf:type skos:Concept ;
	skos:prefLabel	"steeplechase"@en-GB ;
	skos:definition	"A mounted horse race over at least eight classic obstacles, four of which must be different, such as the water jump, spruce fences, mud walls etc."@en-GB ;
	skos:inScheme <http://cv.iptc.org/newscodes/asportfacetvalue/>  ;
	ikos:created "2017-07-04T12:00:00+00:00"^^xsd:dateTime ;
	dct:created "2017-07-04T12:00:00+00:00"^^xsd:dateTime ;
	ikos:modified "2019-07-23T12:00:00+00:00"^^xsd:dateTime ;
	dct:modified "2019-07-23T12:00:00+00:00"^^xsd:dateTime  ;
	ikos:isObjectOf aspfacet:horseracingtype .

aspfacetvalue:street
	rdf:type skos:Concept ;
	skos:prefLabel	"street"@en-GB ;
	skos:definition	"BMX that makes use of urban and public spaces to perform tricks."@en-GB ;
	skos:inScheme <http://cv.iptc.org/newscodes/asportfacetvalue/>  ;
	ikos:created "2017-07-04T12:00:00+00:00"^^xsd:dateTime ;
	dct:created "2017-07-04T12:00:00+00:00"^^xsd:dateTime ;
	ikos:modified "2017-07-04T12:00:00+00:00"^^xsd:dateTime ;
	dct:modified "2017-07-04T12:00:00+00:00"^^xsd:dateTime  ;
	ikos:isObjectOf aspfacet:bmxfreestyletype .

aspfacetvalue:supercross
	rdf:type skos:Concept ;
	skos:prefLabel	"supercross"@en-GB ;
	skos:definition	"Racing specialized high performance off-road motorcycles on artificially made dirt tracks consisting of steep jumps and obstacles"@en-GB ;
	skos:inScheme <http://cv.iptc.org/newscodes/asportfacetvalue/>  ;
	ikos:created "2017-07-04T12:00:00+00:00"^^xsd:dateTime ;
	dct:created "2017-07-04T12:00:00+00:00"^^xsd:dateTime ;
	ikos:modified "2017-07-04T12:00:00+00:00"^^xsd:dateTime ;
	dct:modified "2017-07-04T12:00:00+00:00"^^xsd:dateTime  ;
	ikos:isObjectOf aspfacet:motorcyclingtype .

aspfacetvalue:superg
	rdf:type skos:Concept ;
	skos:prefLabel	"super-G"@en-GB ;
	skos:definition	"Alpine skiing speed race between widly set gates. "@en-GB ;
	skos:inScheme <http://cv.iptc.org/newscodes/asportfacetvalue/>  ;
	ikos:created "2017-07-04T12:00:00+00:00"^^xsd:dateTime ;
	dct:created "2017-07-04T12:00:00+00:00"^^xsd:dateTime ;
	ikos:modified "2017-07-04T12:00:00+00:00"^^xsd:dateTime ;
	dct:modified "2017-07-04T12:00:00+00:00"^^xsd:dateTime  ;
	ikos:isObjectOf aspfacet:alpineskiingtype .

aspfacetvalue:teamsprint-cycling
	rdf:type skos:Concept ;
	skos:prefLabel	"team sprint"@en-GB ;
	skos:definition	"Track cycling event.  The men's event involves a three-man team time trial held over three laps in a velodrome. The women's event involves a two-woman event held over two laps."@en-GB ;
	skos:inScheme <http://cv.iptc.org/newscodes/asportfacetvalue/>  ;
	ikos:created "2017-07-04T12:00:00+00:00"^^xsd:dateTime ;
	dct:created "2017-07-04T12:00:00+00:00"^^xsd:dateTime ;
	ikos:modified "2017-07-04T12:00:00+00:00"^^xsd:dateTime ;
	dct:modified "2017-07-04T12:00:00+00:00"^^xsd:dateTime  ;
	ikos:isObjectOf aspfacet:cyclingtype .

aspfacetvalue:teamsprint-nordicskiing
	rdf:type skos:Concept ;
	skos:prefLabel	"team sprint"@en-GB ;
	skos:definition	"Skiing competition where two skiers do three laps each alternating around a short ski course. There are qualification rounds that lead to a final."@en-GB ;
	skos:note	"Moved from *nordicskiingtype* to *crosscountryskiingtype* in August 2019"@en-GB ;
	skos:inScheme <http://cv.iptc.org/newscodes/asportfacetvalue/>  ;
	ikos:created "2017-07-04T12:00:00+00:00"^^xsd:dateTime ;
	dct:created "2017-07-04T12:00:00+00:00"^^xsd:dateTime ;
	ikos:modified "2017-07-04T12:00:00+00:00"^^xsd:dateTime ;
	dct:modified "2017-07-04T12:00:00+00:00"^^xsd:dateTime  ;
	ikos:isObjectOf aspfacet:crosscountryskiingtype .

aspfacetvalue:time-trial
	rdf:type skos:Concept ;
	skos:prefLabel	"time trial"@en-GB ;
	skos:definition	"Race in a fixed distance against the clock."@en-GB ;
	skos:inScheme <http://cv.iptc.org/newscodes/asportfacetvalue/>  ;
	ikos:created "2017-07-04T12:00:00+00:00"^^xsd:dateTime ;
	dct:created "2017-07-04T12:00:00+00:00"^^xsd:dateTime ;
	ikos:modified "2017-07-04T12:00:00+00:00"^^xsd:dateTime ;
	dct:modified "2017-07-04T12:00:00+00:00"^^xsd:dateTime  ;
	ikos:isObjectOf aspfacet:racetype .

aspfacetvalue:tornado
	rdf:type skos:Concept ;
	skos:prefLabel	"tornado"@en-GB ;
	skos:definition	"Boat Category: two man catamaran (21m/sq mainsail) Olympic sport "@en-GB ;
	skos:inScheme <http://cv.iptc.org/newscodes/asportfacetvalue/>  ;
	ikos:created "2017-07-04T12:00:00+00:00"^^xsd:dateTime ;
	dct:created "2017-07-04T12:00:00+00:00"^^xsd:dateTime ;
	ikos:modified "2017-07-04T12:00:00+00:00"^^xsd:dateTime ;
	dct:modified "2017-07-04T12:00:00+00:00"^^xsd:dateTime  ;
	ikos:isObjectOf aspfacet:sailingtype .

aspfacetvalue:track
	rdf:type skos:Concept ;
	skos:prefLabel	"track"@en-GB ;
	skos:definition	"A bicycle racing sport usually held on specially built banked tracks or velodromes using track bicycles."@en-GB ;
	skos:inScheme <http://cv.iptc.org/newscodes/asportfacetvalue/>  ;
	ikos:created "2017-07-04T12:00:00+00:00"^^xsd:dateTime ;
	dct:created "2017-07-04T12:00:00+00:00"^^xsd:dateTime ;
	ikos:modified "2017-07-04T12:00:00+00:00"^^xsd:dateTime ;
	dct:modified "2017-07-04T12:00:00+00:00"^^xsd:dateTime  ;
	ikos:isObjectOf aspfacet:cyclingtype .

aspfacetvalue:trap
	rdf:type skos:Concept ;
	skos:prefLabel	"trap"@en-GB ;
	skos:definition	"Shooting event with moving targets shot from a single machine, generally away from the shooter."@en-GB ;
	skos:inScheme <http://cv.iptc.org/newscodes/asportfacetvalue/>  ;
	ikos:created "2017-07-04T12:00:00+00:00"^^xsd:dateTime ;
	dct:created "2017-07-04T12:00:00+00:00"^^xsd:dateTime ;
	ikos:modified "2017-07-04T12:00:00+00:00"^^xsd:dateTime ;
	dct:modified "2017-07-04T12:00:00+00:00"^^xsd:dateTime  ;
	ikos:isObjectOf aspfacet:shootingtype .

aspfacetvalue:TRC
	rdf:type skos:Concept ;
	skos:prefLabel	"TRC"@en-GB ;
	skos:definition	"In the TRC (Throw Run Catch) sub event the player throws a disc and then runs to catch it as far away as possible with one hand before it hits the ground. "@en-GB ;
	skos:inScheme <http://cv.iptc.org/newscodes/asportfacetvalue/>  ;
	ikos:created "2017-07-04T12:00:00+00:00"^^xsd:dateTime ;
	dct:created "2017-07-04T12:00:00+00:00"^^xsd:dateTime ;
	ikos:modified "2017-07-04T12:00:00+00:00"^^xsd:dateTime ;
	dct:modified "2017-07-04T12:00:00+00:00"^^xsd:dateTime  ;
	ikos:isObjectOf aspfacet:flyingdisctype .

aspfacetvalue:trial
	rdf:type skos:Concept ;
	skos:prefLabel	"trial"@en-GB ;
	skos:definition	"A timed race in which competitors must negotiate tricky terrain and obstacles without putting their feet down."@en-GB ;
	skos:inScheme <http://cv.iptc.org/newscodes/asportfacetvalue/>  ;
	ikos:created "2017-07-04T12:00:00+00:00"^^xsd:dateTime ;
	dct:created "2017-07-04T12:00:00+00:00"^^xsd:dateTime ;
	ikos:modified "2017-07-04T12:00:00+00:00"^^xsd:dateTime ;
	dct:modified "2017-07-04T12:00:00+00:00"^^xsd:dateTime  ;
	ikos:isObjectOf aspfacet:racetype .

aspfacetvalue:trick
	rdf:type skos:Concept ;
	skos:prefLabel	"trick"@en-GB ;
	skos:definition	"Skiers perform a maximum of figures in a limited time period"@en-GB ;
	skos:inScheme <http://cv.iptc.org/newscodes/asportfacetvalue/>  ;
	ikos:created "2017-07-04T12:00:00+00:00"^^xsd:dateTime ;
	dct:created "2017-07-04T12:00:00+00:00"^^xsd:dateTime ;
	ikos:modified "2017-07-04T12:00:00+00:00"^^xsd:dateTime ;
	dct:modified "2017-07-04T12:00:00+00:00"^^xsd:dateTime  ;
	ikos:isObjectOf aspfacet:waterskiingtype .

aspfacetvalue:trinquet
	rdf:type skos:Concept ;
	skos:prefLabel	"trinquet"@en-GB ;
	skos:definition	"A *Trinquet* is an indoor fronton with a 28.5 meters long court surrounded by four walls. The four walls are used in the game. "@en-GB ;
	skos:inScheme <http://cv.iptc.org/newscodes/asportfacetvalue/>  ;
	ikos:created "2017-07-04T12:00:00+00:00"^^xsd:dateTime ;
	dct:created "2017-07-04T12:00:00+00:00"^^xsd:dateTime ;
	ikos:modified "2017-07-04T12:00:00+00:00"^^xsd:dateTime ;
	dct:modified "2017-07-04T12:00:00+00:00"^^xsd:dateTime  ;
	ikos:isObjectOf aspfacet:jaialaitype .

aspfacetvalue:trotting
	rdf:type skos:Concept ;
	skos:prefLabel	"trotting"@en-GB ;
	skos:definition	"Horses pitched to a jockeyed buggy race in a trot round a flat course."@en-GB ;
	skos:inScheme <http://cv.iptc.org/newscodes/asportfacetvalue/>  ;
	ikos:created "2017-07-04T12:00:00+00:00"^^xsd:dateTime ;
	dct:created "2017-07-04T12:00:00+00:00"^^xsd:dateTime ;
	ikos:modified "2017-07-04T12:00:00+00:00"^^xsd:dateTime ;
	dct:modified "2017-07-04T12:00:00+00:00"^^xsd:dateTime  ;
	ikos:isObjectOf aspfacet:horseracingtype .

aspfacetvalue:ultimate
	rdf:type skos:Concept ;
	skos:prefLabel	"ultimate"@en-GB ;
	skos:definition	"Team game. Played outdoors on soccer-size field with 7 players per team and indoors with 5 players per team. Games are played to a preset number of goals. Goals are scored by passing the disc to a team-member catching it inside the goal area. "@en-GB ;
	skos:inScheme <http://cv.iptc.org/newscodes/asportfacetvalue/>  ;
	ikos:created "2017-07-04T12:00:00+00:00"^^xsd:dateTime ;
	dct:created "2017-07-04T12:00:00+00:00"^^xsd:dateTime ;
	ikos:modified "2017-07-04T12:00:00+00:00"^^xsd:dateTime ;
	dct:modified "2017-07-04T12:00:00+00:00"^^xsd:dateTime  ;
	ikos:isObjectOf aspfacet:flyingdisctype .

aspfacetvalue:unevenbars
	rdf:type skos:Concept ;
	skos:prefLabel	"uneven bars"@en-GB ;
	skos:definition	"Artistic gymnastics event where gymnasts run through an airborne routine swinging around and between the uneven bars."@en-GB ;
	skos:inScheme <http://cv.iptc.org/newscodes/asportfacetvalue/>  ;
	ikos:created "2017-07-04T12:00:00+00:00"^^xsd:dateTime ;
	dct:created "2017-07-04T12:00:00+00:00"^^xsd:dateTime ;
	ikos:modified "2017-07-04T12:00:00+00:00"^^xsd:dateTime ;
	dct:modified "2017-07-04T12:00:00+00:00"^^xsd:dateTime  ;
	ikos:isObjectOf aspfacet:artisticgymtype .

aspfacetvalue:vault
	rdf:type skos:Concept ;
	skos:prefLabel	"vault"@en-GB ;
	skos:definition	"Artistic gymnastics event where gymnasts propel themselves by jumping on a trampoline after running quickly down a 25m lane."@en-GB ;
	skos:inScheme <http://cv.iptc.org/newscodes/asportfacetvalue/>  ;
	ikos:created "2017-07-04T12:00:00+00:00"^^xsd:dateTime ;
	dct:created "2017-07-04T12:00:00+00:00"^^xsd:dateTime ;
	ikos:modified "2017-07-04T12:00:00+00:00"^^xsd:dateTime ;
	dct:modified "2017-07-04T12:00:00+00:00"^^xsd:dateTime  ;
	ikos:isObjectOf aspfacet:artisticgymtype .

aspfacetvalue:vaulting
	rdf:type skos:Concept ;
	skos:prefLabel	"vaulting"@en-GB ;
	skos:definition	"Gymnastics and dance performed on horseback."@en-GB ;
	skos:inScheme <http://cv.iptc.org/newscodes/asportfacetvalue/>  ;
	ikos:created "2017-07-04T12:00:00+00:00"^^xsd:dateTime ;
	dct:created "2017-07-04T12:00:00+00:00"^^xsd:dateTime ;
	ikos:modified "2017-07-04T12:00:00+00:00"^^xsd:dateTime ;
	dct:modified "2017-07-04T12:00:00+00:00"^^xsd:dateTime  ;
	ikos:isObjectOf aspfacet:equestriantype .

aspfacetvalue:vertramp
	rdf:type skos:Concept ;
	skos:prefLabel	"vert ramp"@en-GB ;
	skos:definition	"BMX competition held on a vert ramp which allows the competitors to fly into the air and land back on the ramp."@en-GB ;
	skos:inScheme <http://cv.iptc.org/newscodes/asportfacetvalue/>  ;
	ikos:created "2017-07-04T12:00:00+00:00"^^xsd:dateTime ;
	dct:created "2017-07-04T12:00:00+00:00"^^xsd:dateTime ;
	ikos:modified "2017-07-04T12:00:00+00:00"^^xsd:dateTime ;
	dct:modified "2017-07-04T12:00:00+00:00"^^xsd:dateTime  ;
	ikos:isObjectOf aspfacet:bmxfreestyletype .

aspfacetvalue:vtt-cross
	rdf:type skos:Concept ;
	skos:prefLabel	"vtt-cross"@en-GB ;
	skos:definition	"An endurance race on mountain bikes around a 10km circuit over various terrain and with different degrees of slopes. Competitors are not allowed any exterior help."@en-GB ;
	skos:inScheme <http://cv.iptc.org/newscodes/asportfacetvalue/>  ;
	ikos:created "2017-07-04T12:00:00+00:00"^^xsd:dateTime ;
	dct:created "2017-07-04T12:00:00+00:00"^^xsd:dateTime ;
	ikos:modified "2017-07-04T12:00:00+00:00"^^xsd:dateTime ;
	dct:modified "2017-07-04T12:00:00+00:00"^^xsd:dateTime  ;
	ikos:isObjectOf aspfacet:mountainbikingtype .

aspfacetvalue:vtt-downhill
	rdf:type skos:Concept ;
	skos:prefLabel	"vtt-downhill"@en-GB ;
	skos:definition	"Individual mountain bike race against the clock staged on a downhill circuit featuring obstacles."@en-GB ;
	skos:inScheme <http://cv.iptc.org/newscodes/asportfacetvalue/>  ;
	ikos:created "2017-07-04T12:00:00+00:00"^^xsd:dateTime ;
	dct:created "2017-07-04T12:00:00+00:00"^^xsd:dateTime ;
	ikos:modified "2017-07-04T12:00:00+00:00"^^xsd:dateTime ;
	dct:modified "2017-07-04T12:00:00+00:00"^^xsd:dateTime  ;
	ikos:isObjectOf aspfacet:mountainbikingtype .

aspfacetvalue:women
	rdf:type skos:Concept ;
	skos:prefLabel	"women "@en-GB ;
	skos:definition	"Single female human person"@en-GB ;
	skos:inScheme <http://cv.iptc.org/newscodes/asportfacetvalue/>  ;
	ikos:created "2017-07-04T12:00:00+00:00"^^xsd:dateTime ;
	dct:created "2017-07-04T12:00:00+00:00"^^xsd:dateTime ;
	ikos:modified "2017-07-04T12:00:00+00:00"^^xsd:dateTime ;
	dct:modified "2017-07-04T12:00:00+00:00"^^xsd:dateTime  ;
	ikos:isObjectOf aspfacet:gender .

aspfacetvalue:xare
	rdf:type skos:Concept ;
	skos:prefLabel	"xare"@en-GB ;
	skos:definition	"The *xare*, is the name of the game played in a trinquet by teams of 2 players. The players use a *xare* (or the Argentina bat) 55 cm long and 16 cm wide. "@en-GB ;
	skos:inScheme <http://cv.iptc.org/newscodes/asportfacetvalue/>  ;
	ikos:created "2017-07-04T12:00:00+00:00"^^xsd:dateTime ;
	dct:created "2017-07-04T12:00:00+00:00"^^xsd:dateTime ;
	ikos:modified "2017-07-04T12:00:00+00:00"^^xsd:dateTime ;
	dct:modified "2017-07-04T12:00:00+00:00"^^xsd:dateTime  ;
	ikos:isObjectOf aspfacet:jaialaitype .

aspfacetvalue:yngling
	rdf:type skos:Concept ;
	skos:prefLabel	"yngling"@en-GB ;
	skos:definition	"Olympic boat class. A race around different courses in a boat of 6.35 metres (20ft 10in) long and 1.73 metres (5ft 8in) wide, crewed in Olympic competition only by women. The number of races and the length of the courses varies. "@en-GB ;
	skos:inScheme <http://cv.iptc.org/newscodes/asportfacetvalue/>  ;
	ikos:created "2017-07-04T12:00:00+00:00"^^xsd:dateTime ;
	dct:created "2017-07-04T12:00:00+00:00"^^xsd:dateTime ;
	ikos:modified "2017-07-04T12:00:00+00:00"^^xsd:dateTime ;
	dct:modified "2017-07-04T12:00:00+00:00"^^xsd:dateTime  ;
	ikos:isObjectOf aspfacet:sailingtype .
