
@prefix rdf:	<http://www.w3.org/1999/02/22-rdf-syntax-ns#>.
@prefix skos:	<http://www.w3.org/2004/02/skos/core#>.
@prefix owl:	<http://www.w3.org/2002/07/owl#>.
@prefix sptournamentform:	<http://cv.iptc.org/newscodes/sptournamentform/>
		
<http://cv.iptc.org/newscodes/sptournamentform/> 
	rdf:type skos:ConceptScheme;
	skos:HasTopConcept		sptournamentform:hosted;
	skos:HasTopConcept		sptournamentform:single-group;
	skos:HasTopConcept		sptournamentform:series;
	skos:HasTopConcept		sptournamentform:single-elimination;
	skos:HasTopConcept		sptournamentform:home-and-home.

sptournamentform:hosted
	rdf:type skos:Concept;
	skos:prefLabel	"hosted"@en-GB;
	skos:definition	"For a tournament that holds stages in different locations. Eg. different host cities/countries for PGA, FIS, Diamond League (IAAF) and even Tour de France"@en-GB;
	skos:inScheme <http://cv.iptc.org/newscodes/sptournamentform/>.

sptournamentform:single-group
	rdf:type skos:Concept;
	skos:prefLabel	"single-group"@en-GB;
	skos:definition	"The stage involves only a single group of competitors. For example Italian Serie A where teams vie for placement in the league table. Also, a single group competition in a multi-group stage, such as the World Cup group stage."@en-GB;
	skos:inScheme <http://cv.iptc.org/newscodes/sptournamentform/>.

sptournamentform:series
	rdf:type skos:Concept;
	skos:prefLabel	"series"@en-GB;
	skos:definition	"A stage in which two competitors face off in a series of games (eg. best 3 of 5) the winner of which proceeds to the next stage, or wins the tournament."@en-GB;
	skos:inScheme <http://cv.iptc.org/newscodes/sptournamentform/>.

sptournamentform:single-elimination
	rdf:type skos:Concept;
	skos:prefLabel	"single-elimination"@en-GB;
	skos:definition	"A stage in which two competitors face off in a single match to determine who proceeds to the next stage, or wins the tournament. Eg. elimination stage of World Cup of Soccer or NFL playoffs."@en-GB;
	skos:inScheme <http://cv.iptc.org/newscodes/sptournamentform/>.

sptournamentform:home-and-home
	rdf:type skos:Concept;
	skos:prefLabel	"home-and-home"@en-GB;
	skos:definition	"A stage in which two competitors face off in a two matches (or legs) at each team's home location. The overall winner proceeds ahead. Usually culiminates in a single-elimination match at a neutral location i.e. UEFA Champions League."@en-GB;
	skos:inScheme <http://cv.iptc.org/newscodes/sptournamentform/>.
