spamfstat:yardsPerAttempt rdf:type rdf:Property ; 
        rdfs:label "yardsPerAttempt"@en ; 
        rdfs:comment "The average yards gained per play."@en ; 
        rdfs:domain [fill in] ; 
        rdfs:range xsd:integer ; 
        rdf:isDefinedBy <https://sportschema.org/ontologies/american-football-statistics> . 
        
	spamfstat:numberOfPlays rdf:type rdf:Property ; 
        rdfs:label "numberOfPlays"@en ; 
        rdfs:comment "The number of plays this team has completed, including for
                offensive, defensive, and special teams."@en ; 
        rdfs:domain [fill in] ; 
        rdfs:range xsd:integer ; 
        rdf:isDefinedBy <https://sportschema.org/ontologies/american-football-statistics> . 
        
	spamfstat:numberOfPlaysGaining rdf:type rdf:Property ; 
        rdfs:label "numberOfPlaysGaining"@en ; 
        rdfs:comment "The number of plays this team has completed for which yards
                were gained, including for offensive, defensive, and special teams."@en ; 
        rdfs:domain [fill in] ; 
        rdfs:range xsd:integer ; 
        rdf:isDefinedBy <https://sportschema.org/ontologies/american-football-statistics> . 
        
	spamfstat:numberOfPlaysLosing rdf:type rdf:Property ; 
        rdfs:label "numberOfPlaysLosing"@en ; 
        rdfs:comment "The number of plays this team has completed for which yards
                were lost, including for offensive, defensive, and special teams."@en ; 
        rdfs:domain [fill in] ; 
        rdfs:range xsd:integer ; 
        rdf:isDefinedBy <https://sportschema.org/ontologies/american-football-statistics> . 
        
	spamfstat:averageStartingPosition rdf:type rdf:Property ; 
        rdfs:label "averageStartingPosition"@en ; 
        rdfs:comment "Average yard-line that the team started on
                per-drive."@en ; 
        rdfs:domain [fill in] ; 
        rdfs:range xsd:integer ; 
        rdf:isDefinedBy <https://sportschema.org/ontologies/american-football-statistics> . 
        
	spamfstat:timeouts rdf:type rdf:Property ; 
        rdfs:label "timeouts"@en ; 
        rdfs:comment "The number of timeouts a team has remaining, either in
                regulation or in overtime, whichever state the game is currently in."@en ; 
        rdfs:domain [fill in] ; 
        rdfs:range xsd:integer ; 
        rdf:isDefinedBy <https://sportschema.org/ontologies/american-football-statistics> . 
        
	spamfstat:turnoverRatio rdf:type rdf:Property ; 
        rdfs:label "turnoverRatio"@en ; 
        rdfs:comment "Derived by subtracting turnovers-giveaways from
                turnovers-takeaways."@en ; 
        rdfs:domain [fill in] ; 
        rdfs:range xsd:integer ; 
        rdf:isDefinedBy <https://sportschema.org/ontologies/american-football-statistics> . 
        
	spamfstat:offensivePlaysYards rdf:type rdf:Property ; 
        rdfs:label "offensivePlaysYards"@en ; 
        rdfs:comment "The total yards accumulated through offensive
                plays."@en ; 
        rdfs:domain [fill in] ; 
        rdfs:range xsd:integer ; 
        rdf:isDefinedBy <https://sportschema.org/ontologies/american-football-statistics> . 
        
	spamfstat:offensivePlaysNumber rdf:type rdf:Property ; 
        rdfs:label "offensivePlaysNumber"@en ; 
        rdfs:comment "The number of offensive plays."@en ; 
        rdfs:domain [fill in] ; 
        rdfs:range xsd:integer ; 
        rdf:isDefinedBy <https://sportschema.org/ontologies/american-football-statistics> . 
        
	spamfstat:offensivePlaysAverageYardsPer rdf:type rdf:Property ; 
        rdfs:label "offensivePlaysAverageYardsPer"@en ; 
        rdfs:comment "The average number of yards gained per play."@en ; 
        rdfs:domain [fill in] ; 
        rdfs:range xsd:integer ; 
        rdf:isDefinedBy <https://sportschema.org/ontologies/american-football-statistics> . 
        
	spamfstat:offensivePlaysAverageYardsPerGame rdf:type rdf:Property ; 
        rdfs:label "offensivePlaysAverageYardsPerGame"@en ; 
        rdfs:comment "The average number of yards gained via offensive plays per
                game."@en ; 
        rdfs:domain [fill in] ; 
        rdfs:range xsd:integer ; 
        rdf:isDefinedBy <https://sportschema.org/ontologies/american-football-statistics> . 
        
	spamfstat:offensiveRank rdf:type rdf:Property ; 
        rdfs:label "offensiveRank"@en ; 
        rdfs:comment "How team's offense compares with rest of league or
                conference."@en ; 
        rdfs:domain [fill in] ; 
        rdfs:range xsd:integer ; 
        rdf:isDefinedBy <https://sportschema.org/ontologies/american-football-statistics> . 
        
	spamfstat:possessionDuration rdf:type rdf:Property ; 
        rdfs:label "possessionDuration"@en ; 
        rdfs:comment "The average amount of time the team had possession
                per-drive."@en ; 
        rdfs:domain [fill in] ; 
        rdfs:range xsd:integer ; 
        rdf:isDefinedBy <https://sportschema.org/ontologies/american-football-statistics> . 
        
	spamfstat:possessionsInside20 rdf:type rdf:Property ; 
        rdfs:label "possessionsInside20"@en ; 
        rdfs:comment "Number of times team has driven inside its opponent's 20
                yard line."@en ; 
        rdfs:domain [fill in] ; 
        rdfs:range xsd:integer ; 
        rdf:isDefinedBy <https://sportschema.org/ontologies/american-football-statistics> . 
        
	spamfstat:turnoversGiveaway rdf:type rdf:Property ; 
        rdfs:label "turnoversGiveaway"@en ; 
        rdfs:comment "Derived by adding passes-interceptions plus
                fumbles-own-lost."@en ; 
        rdfs:domain [fill in] ; 
        rdfs:range xsd:integer ; 
        rdf:isDefinedBy <https://sportschema.org/ontologies/american-football-statistics> . 
        
	spamfstat:turnoversGiveawayAverage rdf:type rdf:Property ; 
        rdfs:label "turnoversGiveawayAverage"@en ; 
        rdfs:comment "Average-per-game for turnovers-giveaway."@en ; 
        rdfs:domain [fill in] ; 
        rdfs:range xsd:integer ; 
        rdf:isDefinedBy <https://sportschema.org/ontologies/american-football-statistics> . 
        
	spamfstat:handoffsTotal rdf:type rdf:Property ; 
        rdfs:label "handoffsTotal"@en ; 
        rdfs:comment "Usually, number of times QB has handed off, typically
                leading to a running play."@en ; 
        rdfs:domain [fill in] ; 
        rdfs:range xsd:integer ; 
        rdf:isDefinedBy <https://sportschema.org/ontologies/american-football-statistics> . 
        
	spamfstat:pitchesTotal rdf:type rdf:Property ; 
        rdfs:label "pitchesTotal"@en ; 
        rdfs:comment "Usually, number of times QB has pitched back to another
                player, typically leading to a running play."@en ; 
        rdfs:domain [fill in] ; 
        rdfs:range xsd:integer ; 
        rdf:isDefinedBy <https://sportschema.org/ontologies/american-football-statistics> . 
        
	spamfstat:tacklesOffense rdf:type rdf:Property ; 
        rdfs:label "tacklesOffense"@en ; 
        rdfs:comment "The number of tackles performed while on
                offense."@en ; 
        rdfs:domain [fill in] ; 
        rdfs:range xsd:integer ; 
        rdf:isDefinedBy <https://sportschema.org/ontologies/american-football-statistics> . 
        
	spamfstat:tacklesAssistsOffense rdf:type rdf:Property ; 
        rdfs:label "tacklesAssistsOffense"@en ; 
        rdfs:comment "The number of tackle assists performed while on
                offense."@en ; 
        rdfs:domain [fill in] ; 
        rdfs:range xsd:integer ; 
        rdf:isDefinedBy <https://sportschema.org/ontologies/american-football-statistics> . 
        
	spamfstat:passesAttempts rdf:type rdf:Property ; 
        rdfs:label "passesAttempts"@en ; 
        rdfs:comment "The number of passes attempted."@en ; 
        rdfs:domain [fill in] ; 
        rdfs:range xsd:integer ; 
        rdf:isDefinedBy <https://sportschema.org/ontologies/american-football-statistics> . 
        
	spamfstat:passesCompletions rdf:type rdf:Property ; 
        rdfs:label "passesCompletions"@en ; 
        rdfs:comment "The number of passes completed successfully."@en ; 
        rdfs:domain [fill in] ; 
        rdfs:range xsd:integer ; 
        rdf:isDefinedBy <https://sportschema.org/ontologies/american-football-statistics> . 
        
	spamfstat:passesCompletionsAveragePerGame rdf:type rdf:Property ; 
        rdfs:label "passesCompletionsAveragePerGame"@en ; 
        rdfs:comment "Average number of completed passes a game."@en ; 
        rdfs:domain [fill in] ; 
        rdfs:range xsd:integer ; 
        rdf:isDefinedBy <https://sportschema.org/ontologies/american-football-statistics> . 
        
	spamfstat:passesPercentage rdf:type rdf:Property ; 
        rdfs:label "passesPercentage"@en ; 
        rdfs:comment "The percentage of all passes that are completed
                successfully."@en ; 
        rdfs:domain [fill in] ; 
        rdfs:range xsd:integer ; 
        rdf:isDefinedBy <https://sportschema.org/ontologies/american-football-statistics> . 
        
	spamfstat:passesYardsGross rdf:type rdf:Property ; 
        rdfs:label "passesYardsGross"@en ; 
        rdfs:comment "The number of yards gained from passing."@en ; 
        rdfs:domain [fill in] ; 
        rdfs:range xsd:integer ; 
        rdf:isDefinedBy <https://sportschema.org/ontologies/american-football-statistics> . 
        
	spamfstat:passesYardsNet rdf:type rdf:Property ; 
        rdfs:label "passesYardsNet"@en ; 
        rdfs:comment "Subtracts out the sacks-against-yards-lost value of
                stats-american-football-sacks-against element."@en ; 
        rdfs:domain [fill in] ; 
        rdfs:range xsd:integer ; 
        rdf:isDefinedBy <https://sportschema.org/ontologies/american-football-statistics> . 
        
	spamfstat:passesYardsLost rdf:type rdf:Property ; 
        rdfs:label "passesYardsLost"@en ; 
        rdfs:comment "Amount of yards lost due to sacks and completed passing
                plays that ended behind the line of scrimmage."@en ; 
        rdfs:domain [fill in] ; 
        rdfs:range xsd:integer ; 
        rdf:isDefinedBy <https://sportschema.org/ontologies/american-football-statistics> . 
        
	spamfstat:passesYardsPerAttempt rdf:type rdf:Property ; 
        rdfs:label "passesYardsPerAttempt"@en ; 
        rdfs:comment "Gross passing yards divided by number of pass
                attempts."@en ; 
        rdfs:domain [fill in] ; 
        rdfs:range xsd:integer ; 
        rdf:isDefinedBy <https://sportschema.org/ontologies/american-football-statistics> . 
        
	spamfstat:passesFirstDown rdf:type rdf:Property ; 
        rdfs:label "passesFirstDown"@en ; 
        rdfs:comment "Number of passes a player or team has made for a
                first-down."@en ; 
        rdfs:domain [fill in] ; 
        rdfs:range xsd:integer ; 
        rdf:isDefinedBy <https://sportschema.org/ontologies/american-football-statistics> . 
        
	spamfstat:passesTouchdownsPercentage rdf:type rdf:Property ; 
        rdfs:label "passesTouchdownsPercentage"@en ; 
        rdfs:comment "The ratio of touchdown passes to attempted
                passes."@en ; 
        rdfs:domain [fill in] ; 
        rdfs:range xsd:integer ; 
        rdf:isDefinedBy <https://sportschema.org/ontologies/american-football-statistics> . 
        
	spamfstat:passesInterceptions rdf:type rdf:Property ; 
        rdfs:label "passesInterceptions"@en ; 
        rdfs:comment "The number of passes that were intercepted."@en ; 
        rdfs:domain [fill in] ; 
        rdfs:range xsd:integer ; 
        rdf:isDefinedBy <https://sportschema.org/ontologies/american-football-statistics> . 
        
	spamfstat:passesInterceptionsPercentage rdf:type rdf:Property ; 
        rdfs:label "passesInterceptionsPercentage"@en ; 
        rdfs:comment "The ratio of intercepted passes to attempted
                passes."@en ; 
        rdfs:domain [fill in] ; 
        rdfs:range xsd:integer ; 
        rdf:isDefinedBy <https://sportschema.org/ontologies/american-football-statistics> . 
        
	spamfstat:passesInterceptionsYards rdf:type rdf:Property ; 
        rdfs:label "passesInterceptionsYards"@en ; 
        rdfs:comment "Opponent's yards gained after interceptions."@en ; 
        rdfs:domain [fill in] ; 
        rdfs:range xsd:integer ; 
        rdf:isDefinedBy <https://sportschema.org/ontologies/american-football-statistics> . 
        
	spamfstat:passesInterceptionsAverage rdf:type rdf:Property ; 
        rdfs:label "passesInterceptionsAverage"@en ; 
        rdfs:comment "Average number of interceptions per game."@en ; 
        rdfs:domain [fill in] ; 
        rdfs:range xsd:integer ; 
        rdf:isDefinedBy <https://sportschema.org/ontologies/american-football-statistics> . 
        
	spamfstat:passesInterceptionsLongest rdf:type rdf:Property ; 
        rdfs:label "passesInterceptionsLongest"@en ; 
        rdfs:comment "Longest interception return against a passer."@en ; 
        rdfs:domain [fill in] ; 
        rdfs:range xsd:integer ; 
        rdf:isDefinedBy <https://sportschema.org/ontologies/american-football-statistics> . 
        
	spamfstat:passesInterceptionsTouchdown rdf:type rdf:Property ; 
        rdfs:label "passesInterceptionsTouchdown"@en ; 
        rdfs:comment "Number of opponents' touchdowns scored from passer's
                interceptions."@en ; 
        rdfs:domain [fill in] ; 
        rdfs:range xsd:integer ; 
        rdf:isDefinedBy <https://sportschema.org/ontologies/american-football-statistics> . 
        
	spamfstat:passesLongest rdf:type rdf:Property ; 
        rdfs:label "passesLongest"@en ; 
        rdfs:comment "The yards gained by the single longest
                completion."@en ; 
        rdfs:domain [fill in] ; 
        rdfs:range xsd:integer ; 
        rdf:isDefinedBy <https://sportschema.org/ontologies/american-football-statistics> . 
        
	spamfstat:passesAverageYardsPer rdf:type rdf:Property ; 
        rdfs:label "passesAverageYardsPer"@en ; 
        rdfs:comment "Gross passing yards divided by number of pass
                completions."@en ; 
        rdfs:domain [fill in] ; 
        rdfs:range xsd:integer ; 
        rdf:isDefinedBy <https://sportschema.org/ontologies/american-football-statistics> . 
        
	spamfstat:passesAverageYardsPerGame rdf:type rdf:Property ; 
        rdfs:label "passesAverageYardsPerGame"@en ; 
        rdfs:comment "Total yards passing divided by number of games
                played."@en ; 
        rdfs:domain [fill in] ; 
        rdfs:range xsd:integer ; 
        rdf:isDefinedBy <https://sportschema.org/ontologies/american-football-statistics> . 
        
	spamfstat:passerRating rdf:type rdf:Property ; 
        rdfs:label "passerRating"@en ; 
        rdfs:comment "A complex formula designed to measure quarterback
                performance."@en ; 
        rdfs:domain [fill in] ; 
        rdfs:range xsd:integer ; 
        rdf:isDefinedBy <https://sportschema.org/ontologies/american-football-statistics> . 
        
	spamfstat:receptionsTotal rdf:type rdf:Property ; 
        rdfs:label "receptionsTotal"@en ; 
        rdfs:comment "The total number of successful passes."@en ; 
        rdfs:domain [fill in] ; 
        rdfs:range xsd:integer ; 
        rdf:isDefinedBy <https://sportschema.org/ontologies/american-football-statistics> . 
        
	spamfstat:receptionsAveragePerGame rdf:type rdf:Property ; 
        rdfs:label "receptionsAveragePerGame"@en ; 
        rdfs:comment "Average number of receptions per game."@en ; 
        rdfs:domain [fill in] ; 
        rdfs:range xsd:integer ; 
        rdf:isDefinedBy <https://sportschema.org/ontologies/american-football-statistics> . 
        
	spamfstat:receptionsYards rdf:type rdf:Property ; 
        rdfs:label "receptionsYards"@en ; 
        rdfs:comment "Number of yards a receiver is credited for."@en ; 
        rdfs:domain [fill in] ; 
        rdfs:range xsd:integer ; 
        rdf:isDefinedBy <https://sportschema.org/ontologies/american-football-statistics> . 
        
	spamfstat:receptionsFirstDown rdf:type rdf:Property ; 
        rdfs:label "receptionsFirstDown"@en ; 
        rdfs:comment "Number of receptions a player has taken for a
                first-down."@en ; 
        rdfs:domain [fill in] ; 
        rdfs:range xsd:integer ; 
        rdf:isDefinedBy <https://sportschema.org/ontologies/american-football-statistics> . 
        
	spamfstat:receptionsLongest rdf:type rdf:Property ; 
        rdfs:label "receptionsLongest"@en ; 
        rdfs:comment "The longest reception a player had, including to the point
                where they scored, were-tackled, etc."@en ; 
        rdfs:domain [fill in] ; 
        rdfs:range xsd:integer ; 
        rdf:isDefinedBy <https://sportschema.org/ontologies/american-football-statistics> . 
        
	spamfstat:receptionsLooks rdf:type rdf:Property ; 
        rdfs:label "receptionsLooks"@en ; 
        rdfs:comment "The number of opportunities this receiver had to receive
                the ball."@en ; 
        rdfs:domain [fill in] ; 
        rdfs:range xsd:integer ; 
        rdf:isDefinedBy <https://sportschema.org/ontologies/american-football-statistics> . 
        
	spamfstat:receptionsAverageYards rdf:type rdf:Property ; 
        rdfs:label "receptionsAverageYards"@en ; 
        rdfs:comment "Average yards per game from receptions."@en ; 
        rdfs:domain [fill in] ; 
        rdfs:range xsd:integer ; 
        rdf:isDefinedBy <https://sportschema.org/ontologies/american-football-statistics> . 
        
	spamfstat:receptionsAverageYardsPer rdf:type rdf:Property ; 
        rdfs:label "receptionsAverageYardsPer"@en ; 
        rdfs:comment "The average yards per reception."@en ; 
        rdfs:domain [fill in] ; 
        rdfs:range xsd:integer ; 
        rdf:isDefinedBy <https://sportschema.org/ontologies/american-football-statistics> . 
        
	spamfstat:passingRank rdf:type rdf:Property ; 
        rdfs:label "passingRank"@en ; 
        rdfs:comment "How a player or team's passing stats ranks in a league or
                conference, usually using total passing yards as the measure."@en ; 
        rdfs:domain [fill in] ; 
        rdfs:range xsd:integer ; 
        rdf:isDefinedBy <https://sportschema.org/ontologies/american-football-statistics> . 
        
	spamfstat:timesThrownTotal rdf:type rdf:Property ; 
        rdfs:label "timesThrownTotal"@en ; 
        rdfs:comment "Number of passes directed at receiver, including
                incompletions, interceptions, etc."@en ; 
        rdfs:domain [fill in] ; 
        rdfs:range xsd:integer ; 
        rdf:isDefinedBy <https://sportschema.org/ontologies/american-football-statistics> . 
        
	spamfstat:receptionsCareer100YardGames rdf:type rdf:Property ; 
        rdfs:label "receptionsCareer100YardGames"@en ; 
        rdfs:comment "Number of times in receiver's career where total receiving
                yardage per game exceeded 100."@en ; 
        rdfs:domain [fill in] ; 
        rdfs:range xsd:integer ; 
        rdf:isDefinedBy <https://sportschema.org/ontologies/american-football-statistics> . 
        
	spamfstat:passingCareer300YardGames rdf:type rdf:Property ; 
        rdfs:label "passingCareer300YardGames"@en ; 
        rdfs:comment "Number of times in passer's career where total passing
                yardage per game exceeded 300."@en ; 
        rdfs:domain [fill in] ; 
        rdfs:range xsd:integer ; 
        rdf:isDefinedBy <https://sportschema.org/ontologies/american-football-statistics> . 
        
	spamfstat:rushesAttempts rdf:type rdf:Property ; 
        rdfs:label "rushesAttempts"@en ; 
        rdfs:comment "The number of attempted rushes."@en ; 
        rdfs:domain [fill in] ; 
        rdfs:range xsd:integer ; 
        rdf:isDefinedBy <https://sportschema.org/ontologies/american-football-statistics> . 
        
	spamfstat:rushesYards rdf:type rdf:Property ; 
        rdfs:label "rushesYards"@en ; 
        rdfs:comment "The number of yards gained by rushing."@en ; 
        rdfs:domain [fill in] ; 
        rdfs:range xsd:integer ; 
        rdf:isDefinedBy <https://sportschema.org/ontologies/american-football-statistics> . 
        
	spamfstat:rushesYardsLeft rdf:type rdf:Property ; 
        rdfs:label "rushesYardsLeft"@en ; 
        rdfs:comment "The number of yards gained by rushing up the left side of
                the field."@en ; 
        rdfs:domain [fill in] ; 
        rdfs:range xsd:integer ; 
        rdf:isDefinedBy <https://sportschema.org/ontologies/american-football-statistics> . 
        
	spamfstat:rushesYardsMiddle rdf:type rdf:Property ; 
        rdfs:label "rushesYardsMiddle"@en ; 
        rdfs:comment "The number of yards gained by rushing up the middle of the
                field."@en ; 
        rdfs:domain [fill in] ; 
        rdfs:range xsd:integer ; 
        rdf:isDefinedBy <https://sportschema.org/ontologies/american-football-statistics> . 
        
	spamfstat:rushesYardsRight rdf:type rdf:Property ; 
        rdfs:label "rushesYardsRight"@en ; 
        rdfs:comment "The number of yards gained by rushing up the right side of
                the field."@en ; 
        rdfs:domain [fill in] ; 
        rdfs:range xsd:integer ; 
        rdf:isDefinedBy <https://sportschema.org/ontologies/american-football-statistics> . 
        
	spamfstat:rushingAverageYardsPer rdf:type rdf:Property ; 
        rdfs:label "rushingAverageYardsPer"@en ; 
        rdfs:comment "The average number of yards per rush."@en ; 
        rdfs:domain [fill in] ; 
        rdfs:range xsd:integer ; 
        rdf:isDefinedBy <https://sportschema.org/ontologies/american-football-statistics> . 
        
	spamfstat:rushesFirstDown rdf:type rdf:Property ; 
        rdfs:label "rushesFirstDown"@en ; 
        rdfs:comment "The number of rushes that have resulted in a
                first-down."@en ; 
        rdfs:domain [fill in] ; 
        rdfs:range xsd:integer ; 
        rdf:isDefinedBy <https://sportschema.org/ontologies/american-football-statistics> . 
        
	spamfstat:rushesLongest rdf:type rdf:Property ; 
        rdfs:label "rushesLongest"@en ; 
        rdfs:comment "The number of yards gained by the single longest rushing
                play."@en ; 
        rdfs:domain [fill in] ; 
        rdfs:range xsd:integer ; 
        rdf:isDefinedBy <https://sportschema.org/ontologies/american-football-statistics> . 
        
	spamfstat:rushesAverageAttemptsPerGame rdf:type rdf:Property ; 
        rdfs:label "rushesAverageAttemptsPerGame"@en ; 
        rdfs:comment "Average number of rushing attempts per game."@en ; 
        rdfs:domain [fill in] ; 
        rdfs:range xsd:integer ; 
        rdf:isDefinedBy <https://sportschema.org/ontologies/american-football-statistics> . 
        
	spamfstat:rushesAverageYardsPerGame rdf:type rdf:Property ; 
        rdfs:label "rushesAverageYardsPerGame"@en ; 
        rdfs:comment "Average number of yards gaining from rushes a
                game."@en ; 
        rdfs:domain [fill in] ; 
        rdfs:range xsd:integer ; 
        rdf:isDefinedBy <https://sportschema.org/ontologies/american-football-statistics> . 
        
	spamfstat:rushingRank rdf:type rdf:Property ; 
        rdfs:label "rushingRank"@en ; 
        rdfs:comment "How a player or team's rushing stats ranks in a league or
                conference, usually using total rushing yards as the measure."@en ; 
        rdfs:domain [fill in] ; 
        rdfs:range xsd:integer ; 
        rdf:isDefinedBy <https://sportschema.org/ontologies/american-football-statistics> . 
        
	spamfstat:rushesCareer100YardGames rdf:type rdf:Property ; 
        rdfs:label "rushesCareer100YardGames"@en ; 
        rdfs:comment "Number of times in rusher's career where total rushing
                yardage per game exceeded 100."@en ; 
        rdfs:domain [fill in] ; 
        rdfs:range xsd:integer ; 
        rdf:isDefinedBy <https://sportschema.org/ontologies/american-football-statistics> . 
        
	spamfstat:firstDownsTotal rdf:type rdf:Property ; 
        rdfs:label "firstDownsTotal"@en ; 
        rdfs:comment "The number of first downs achieved."@en ; 
        rdfs:domain [fill in] ; 
        rdfs:range xsd:integer ; 
        rdf:isDefinedBy <https://sportschema.org/ontologies/american-football-statistics> . 
        
	spamfstat:firstDownsPass rdf:type rdf:Property ; 
        rdfs:label "firstDownsPass"@en ; 
        rdfs:comment "The number of first downs achieved from
                passing."@en ; 
        rdfs:domain [fill in] ; 
        rdfs:range xsd:integer ; 
        rdf:isDefinedBy <https://sportschema.org/ontologies/american-football-statistics> . 
        
	spamfstat:firstDownsRun rdf:type rdf:Property ; 
        rdfs:label "firstDownsRun"@en ; 
        rdfs:comment "The number of first downs achieved from
                rushing."@en ; 
        rdfs:domain [fill in] ; 
        rdfs:range xsd:integer ; 
        rdf:isDefinedBy <https://sportschema.org/ontologies/american-football-statistics> . 
        
	spamfstat:firstDownsPenalty rdf:type rdf:Property ; 
        rdfs:label "firstDownsPenalty"@en ; 
        rdfs:comment "The number of first downs achieved from penalties on the
                other team."@en ; 
        rdfs:domain [fill in] ; 
        rdfs:range xsd:integer ; 
        rdf:isDefinedBy <https://sportschema.org/ontologies/american-football-statistics> . 
        
	spamfstat:firstDownsYards rdf:type rdf:Property ; 
        rdfs:label "firstDownsYards"@en ; 
        rdfs:comment "Number of yards gained on first down plays."@en ; 
        rdfs:domain [fill in] ; 
        rdfs:range xsd:integer ; 
        rdf:isDefinedBy <https://sportschema.org/ontologies/american-football-statistics> . 
        
	spamfstat:firstDownsAverageYardsPer rdf:type rdf:Property ; 
        rdfs:label "firstDownsAverageYardsPer"@en ; 
        rdfs:comment "Number of average yards gained on first down
                plays."@en ; 
        rdfs:domain [fill in] ; 
        rdfs:range xsd:integer ; 
        rdf:isDefinedBy <https://sportschema.org/ontologies/american-football-statistics> . 
        
	spamfstat:conversionsSecondDown rdf:type rdf:Property ; 
        rdfs:label "conversionsSecondDown"@en ; 
        rdfs:comment "The number of first downs achieved on a second
                down."@en ; 
        rdfs:domain [fill in] ; 
        rdfs:range xsd:integer ; 
        rdf:isDefinedBy <https://sportschema.org/ontologies/american-football-statistics> . 
        
	spamfstat:conversionsSecondDownAttempts rdf:type rdf:Property ; 
        rdfs:label "conversionsSecondDownAttempts"@en ; 
        rdfs:comment "The number of second downs."@en ; 
        rdfs:domain [fill in] ; 
        rdfs:range xsd:integer ; 
        rdf:isDefinedBy <https://sportschema.org/ontologies/american-football-statistics> . 
        
	spamfstat:conversionsSecondDownPercentage rdf:type rdf:Property ; 
        rdfs:label "conversionsSecondDownPercentage"@en ; 
        rdfs:comment "The percentage of first down attempts on a second down that
                were successful."@en ; 
        rdfs:domain [fill in] ; 
        rdfs:range xsd:integer ; 
        rdf:isDefinedBy <https://sportschema.org/ontologies/american-football-statistics> . 
        
	spamfstat:conversionsThirdDown rdf:type rdf:Property ; 
        rdfs:label "conversionsThirdDown"@en ; 
        rdfs:comment "The number of first downs achieved on a third
                down."@en ; 
        rdfs:domain [fill in] ; 
        rdfs:range xsd:integer ; 
        rdf:isDefinedBy <https://sportschema.org/ontologies/american-football-statistics> . 
        
	spamfstat:conversionsThirdDownAttempts rdf:type rdf:Property ; 
        rdfs:label "conversionsThirdDownAttempts"@en ; 
        rdfs:comment "The number of third downs."@en ; 
        rdfs:domain [fill in] ; 
        rdfs:range xsd:integer ; 
        rdf:isDefinedBy <https://sportschema.org/ontologies/american-football-statistics> . 
        
	spamfstat:conversionsThirdDownPercentage rdf:type rdf:Property ; 
        rdfs:label "conversionsThirdDownPercentage"@en ; 
        rdfs:comment "The percentage of first down attempts on a third down that
                were successful."@en ; 
        rdfs:domain [fill in] ; 
        rdfs:range xsd:integer ; 
        rdf:isDefinedBy <https://sportschema.org/ontologies/american-football-statistics> . 
        
	spamfstat:conversionsFourthDown rdf:type rdf:Property ; 
        rdfs:label "conversionsFourthDown"@en ; 
        rdfs:comment "The number of first downs achieved on a fourth
                down."@en ; 
        rdfs:domain [fill in] ; 
        rdfs:range xsd:integer ; 
        rdf:isDefinedBy <https://sportschema.org/ontologies/american-football-statistics> . 
        
	spamfstat:conversionsFourthDownAttempts rdf:type rdf:Property ; 
        rdfs:label "conversionsFourthDownAttempts"@en ; 
        rdfs:comment "The number of fourth downs."@en ; 
        rdfs:domain [fill in] ; 
        rdfs:range xsd:integer ; 
        rdf:isDefinedBy <https://sportschema.org/ontologies/american-football-statistics> . 
        
	spamfstat:conversionsFourthDownPercentage rdf:type rdf:Property ; 
        rdfs:label "conversionsFourthDownPercentage"@en ; 
        rdfs:comment "The percentage of first down attempts on a fourth down that
                were successful."@en ; 
        rdfs:domain [fill in] ; 
        rdfs:range xsd:integer ; 
        rdf:isDefinedBy <https://sportschema.org/ontologies/american-football-statistics> . 
        
	spamfstat:sacksAgainstYards rdf:type rdf:Property ; 
        rdfs:label "sacksAgainstYards"@en ; 
        rdfs:comment "Total number of yards lost by the offense from
                sacks."@en ; 
        rdfs:domain [fill in] ; 
        rdfs:range xsd:integer ; 
        rdf:isDefinedBy <https://sportschema.org/ontologies/american-football-statistics> . 
        
	spamfstat:sacksAgainstTotal rdf:type rdf:Property ; 
        rdfs:label "sacksAgainstTotal"@en ; 
        rdfs:comment "Total number of times that the offense was
                sacked."@en ; 
        rdfs:domain [fill in] ; 
        rdfs:range xsd:integer ; 
        rdf:isDefinedBy <https://sportschema.org/ontologies/american-football-statistics> . 
        
	spamfstat:sacksAgainstAverage rdf:type rdf:Property ; 
        rdfs:label "sacksAgainstAverage"@en ; 
        rdfs:comment "Average number of times per game a quarterback is
                sacked."@en ; 
        rdfs:domain [fill in] ; 
        rdfs:range xsd:integer ; 
        rdf:isDefinedBy <https://sportschema.org/ontologies/american-football-statistics> . 
        
	spamfstat:sacksAgainstSafeties rdf:type rdf:Property ; 
        rdfs:label "sacksAgainstSafeties"@en ; 
        rdfs:comment "Number of sacks that resulted in safeties."@en ; 
        rdfs:domain [fill in] ; 
        rdfs:range xsd:integer ; 
        rdf:isDefinedBy <https://sportschema.org/ontologies/american-football-statistics> . 
        
	spamfstat:tacklesTotal rdf:type rdf:Property ; 
        rdfs:label "tacklesTotal"@en ; 
        rdfs:comment "The number of tackles made by the defense. Commonly the sum
                of tackles-solo and tackles-assists."@en ; 
        rdfs:domain [fill in] ; 
        rdfs:range xsd:integer ; 
        rdf:isDefinedBy <https://sportschema.org/ontologies/american-football-statistics> . 
        
	spamfstat:tacklesSolo rdf:type rdf:Property ; 
        rdfs:label "tacklesSolo"@en ; 
        rdfs:comment "The number of tackles made where only one member of the
                defense commited the tackle."@en ; 
        rdfs:domain [fill in] ; 
        rdfs:range xsd:integer ; 
        rdf:isDefinedBy <https://sportschema.org/ontologies/american-football-statistics> . 
        
	spamfstat:tacklesAssists rdf:type rdf:Property ; 
        rdfs:label "tacklesAssists"@en ; 
        rdfs:comment "The number of tackles made where multiple members of the
                defense commited the tackle."@en ; 
        rdfs:domain [fill in] ; 
        rdfs:range xsd:integer ; 
        rdf:isDefinedBy <https://sportschema.org/ontologies/american-football-statistics> . 
        
	spamfstat:tacklesTeam rdf:type rdf:Property ; 
        rdfs:label "tacklesTeam"@en ; 
        rdfs:comment "The number of tackles made which were credited to the team
                as a whole."@en ; 
        rdfs:domain [fill in] ; 
        rdfs:range xsd:integer ; 
        rdf:isDefinedBy <https://sportschema.org/ontologies/american-football-statistics> . 
        
	spamfstat:quarterbackHurries rdf:type rdf:Property ; 
        rdfs:label "quarterbackHurries"@en ; 
        rdfs:comment "An unofficial stat given when a defensive player pressures
                and hurries the quarterback into making a throw to avoid being sacked."@en ; 
        rdfs:domain [fill in] ; 
        rdfs:range xsd:integer ; 
        rdf:isDefinedBy <https://sportschema.org/ontologies/american-football-statistics> . 
        
	spamfstat:passesDefensed rdf:type rdf:Property ; 
        rdfs:label "passesDefensed"@en ; 
        rdfs:comment "Total number of times a pass was deflected or otherwise
                defended against, causing a pass to be incomplete."@en ; 
        rdfs:domain [fill in] ; 
        rdfs:range xsd:integer ; 
        rdf:isDefinedBy <https://sportschema.org/ontologies/american-football-statistics> . 
        
	spamfstat:turnoversTakeaway rdf:type rdf:Property ; 
        rdfs:label "turnoversTakeaway"@en ; 
        rdfs:comment "Derived by adding interceptions-total plus
                fumbles-opposing-recovered."@en ; 
        rdfs:domain [fill in] ; 
        rdfs:range xsd:integer ; 
        rdf:isDefinedBy <https://sportschema.org/ontologies/american-football-statistics> . 
        
	spamfstat:yardsAllowedTotal rdf:type rdf:Property ; 
        rdfs:label "yardsAllowedTotal"@en ; 
        rdfs:comment "Total yardage a defense allowed, usually through passing
                and rushing."@en ; 
        rdfs:domain [fill in] ; 
        rdfs:range xsd:integer ; 
        rdf:isDefinedBy <https://sportschema.org/ontologies/american-football-statistics> . 
        
	spamfstat:yardsAllowedAverage rdf:type rdf:Property ; 
        rdfs:label "yardsAllowedAverage"@en ; 
        rdfs:comment "Total yardage a defense allows per game."@en ; 
        rdfs:domain [fill in] ; 
        rdfs:range xsd:integer ; 
        rdf:isDefinedBy <https://sportschema.org/ontologies/american-football-statistics> . 
        
	spamfstat:defensivePlaysNumber rdf:type rdf:Property ; 
        rdfs:label "defensivePlaysNumber"@en ; 
        rdfs:comment "Number of plays a defense is on the field."@en ; 
        rdfs:domain [fill in] ; 
        rdfs:range xsd:integer ; 
        rdf:isDefinedBy <https://sportschema.org/ontologies/american-football-statistics> . 
        
	spamfstat:inside20Plays rdf:type rdf:Property ; 
        rdfs:label "inside20Plays"@en ; 
        rdfs:comment "Number of plays inside defensive team's 20 yard
                line."@en ; 
        rdfs:domain [fill in] ; 
        rdfs:range xsd:integer ; 
        rdf:isDefinedBy <https://sportschema.org/ontologies/american-football-statistics> . 
        
	spamfstat:inside20PointsAgainst rdf:type rdf:Property ; 
        rdfs:label "inside20PointsAgainst"@en ; 
        rdfs:comment "Number of points given up when opponents' possession starts
                inside defensive team's 20 yard line."@en ; 
        rdfs:domain [fill in] ; 
        rdfs:range xsd:integer ; 
        rdf:isDefinedBy <https://sportschema.org/ontologies/american-football-statistics> . 
        
	spamfstat:inside20TouchdownsAgainst rdf:type rdf:Property ; 
        rdfs:label "inside20TouchdownsAgainst"@en ; 
        rdfs:comment "Number of touchdowns given up when opponents' possession
                starts inside defensive team's 20 yard line."@en ; 
        rdfs:domain [fill in] ; 
        rdfs:range xsd:integer ; 
        rdf:isDefinedBy <https://sportschema.org/ontologies/american-football-statistics> . 
        
	spamfstat:inside20TouchdownsAgainstPercentage rdf:type rdf:Property ; 
        rdfs:label "inside20TouchdownsAgainstPercentage"@en ; 
        rdfs:comment "Ratio of touchdowns allowed to possessions when opponents'
                possession starts inside defensive team's 20 yard line."@en ; 
        rdfs:domain [fill in] ; 
        rdfs:range xsd:integer ; 
        rdf:isDefinedBy <https://sportschema.org/ontologies/american-football-statistics> . 
        
	spamfstat:defenseRank rdf:type rdf:Property ; 
        rdfs:label "defenseRank"@en ; 
        rdfs:comment "How a team's defensive stats rank in a league or
                conference, usually using yards allowed per game as the measure."@en ; 
        rdfs:domain [fill in] ; 
        rdfs:range xsd:integer ; 
        rdf:isDefinedBy <https://sportschema.org/ontologies/american-football-statistics> . 
        
	spamfstat:defenseRankPass rdf:type rdf:Property ; 
        rdfs:label "defenseRankPass"@en ; 
        rdfs:comment "How a team's passing defense stats rank in a league or
                conference, usually using passing yards allowed per game as the
                measure."@en ; 
        rdfs:domain [fill in] ; 
        rdfs:range xsd:integer ; 
        rdf:isDefinedBy <https://sportschema.org/ontologies/american-football-statistics> . 
        
	spamfstat:defenseRankRush rdf:type rdf:Property ; 
        rdfs:label "defenseRankRush"@en ; 
        rdfs:comment "How a team's rushing defense stats rank in a league or
                conference, usually using rushing yards allowed per game as the
                measure."@en ; 
        rdfs:domain [fill in] ; 
        rdfs:range xsd:integer ; 
        rdf:isDefinedBy <https://sportschema.org/ontologies/american-football-statistics> . 
        
	spamfstat:interceptionsTotal rdf:type rdf:Property ; 
        rdfs:label "interceptionsTotal"@en ; 
        rdfs:comment "The number of passes the defense has
                intercepted."@en ; 
        rdfs:domain [fill in] ; 
        rdfs:range xsd:integer ; 
        rdf:isDefinedBy <https://sportschema.org/ontologies/american-football-statistics> . 
        
	spamfstat:interceptionsYards rdf:type rdf:Property ; 
        rdfs:label "interceptionsYards"@en ; 
        rdfs:comment "The number of yards gained as a result of an
                interception."@en ; 
        rdfs:domain [fill in] ; 
        rdfs:range xsd:integer ; 
        rdf:isDefinedBy <https://sportschema.org/ontologies/american-football-statistics> . 
        
	spamfstat:interceptionsAverage rdf:type rdf:Property ; 
        rdfs:label "interceptionsAverage"@en ; 
        rdfs:comment "The average number of yards gained from
                interceptions."@en ; 
        rdfs:domain [fill in] ; 
        rdfs:range xsd:integer ; 
        rdf:isDefinedBy <https://sportschema.org/ontologies/american-football-statistics> . 
        
	spamfstat:interceptionsPercentage rdf:type rdf:Property ; 
        rdfs:label "interceptionsPercentage"@en ; 
        rdfs:comment "Percentage of passes intercepted."@en ; 
        rdfs:domain [fill in] ; 
        rdfs:range xsd:integer ; 
        rdf:isDefinedBy <https://sportschema.org/ontologies/american-football-statistics> . 
        
	spamfstat:interceptionsLongest rdf:type rdf:Property ; 
        rdfs:label "interceptionsLongest"@en ; 
        rdfs:comment "The longest interception returned. Greatest number of yards
                gained on an interception."@en ; 
        rdfs:domain [fill in] ; 
        rdfs:range xsd:integer ; 
        rdf:isDefinedBy <https://sportschema.org/ontologies/american-football-statistics> . 
        
	spamfstat:interceptionsTouchdown rdf:type rdf:Property ; 
        rdfs:label "interceptionsTouchdown"@en ; 
        rdfs:comment "Number of interceptions that were run back for a
                touchdown."@en ; 
        rdfs:domain [fill in] ; 
        rdfs:range xsd:integer ; 
        rdf:isDefinedBy <https://sportschema.org/ontologies/american-football-statistics> . 
        
	spamfstat:sacksTotal rdf:type rdf:Property ; 
        rdfs:label "sacksTotal"@en ; 
        rdfs:comment "The number of sacks made by the defense."@en ; 
        rdfs:domain [fill in] ; 
        rdfs:range xsd:integer ; 
        rdf:isDefinedBy <https://sportschema.org/ontologies/american-football-statistics> . 
        
	spamfstat:sacksYards rdf:type rdf:Property ; 
        rdfs:label "sacksYards"@en ; 
        rdfs:comment "Number of yards gained by the defense."@en ; 
        rdfs:domain [fill in] ; 
        rdfs:range xsd:integer ; 
        rdf:isDefinedBy <https://sportschema.org/ontologies/american-football-statistics> . 
        
	spamfstat:sacksTeam rdf:type rdf:Property ; 
        rdfs:label "sacksTeam"@en ; 
        rdfs:comment "The number of sacks credited to the team as a
                whole."@en ; 
        rdfs:domain [fill in] ; 
        rdfs:range xsd:integer ; 
        rdf:isDefinedBy <https://sportschema.org/ontologies/american-football-statistics> . 
        
	spamfstat:sacksYardsTeam rdf:type rdf:Property ; 
        rdfs:label "sacksYardsTeam"@en ; 
        rdfs:comment "Number of yards gained by the defense on sacks credited to
                the team as a whole."@en ; 
        rdfs:domain [fill in] ; 
        rdfs:range xsd:integer ; 
        rdf:isDefinedBy <https://sportschema.org/ontologies/american-football-statistics> . 
        
	spamfstat:touchdownsTotal rdf:type rdf:Property ; 
        rdfs:label "touchdownsTotal"@en ; 
        rdfs:comment "The number of touchdowns scored by the
                offense."@en ; 
        rdfs:domain [fill in] ; 
        rdfs:range xsd:integer ; 
        rdf:isDefinedBy <https://sportschema.org/ontologies/american-football-statistics> . 
        
	spamfstat:touchdownsPassing rdf:type rdf:Property ; 
        rdfs:label "touchdownsPassing"@en ; 
        rdfs:comment "The number of touchdowns scored by passing."@en ; 
        rdfs:domain [fill in] ; 
        rdfs:range xsd:integer ; 
        rdf:isDefinedBy <https://sportschema.org/ontologies/american-football-statistics> . 
        
	spamfstat:touchdownsRushing rdf:type rdf:Property ; 
        rdfs:label "touchdownsRushing"@en ; 
        rdfs:comment "The number of touchdowns scored by rushing."@en ; 
        rdfs:domain [fill in] ; 
        rdfs:range xsd:integer ; 
        rdf:isDefinedBy <https://sportschema.org/ontologies/american-football-statistics> . 
        
	spamfstat:touchdownsSpecialTeams rdf:type rdf:Property ; 
        rdfs:label "touchdownsSpecialTeams"@en ; 
        rdfs:comment "The number of touchdowns scored by special
                teams."@en ; 
        rdfs:domain [fill in] ; 
        rdfs:range xsd:integer ; 
        rdf:isDefinedBy <https://sportschema.org/ontologies/american-football-statistics> . 
        
	spamfstat:touchdownsDefensive rdf:type rdf:Property ; 
        rdfs:label "touchdownsDefensive"@en ; 
        rdfs:comment "The number of touchdowns scored by the
                defense."@en ; 
        rdfs:domain [fill in] ; 
        rdfs:range xsd:integer ; 
        rdf:isDefinedBy <https://sportschema.org/ontologies/american-football-statistics> . 
        
	spamfstat:touchdownsReceptions rdf:type rdf:Property ; 
        rdfs:label "touchdownsReceptions"@en ; 
        rdfs:comment "The number of receptions resulting in a
                touchdown."@en ; 
        rdfs:domain [fill in] ; 
        rdfs:range xsd:integer ; 
        rdf:isDefinedBy <https://sportschema.org/ontologies/american-football-statistics> . 
        
	spamfstat:extraPointsAttempts rdf:type rdf:Property ; 
        rdfs:label "extraPointsAttempts"@en ; 
        rdfs:comment "The number of extra points attempted by the
                offense."@en ; 
        rdfs:domain [fill in] ; 
        rdfs:range xsd:integer ; 
        rdf:isDefinedBy <https://sportschema.org/ontologies/american-football-statistics> . 
        
	spamfstat:extraPointsMade rdf:type rdf:Property ; 
        rdfs:label "extraPointsMade"@en ; 
        rdfs:comment "The number of extra points made."@en ; 
        rdfs:domain [fill in] ; 
        rdfs:range xsd:integer ; 
        rdf:isDefinedBy <https://sportschema.org/ontologies/american-football-statistics> . 
        
	spamfstat:extraPointsMissed rdf:type rdf:Property ; 
        rdfs:label "extraPointsMissed"@en ; 
        rdfs:comment "The number of extra points missed."@en ; 
        rdfs:domain [fill in] ; 
        rdfs:range xsd:integer ; 
        rdf:isDefinedBy <https://sportschema.org/ontologies/american-football-statistics> . 
        
	spamfstat:extraPointsBlocked rdf:type rdf:Property ; 
        rdfs:label "extraPointsBlocked"@en ; 
        rdfs:comment "The number of extra point attempts that were
                blocked."@en ; 
        rdfs:domain [fill in] ; 
        rdfs:range xsd:integer ; 
        rdf:isDefinedBy <https://sportschema.org/ontologies/american-football-statistics> . 
        
	spamfstat:extraPointsPercentage rdf:type rdf:Property ; 
        rdfs:label "extraPointsPercentage"@en ; 
        rdfs:comment "Ratio of extra points completed to attempts."@en ; 
        rdfs:domain [fill in] ; 
        rdfs:range xsd:integer ; 
        rdf:isDefinedBy <https://sportschema.org/ontologies/american-football-statistics> . 
        
	spamfstat:fieldGoalAttempts rdf:type rdf:Property ; 
        rdfs:label "fieldGoalAttempts"@en ; 
        rdfs:comment "The number of field goals attempted."@en ; 
        rdfs:domain [fill in] ; 
        rdfs:range xsd:integer ; 
        rdf:isDefinedBy <https://sportschema.org/ontologies/american-football-statistics> . 
        
	spamfstat:fieldGoalsMade rdf:type rdf:Property ; 
        rdfs:label "fieldGoalsMade"@en ; 
        rdfs:comment "The number of field goals made."@en ; 
        rdfs:domain [fill in] ; 
        rdfs:range xsd:integer ; 
        rdf:isDefinedBy <https://sportschema.org/ontologies/american-football-statistics> . 
        
	spamfstat:fieldGoalsMissed rdf:type rdf:Property ; 
        rdfs:label "fieldGoalsMissed"@en ; 
        rdfs:comment "The number of field goals missed."@en ; 
        rdfs:domain [fill in] ; 
        rdfs:range xsd:integer ; 
        rdf:isDefinedBy <https://sportschema.org/ontologies/american-football-statistics> . 
        
	spamfstat:fieldGoalsBlocked rdf:type rdf:Property ; 
        rdfs:label "fieldGoalsBlocked"@en ; 
        rdfs:comment "The number of field goal attempts that were
                blocked."@en ; 
        rdfs:domain [fill in] ; 
        rdfs:range xsd:integer ; 
        rdf:isDefinedBy <https://sportschema.org/ontologies/american-football-statistics> . 
        
	spamfstat:fieldGoalLongest rdf:type rdf:Property ; 
        rdfs:label "fieldGoalLongest"@en ; 
        rdfs:comment "Yardage of longest successful field goal
                attempt."@en ; 
        rdfs:domain [fill in] ; 
        rdfs:range xsd:integer ; 
        rdf:isDefinedBy <https://sportschema.org/ontologies/american-football-statistics> . 
        
	spamfstat:fieldGoalsPercentage rdf:type rdf:Property ; 
        rdfs:label "fieldGoalsPercentage"@en ; 
        rdfs:comment "Ratio of field goals made to attempts."@en ; 
        rdfs:domain [fill in] ; 
        rdfs:range xsd:integer ; 
        rdf:isDefinedBy <https://sportschema.org/ontologies/american-football-statistics> . 
        
	spamfstat:fieldGoalsAverage rdf:type rdf:Property ; 
        rdfs:label "fieldGoalsAverage"@en ; 
        rdfs:comment "Average number of field goals made per game."@en ; 
        rdfs:domain [fill in] ; 
        rdfs:range xsd:integer ; 
        rdf:isDefinedBy <https://sportschema.org/ontologies/american-football-statistics> . 
        
	spamfstat:safetiesAgainst rdf:type rdf:Property ; 
        rdfs:label "safetiesAgainst"@en ; 
        rdfs:comment "The number of safeties scored against the
                offense."@en ; 
        rdfs:domain [fill in] ; 
        rdfs:range xsd:integer ; 
        rdf:isDefinedBy <https://sportschema.org/ontologies/american-football-statistics> . 
        
	spamfstat:twoPointConversionsAttempts rdf:type rdf:Property ; 
        rdfs:label "twoPointConversionsAttempts"@en ; 
        rdfs:comment "The number of two point conversions attempted."@en ; 
        rdfs:domain [fill in] ; 
        rdfs:range xsd:integer ; 
        rdf:isDefinedBy <https://sportschema.org/ontologies/american-football-statistics> . 
        
	spamfstat:twoPointConversionsMade rdf:type rdf:Property ; 
        rdfs:label "twoPointConversionsMade"@en ; 
        rdfs:comment "The number of successful two point
                conversions."@en ; 
        rdfs:domain [fill in] ; 
        rdfs:range xsd:integer ; 
        rdf:isDefinedBy <https://sportschema.org/ontologies/american-football-statistics> . 
        
	spamfstat:twoPointConversionsMadeRushing rdf:type rdf:Property ; 
        rdfs:label "twoPointConversionsMadeRushing"@en ; 
        rdfs:comment "Number of successful two-point conversions from running
                plays."@en ; 
        rdfs:domain [fill in] ; 
        rdfs:range xsd:integer ; 
        rdf:isDefinedBy <https://sportschema.org/ontologies/american-football-statistics> . 
        
	spamfstat:twoPointConversionsMadePassing rdf:type rdf:Property ; 
        rdfs:label "twoPointConversionsMadePassing"@en ; 
        rdfs:comment "Number of successful two-point conversions from passing
                plays."@en ; 
        rdfs:domain [fill in] ; 
        rdfs:range xsd:integer ; 
        rdf:isDefinedBy <https://sportschema.org/ontologies/american-football-statistics> . 
        
	spamfstat:touchbacks rdf:type rdf:Property ; 
        rdfs:label "touchbacks"@en ; 
        rdfs:comment "For Canadian Football. Used to record the number of
                touchbacks that resulted in scores."@en ; 
        rdfs:domain [fill in] ; 
        rdfs:range xsd:integer ; 
        rdf:isDefinedBy <https://sportschema.org/ontologies/american-football-statistics> . 
        
	spamfstat:singlePoints rdf:type rdf:Property ; 
        rdfs:label "singlePoints"@en ; 
        rdfs:comment "Number of points earned from the single, a CFL-specific
                scoring play where a kicking team prevents its opponent from returning a kickoff,
                punt or missed field goal from outside the opponent's own end zone."@en ; 
        rdfs:domain [fill in] ; 
        rdfs:range xsd:integer ; 
        rdf:isDefinedBy <https://sportschema.org/ontologies/american-football-statistics> . 
        
	spamfstat:inside20Points rdf:type rdf:Property ; 
        rdfs:label "inside20Points"@en ; 
        rdfs:comment "Points earned by offensive team when possession starts
                inside opponent's 20 yard line."@en ; 
        rdfs:domain [fill in] ; 
        rdfs:range xsd:integer ; 
        rdf:isDefinedBy <https://sportschema.org/ontologies/american-football-statistics> . 
        
	spamfstat:inside20Touchdowns rdf:type rdf:Property ; 
        rdfs:label "inside20Touchdowns"@en ; 
        rdfs:comment "Touchdowns scored by offensive team when possession starts
                inside opponent's 20 yard line."@en ; 
        rdfs:domain [fill in] ; 
        rdfs:range xsd:integer ; 
        rdf:isDefinedBy <https://sportschema.org/ontologies/american-football-statistics> . 
        
	spamfstat:inside20TouchdownsPercentage rdf:type rdf:Property ; 
        rdfs:label "inside20TouchdownsPercentage"@en ; 
        rdfs:comment "Ratio of touchdowns to possessions when possession starts
                inside opponent's 20 yard line."@en ; 
        rdfs:domain [fill in] ; 
        rdfs:range xsd:integer ; 
        rdf:isDefinedBy <https://sportschema.org/ontologies/american-football-statistics> . 
        
	spamfstat:returnsPuntTotal rdf:type rdf:Property ; 
        rdfs:label "returnsPuntTotal"@en ; 
        rdfs:comment "The number of punts returned."@en ; 
        rdfs:domain [fill in] ; 
        rdfs:range xsd:integer ; 
        rdf:isDefinedBy <https://sportschema.org/ontologies/american-football-statistics> . 
        
	spamfstat:returnsPuntYards rdf:type rdf:Property ; 
        rdfs:label "returnsPuntYards"@en ; 
        rdfs:comment "The number of yards gained from punt returns."@en ; 
        rdfs:domain [fill in] ; 
        rdfs:range xsd:integer ; 
        rdf:isDefinedBy <https://sportschema.org/ontologies/american-football-statistics> . 
        
	spamfstat:returnsPuntAverage rdf:type rdf:Property ; 
        rdfs:label "returnsPuntAverage"@en ; 
        rdfs:comment "The average number of yards gained on each punt
                return."@en ; 
        rdfs:domain [fill in] ; 
        rdfs:range xsd:integer ; 
        rdf:isDefinedBy <https://sportschema.org/ontologies/american-football-statistics> . 
        
	spamfstat:returnsPuntLongest rdf:type rdf:Property ; 
        rdfs:label "returnsPuntLongest"@en ; 
        rdfs:comment "The number of yards gained on the longest punt
                return."@en ; 
        rdfs:domain [fill in] ; 
        rdfs:range xsd:integer ; 
        rdf:isDefinedBy <https://sportschema.org/ontologies/american-football-statistics> . 
        
	spamfstat:returnsPuntTouchdown rdf:type rdf:Property ; 
        rdfs:label "returnsPuntTouchdown"@en ; 
        rdfs:comment "The number of punts returned for a touchdown."@en ; 
        rdfs:domain [fill in] ; 
        rdfs:range xsd:integer ; 
        rdf:isDefinedBy <https://sportschema.org/ontologies/american-football-statistics> . 
        
	spamfstat:returnsPuntAgainstTotal rdf:type rdf:Property ; 
        rdfs:label "returnsPuntAgainstTotal"@en ; 
        rdfs:comment "Total number of punt returns defended."@en ; 
        rdfs:domain [fill in] ; 
        rdfs:range xsd:integer ; 
        rdf:isDefinedBy <https://sportschema.org/ontologies/american-football-statistics> . 
        
	spamfstat:returnsPuntAgainstYards rdf:type rdf:Property ; 
        rdfs:label "returnsPuntAgainstYards"@en ; 
        rdfs:comment "Total number of yards allowed from punt
                returns."@en ; 
        rdfs:domain [fill in] ; 
        rdfs:range xsd:integer ; 
        rdf:isDefinedBy <https://sportschema.org/ontologies/american-football-statistics> . 
        
	spamfstat:returnsPuntAgainstAverage rdf:type rdf:Property ; 
        rdfs:label "returnsPuntAgainstAverage"@en ; 
        rdfs:comment "Average number of yards allowed from punt
                returns."@en ; 
        rdfs:domain [fill in] ; 
        rdfs:range xsd:integer ; 
        rdf:isDefinedBy <https://sportschema.org/ontologies/american-football-statistics> . 
        
	spamfstat:returnsPuntAgainstLongest rdf:type rdf:Property ; 
        rdfs:label "returnsPuntAgainstLongest"@en ; 
        rdfs:comment "Yardage of longest punt return allowed."@en ; 
        rdfs:domain [fill in] ; 
        rdfs:range xsd:integer ; 
        rdf:isDefinedBy <https://sportschema.org/ontologies/american-football-statistics> . 
        
	spamfstat:returnsPuntAgainstTouchdown rdf:type rdf:Property ; 
        rdfs:label "returnsPuntAgainstTouchdown"@en ; 
        rdfs:comment "Number of touchdowns from punt returns
                allowed."@en ; 
        rdfs:domain [fill in] ; 
        rdfs:range xsd:integer ; 
        rdf:isDefinedBy <https://sportschema.org/ontologies/american-football-statistics> . 
        
	spamfstat:kickoffsTotal rdf:type rdf:Property ; 
        rdfs:label "kickoffsTotal"@en ; 
        rdfs:comment "Total number of kickoffs to opposition."@en ; 
        rdfs:domain [fill in] ; 
        rdfs:range xsd:integer ; 
        rdf:isDefinedBy <https://sportschema.org/ontologies/american-football-statistics> . 
        
	spamfstat:kickoffsAdjusted rdf:type rdf:Property ; 
        rdfs:label "kickoffsAdjusted"@en ; 
        rdfs:comment "Number of kickoffs excluding onside kicks or kickoffs at
                the end of a half unless either kickoff is returned for a touchdown."@en ; 
        rdfs:domain [fill in] ; 
        rdfs:range xsd:integer ; 
        rdf:isDefinedBy <https://sportschema.org/ontologies/american-football-statistics> . 
        
	spamfstat:kickoffsToInside20 rdf:type rdf:Property ; 
        rdfs:label "kickoffsToInside20"@en ; 
        rdfs:comment "Number of kickoffs resulting in opponent's possession
                starting inside own 20 yard line."@en ; 
        rdfs:domain [fill in] ; 
        rdfs:range xsd:integer ; 
        rdf:isDefinedBy <https://sportschema.org/ontologies/american-football-statistics> . 
        
	spamfstat:kickoffsDriveStartAgainstAverage rdf:type rdf:Property ; 
        rdfs:label "kickoffsDriveStartAgainstAverage"@en ; 
        rdfs:comment "Average starting position of opponent's possession after a
                kickoff."@en ; 
        rdfs:domain [fill in] ; 
        rdfs:range xsd:integer ; 
        rdf:isDefinedBy <https://sportschema.org/ontologies/american-football-statistics> . 
        
	spamfstat:onsideKicksAttempted rdf:type rdf:Property ; 
        rdfs:label "onsideKicksAttempted"@en ; 
        rdfs:comment "Number of onside kicks attempted."@en ; 
        rdfs:domain [fill in] ; 
        rdfs:range xsd:integer ; 
        rdf:isDefinedBy <https://sportschema.org/ontologies/american-football-statistics> . 
        
	spamfstat:onsideKicksRecovered rdf:type rdf:Property ; 
        rdfs:label "onsideKicksRecovered"@en ; 
        rdfs:comment "Number of onside kicks recovered by kicking
                team."@en ; 
        rdfs:domain [fill in] ; 
        rdfs:range xsd:integer ; 
        rdf:isDefinedBy <https://sportschema.org/ontologies/american-football-statistics> . 
        
	spamfstat:returnsKickoffTotal rdf:type rdf:Property ; 
        rdfs:label "returnsKickoffTotal"@en ; 
        rdfs:comment "The number of kickoffs returned."@en ; 
        rdfs:domain [fill in] ; 
        rdfs:range xsd:integer ; 
        rdf:isDefinedBy <https://sportschema.org/ontologies/american-football-statistics> . 
        
	spamfstat:returnsKickoffYards rdf:type rdf:Property ; 
        rdfs:label "returnsKickoffYards"@en ; 
        rdfs:comment "The number of yards gained from kickoff
                returns."@en ; 
        rdfs:domain [fill in] ; 
        rdfs:range xsd:integer ; 
        rdf:isDefinedBy <https://sportschema.org/ontologies/american-football-statistics> . 
        
	spamfstat:returnsKickoffAverage rdf:type rdf:Property ; 
        rdfs:label "returnsKickoffAverage"@en ; 
        rdfs:comment "The average number of yards gained on each kickoff
                return."@en ; 
        rdfs:domain [fill in] ; 
        rdfs:range xsd:integer ; 
        rdf:isDefinedBy <https://sportschema.org/ontologies/american-football-statistics> . 
        
	spamfstat:returnsKickoffLongest rdf:type rdf:Property ; 
        rdfs:label "returnsKickoffLongest"@en ; 
        rdfs:comment "The number of yards gained on the longest kickoff
                return."@en ; 
        rdfs:domain [fill in] ; 
        rdfs:range xsd:integer ; 
        rdf:isDefinedBy <https://sportschema.org/ontologies/american-football-statistics> . 
        
	spamfstat:returnsKickoffTouchdown rdf:type rdf:Property ; 
        rdfs:label "returnsKickoffTouchdown"@en ; 
        rdfs:comment "The number of kickoffs returned for a
                touchdown."@en ; 
        rdfs:domain [fill in] ; 
        rdfs:range xsd:integer ; 
        rdf:isDefinedBy <https://sportschema.org/ontologies/american-football-statistics> . 
        
	spamfstat:returnsKickoffAdjusted rdf:type rdf:Property ; 
        rdfs:label "returnsKickoffAdjusted"@en ; 
        rdfs:comment "Number kickoffs adjusted for onside and end-of-half
                (non-touchdown) kickoffs."@en ; 
        rdfs:domain [fill in] ; 
        rdfs:range xsd:integer ; 
        rdf:isDefinedBy <https://sportschema.org/ontologies/american-football-statistics> . 
        
	spamfstat:returnsKickoffInside20 rdf:type rdf:Property ; 
        rdfs:label "returnsKickoffInside20"@en ; 
        rdfs:comment "Number of kickoff returns that failed to advance past the
                returning team's 20 yard line."@en ; 
        rdfs:domain [fill in] ; 
        rdfs:range xsd:integer ; 
        rdf:isDefinedBy <https://sportschema.org/ontologies/american-football-statistics> . 
        
	spamfstat:returnsKickoffDriveStartAverage rdf:type rdf:Property ; 
        rdfs:label "returnsKickoffDriveStartAverage"@en ; 
        rdfs:comment "Average start position after kickoff returns."@en ; 
        rdfs:domain [fill in] ; 
        rdfs:range xsd:integer ; 
        rdf:isDefinedBy <https://sportschema.org/ontologies/american-football-statistics> . 
        
	spamfstat:returnsKickoffAgainstTotal rdf:type rdf:Property ; 
        rdfs:label "returnsKickoffAgainstTotal"@en ; 
        rdfs:comment "Total number of kickoff returns."@en ; 
        rdfs:domain [fill in] ; 
        rdfs:range xsd:integer ; 
        rdf:isDefinedBy <https://sportschema.org/ontologies/american-football-statistics> . 
        
	spamfstat:returnsKickoffAgainstYards rdf:type rdf:Property ; 
        rdfs:label "returnsKickoffAgainstYards"@en ; 
        rdfs:comment "Yards allowed from kickoff returns."@en ; 
        rdfs:domain [fill in] ; 
        rdfs:range xsd:integer ; 
        rdf:isDefinedBy <https://sportschema.org/ontologies/american-football-statistics> . 
        
	spamfstat:returnsKickoffAgainstAverage rdf:type rdf:Property ; 
        rdfs:label "returnsKickoffAgainstAverage"@en ; 
        rdfs:comment "Average yards allowed per kickoff return."@en ; 
        rdfs:domain [fill in] ; 
        rdfs:range xsd:integer ; 
        rdf:isDefinedBy <https://sportschema.org/ontologies/american-football-statistics> . 
        
	spamfstat:returnsKickoffAgainstLongest rdf:type rdf:Property ; 
        rdfs:label "returnsKickoffAgainstLongest"@en ; 
        rdfs:comment "Yardage of longest kickoff return allowed."@en ; 
        rdfs:domain [fill in] ; 
        rdfs:range xsd:integer ; 
        rdf:isDefinedBy <https://sportschema.org/ontologies/american-football-statistics> . 
        
	spamfstat:returnsKickoffAgainstTouchdown rdf:type rdf:Property ; 
        rdfs:label "returnsKickoffAgainstTouchdown"@en ; 
        rdfs:comment "Touchdowns allowed from kickoff returns."@en ; 
        rdfs:domain [fill in] ; 
        rdfs:range xsd:integer ; 
        rdf:isDefinedBy <https://sportschema.org/ontologies/american-football-statistics> . 
        
	spamfstat:returnsTotal rdf:type rdf:Property ; 
        rdfs:label "returnsTotal"@en ; 
        rdfs:comment "The total number of returns. Punts + kickoffs."@en ; 
        rdfs:domain [fill in] ; 
        rdfs:range xsd:integer ; 
        rdf:isDefinedBy <https://sportschema.org/ontologies/american-football-statistics> . 
        
	spamfstat:returnsYards rdf:type rdf:Property ; 
        rdfs:label "returnsYards"@en ; 
        rdfs:comment "The total number of yards gained on punts and kickoffs
                combined."@en ; 
        rdfs:domain [fill in] ; 
        rdfs:range xsd:integer ; 
        rdf:isDefinedBy <https://sportschema.org/ontologies/american-football-statistics> . 
        
	spamfstat:puntsTotal rdf:type rdf:Property ; 
        rdfs:label "puntsTotal"@en ; 
        rdfs:comment "The number of punts."@en ; 
        rdfs:domain [fill in] ; 
        rdfs:range xsd:integer ; 
        rdf:isDefinedBy <https://sportschema.org/ontologies/american-football-statistics> . 
        
	spamfstat:puntsYardsGross rdf:type rdf:Property ; 
        rdfs:label "puntsYardsGross"@en ; 
        rdfs:comment "The sum of the distances of all punts."@en ; 
        rdfs:domain [fill in] ; 
        rdfs:range xsd:integer ; 
        rdf:isDefinedBy <https://sportschema.org/ontologies/american-football-statistics> . 
        
	spamfstat:puntsYardsNet rdf:type rdf:Property ; 
        rdfs:label "puntsYardsNet"@en ; 
        rdfs:comment "The sum of the distances of all punts, minus the distances
                they were returned."@en ; 
        rdfs:domain [fill in] ; 
        rdfs:range xsd:integer ; 
        rdf:isDefinedBy <https://sportschema.org/ontologies/american-football-statistics> . 
        
	spamfstat:puntsLongest rdf:type rdf:Property ; 
        rdfs:label "puntsLongest"@en ; 
        rdfs:comment "The distance of the longest punt."@en ; 
        rdfs:domain [fill in] ; 
        rdfs:range xsd:integer ; 
        rdf:isDefinedBy <https://sportschema.org/ontologies/american-football-statistics> . 
        
	spamfstat:puntsInside20 rdf:type rdf:Property ; 
        rdfs:label "puntsInside20"@en ; 
        rdfs:comment "The number of punts inside the 20 yard line."@en ; 
        rdfs:domain [fill in] ; 
        rdfs:range xsd:integer ; 
        rdf:isDefinedBy <https://sportschema.org/ontologies/american-football-statistics> . 
        
	spamfstat:puntsInside20Percentage rdf:type rdf:Property ; 
        rdfs:label "puntsInside20Percentage"@en ; 
        rdfs:comment "The percentage of punts inside the 20 yard
                line."@en ; 
        rdfs:domain [fill in] ; 
        rdfs:range xsd:integer ; 
        rdf:isDefinedBy <https://sportschema.org/ontologies/american-football-statistics> . 
        
	spamfstat:puntsAverage rdf:type rdf:Property ; 
        rdfs:label "puntsAverage"@en ; 
        rdfs:comment "The average gross punting yardage."@en ; 
        rdfs:domain [fill in] ; 
        rdfs:range xsd:integer ; 
        rdf:isDefinedBy <https://sportschema.org/ontologies/american-football-statistics> . 
        
	spamfstat:puntsAverageNet rdf:type rdf:Property ; 
        rdfs:label "puntsAverageNet"@en ; 
        rdfs:comment "Average net yards - punt length minus return - per
                punt."@en ; 
        rdfs:domain [fill in] ; 
        rdfs:range xsd:integer ; 
        rdf:isDefinedBy <https://sportschema.org/ontologies/american-football-statistics> . 
        
	spamfstat:puntsAgainstTotal rdf:type rdf:Property ; 
        rdfs:label "puntsAgainstTotal"@en ; 
        rdfs:comment "Number of punts forced by defensive team."@en ; 
        rdfs:domain [fill in] ; 
        rdfs:range xsd:integer ; 
        rdf:isDefinedBy <https://sportschema.org/ontologies/american-football-statistics> . 
        
	spamfstat:puntsAgainstYardsGross rdf:type rdf:Property ; 
        rdfs:label "puntsAgainstYardsGross"@en ; 
        rdfs:comment "Number of yards of opposing team's punts."@en ; 
        rdfs:domain [fill in] ; 
        rdfs:range xsd:integer ; 
        rdf:isDefinedBy <https://sportschema.org/ontologies/american-football-statistics> . 
        
	spamfstat:puntsAgainstYardsNet rdf:type rdf:Property ; 
        rdfs:label "puntsAgainstYardsNet"@en ; 
        rdfs:comment "Number of net yards - punt length minus return - of
                opposing team's punts."@en ; 
        rdfs:domain [fill in] ; 
        rdfs:range xsd:integer ; 
        rdf:isDefinedBy <https://sportschema.org/ontologies/american-football-statistics> . 
        
	spamfstat:puntsAgainstLongest rdf:type rdf:Property ; 
        rdfs:label "puntsAgainstLongest"@en ; 
        rdfs:comment "Longest punt by opposing team."@en ; 
        rdfs:domain [fill in] ; 
        rdfs:range xsd:integer ; 
        rdf:isDefinedBy <https://sportschema.org/ontologies/american-football-statistics> . 
        
	spamfstat:puntsAgainstInside20 rdf:type rdf:Property ; 
        rdfs:label "puntsAgainstInside20"@en ; 
        rdfs:comment "Punt returns failed to advance beyond team's own
                20."@en ; 
        rdfs:domain [fill in] ; 
        rdfs:range xsd:integer ; 
        rdf:isDefinedBy <https://sportschema.org/ontologies/american-football-statistics> . 
        
	spamfstat:puntsAgainstInside20Percentage rdf:type rdf:Property ; 
        rdfs:label "puntsAgainstInside20Percentage"@en ; 
        rdfs:comment "Ratio of punt returns failed to advance beyond team's own
                20 and total punt returns."@en ; 
        rdfs:domain [fill in] ; 
        rdfs:range xsd:integer ; 
        rdf:isDefinedBy <https://sportschema.org/ontologies/american-football-statistics> . 
        
	spamfstat:puntsAgainstAverage rdf:type rdf:Property ; 
        rdfs:label "puntsAgainstAverage"@en ; 
        rdfs:comment "Average length of opponent's punt."@en ; 
        rdfs:domain [fill in] ; 
        rdfs:range xsd:integer ; 
        rdf:isDefinedBy <https://sportschema.org/ontologies/american-football-statistics> . 
        
	spamfstat:puntsAgainstAverageNet rdf:type rdf:Property ; 
        rdfs:label "puntsAgainstAverageNet"@en ; 
        rdfs:comment "Average net length - punt length minus return - of
                opponent's punt.."@en ; 
        rdfs:domain [fill in] ; 
        rdfs:range xsd:integer ; 
        rdf:isDefinedBy <https://sportschema.org/ontologies/american-football-statistics> . 
        
	spamfstat:puntsBlocked rdf:type rdf:Property ; 
        rdfs:label "puntsBlocked"@en ; 
        rdfs:comment "The number of punts that were blocked."@en ; 
        rdfs:domain [fill in] ; 
        rdfs:range xsd:integer ; 
        rdf:isDefinedBy <https://sportschema.org/ontologies/american-football-statistics> . 
        
	spamfstat:puntsAgainstBlocked rdf:type rdf:Property ; 
        rdfs:label "puntsAgainstBlocked"@en ; 
        rdfs:comment "The number of punts made by the opposing team that this
                team or player has blocked."@en ; 
        rdfs:domain [fill in] ; 
        rdfs:range xsd:integer ; 
        rdf:isDefinedBy <https://sportschema.org/ontologies/american-football-statistics> . 
        
	spamfstat:touchbacksTotal rdf:type rdf:Property ; 
        rdfs:label "touchbacksTotal"@en ; 
        rdfs:comment "The total number of touchbacks, from kickoffs, punts,
                interceptions, and fumbles."@en ; 
        rdfs:domain [fill in] ; 
        rdfs:range xsd:integer ; 
        rdf:isDefinedBy <https://sportschema.org/ontologies/american-football-statistics> . 
        
	spamfstat:touchbacksTotalPercentage rdf:type rdf:Property ; 
        rdfs:label "touchbacksTotalPercentage"@en ; 
        rdfs:comment "The percentage of kickoffs, punts, interceptions, and
                fumbles which resulted in a touchback."@en ; 
        rdfs:domain [fill in] ; 
        rdfs:range xsd:integer ; 
        rdf:isDefinedBy <https://sportschema.org/ontologies/american-football-statistics> . 
        
	spamfstat:touchbacksKickoffs rdf:type rdf:Property ; 
        rdfs:label "touchbacksKickoffs"@en ; 
        rdfs:comment "The number of kickoffs that went into the end zone and were
                not brought out."@en ; 
        rdfs:domain [fill in] ; 
        rdfs:range xsd:integer ; 
        rdf:isDefinedBy <https://sportschema.org/ontologies/american-football-statistics> . 
        
	spamfstat:touchbacksKickoffsPercentage rdf:type rdf:Property ; 
        rdfs:label "touchbacksKickoffsPercentage"@en ; 
        rdfs:comment "The percentage of kickoffs resulting in
                touchbacks."@en ; 
        rdfs:domain [fill in] ; 
        rdfs:range xsd:integer ; 
        rdf:isDefinedBy <https://sportschema.org/ontologies/american-football-statistics> . 
        
	spamfstat:touchbacksPunts rdf:type rdf:Property ; 
        rdfs:label "touchbacksPunts"@en ; 
        rdfs:comment "The number of punts that went into the end zone and were
                not brought out."@en ; 
        rdfs:domain [fill in] ; 
        rdfs:range xsd:integer ; 
        rdf:isDefinedBy <https://sportschema.org/ontologies/american-football-statistics> . 
        
	spamfstat:touchbacksPuntsPercentage rdf:type rdf:Property ; 
        rdfs:label "touchbacksPuntsPercentage"@en ; 
        rdfs:comment "The percentage of punts resulting in
                touchbacks."@en ; 
        rdfs:domain [fill in] ; 
        rdfs:range xsd:integer ; 
        rdf:isDefinedBy <https://sportschema.org/ontologies/american-football-statistics> . 
        
	spamfstat:touchbacksInterceptions rdf:type rdf:Property ; 
        rdfs:label "touchbacksInterceptions"@en ; 
        rdfs:comment "The number of interceptions that went into the end zone and
                were not brought out."@en ; 
        rdfs:domain [fill in] ; 
        rdfs:range xsd:integer ; 
        rdf:isDefinedBy <https://sportschema.org/ontologies/american-football-statistics> . 
        
	spamfstat:touchbacksInterceptionsPercentage rdf:type rdf:Property ; 
        rdfs:label "touchbacksInterceptionsPercentage"@en ; 
        rdfs:comment "The percentage of interceptions resulting in
                touchbacks."@en ; 
        rdfs:domain [fill in] ; 
        rdfs:range xsd:integer ; 
        rdf:isDefinedBy <https://sportschema.org/ontologies/american-football-statistics> . 
        
	spamfstat:touchbacksPuntsAgainst rdf:type rdf:Property ; 
        rdfs:label "touchbacksPuntsAgainst"@en ; 
        rdfs:comment "Number of punts not returned out of receiving team's end
                zone."@en ; 
        rdfs:domain [fill in] ; 
        rdfs:range xsd:integer ; 
        rdf:isDefinedBy <https://sportschema.org/ontologies/american-football-statistics> . 
        
	spamfstat:fairCatches rdf:type rdf:Property ; 
        rdfs:label "fairCatches"@en ; 
        rdfs:comment "The number of fair catches."@en ; 
        rdfs:domain [fill in] ; 
        rdfs:range xsd:integer ; 
        rdf:isDefinedBy <https://sportschema.org/ontologies/american-football-statistics> . 
        
	spamfstat:fairCatchesAgainst rdf:type rdf:Property ; 
        rdfs:label "fairCatchesAgainst"@en ; 
        rdfs:comment "Number of fair catches by opponents."@en ; 
        rdfs:domain [fill in] ; 
        rdfs:range xsd:integer ; 
        rdf:isDefinedBy <https://sportschema.org/ontologies/american-football-statistics> . 
        
	spamfstat:totalReturnYardageNotKickoffs rdf:type rdf:Property ; 
        rdfs:label "totalReturnYardageNotKickoffs"@en ; 
        rdfs:comment "Net return yardage excluding kickoff returns."@en ; 
        rdfs:domain [fill in] ; 
        rdfs:range xsd:integer ; 
        rdf:isDefinedBy <https://sportschema.org/ontologies/american-football-statistics> . 
        
	spamfstat:touchdownsAgainst rdf:type rdf:Property ; 
        rdfs:label "touchdownsAgainst"@en ; 
        rdfs:comment "Total number of special teams touchdowns
                allowed."@en ; 
        rdfs:domain [fill in] ; 
        rdfs:range xsd:integer ; 
        rdf:isDefinedBy <https://sportschema.org/ontologies/american-football-statistics> . 
        
	spamfstat:tacklesSpecialTeams rdf:type rdf:Property ; 
        rdfs:label "tacklesSpecialTeams"@en ; 
        rdfs:comment "The number of tackles made while playing for a
                special-team."@en ; 
        rdfs:domain [fill in] ; 
        rdfs:range xsd:integer ; 
        rdf:isDefinedBy <https://sportschema.org/ontologies/american-football-statistics> . 
        
	spamfstat:tacklesAssistsSpecialTeams rdf:type rdf:Property ; 
        rdfs:label "tacklesAssistsSpecialTeams"@en ; 
        rdfs:comment "The number of tackle assists performed while on
                special-teams."@en ; 
        rdfs:domain [fill in] ; 
        rdfs:range xsd:integer ; 
        rdf:isDefinedBy <https://sportschema.org/ontologies/american-football-statistics> . 
        
	spamfstat:extraPointsAgainstMade rdf:type rdf:Property ; 
        rdfs:label "extraPointsAgainstMade"@en ; 
        rdfs:comment "Number of extra point attempts made by the opposing team
                that were successful."@en ; 
        rdfs:domain [fill in] ; 
        rdfs:range xsd:integer ; 
        rdf:isDefinedBy <https://sportschema.org/ontologies/american-football-statistics> . 
        
	spamfstat:extraPointsAgainstMissed rdf:type rdf:Property ; 
        rdfs:label "extraPointsAgainstMissed"@en ; 
        rdfs:comment "Number of extra point attempts made by the opposing team
                that were not successful."@en ; 
        rdfs:domain [fill in] ; 
        rdfs:range xsd:integer ; 
        rdf:isDefinedBy <https://sportschema.org/ontologies/american-football-statistics> . 
        
	spamfstat:extraPointsAgainstBlocked rdf:type rdf:Property ; 
        rdfs:label "extraPointsAgainstBlocked"@en ; 
        rdfs:comment "Number of extra point attempts made by the opposing team
                that were blocked by this team or player."@en ; 
        rdfs:domain [fill in] ; 
        rdfs:range xsd:integer ; 
        rdf:isDefinedBy <https://sportschema.org/ontologies/american-football-statistics> . 
        
	spamfstat:fieldGoalsAgainstMade rdf:type rdf:Property ; 
        rdfs:label "fieldGoalsAgainstMade"@en ; 
        rdfs:comment "Number of field goal attempts made by the opposing team
                that were successful."@en ; 
        rdfs:domain [fill in] ; 
        rdfs:range xsd:integer ; 
        rdf:isDefinedBy <https://sportschema.org/ontologies/american-football-statistics> . 
        
	spamfstat:fieldGoalsAgainstMissed rdf:type rdf:Property ; 
        rdfs:label "fieldGoalsAgainstMissed"@en ; 
        rdfs:comment "Number of field goal attempts made by the opposing team
                that were not successful."@en ; 
        rdfs:domain [fill in] ; 
        rdfs:range xsd:integer ; 
        rdf:isDefinedBy <https://sportschema.org/ontologies/american-football-statistics> . 
        
	spamfstat:fieldGoalsAgainstBlocked rdf:type rdf:Property ; 
        rdfs:label "fieldGoalsAgainstBlocked"@en ; 
        rdfs:comment "Number of field goal attempts made by the opposing team
                that were blocked by this player or team."@en ; 
        rdfs:domain [fill in] ; 
        rdfs:range xsd:integer ; 
        rdf:isDefinedBy <https://sportschema.org/ontologies/american-football-statistics> . 
        
	spamfstat:fumblesCommitted rdf:type rdf:Property ; 
        rdfs:label "fumblesCommitted"@en ; 
        rdfs:comment "The total number of fumbles."@en ; 
        rdfs:domain [fill in] ; 
        rdfs:range xsd:integer ; 
        rdf:isDefinedBy <https://sportschema.org/ontologies/american-football-statistics> . 
        
	spamfstat:fumblesForced rdf:type rdf:Property ; 
        rdfs:label "fumblesForced"@en ; 
        rdfs:comment "The number of fumbles that were forced by the opposing
                team."@en ; 
        rdfs:domain [fill in] ; 
        rdfs:range xsd:integer ; 
        rdf:isDefinedBy <https://sportschema.org/ontologies/american-football-statistics> . 
        
	spamfstat:fumblesRecovered rdf:type rdf:Property ; 
        rdfs:label "fumblesRecovered"@en ; 
        rdfs:comment "The number of fumbles that were recovered by the fumbling
                team."@en ; 
        rdfs:domain [fill in] ; 
        rdfs:range xsd:integer ; 
        rdf:isDefinedBy <https://sportschema.org/ontologies/american-football-statistics> . 
        
	spamfstat:fumblesLost rdf:type rdf:Property ; 
        rdfs:label "fumblesLost"@en ; 
        rdfs:comment "The number of fumbles that were not recovered by the
                fumbling team."@en ; 
        rdfs:domain [fill in] ; 
        rdfs:range xsd:integer ; 
        rdf:isDefinedBy <https://sportschema.org/ontologies/american-football-statistics> . 
        
	spamfstat:fumblesLostAveragePerGame rdf:type rdf:Property ; 
        rdfs:label "fumblesLostAveragePerGame"@en ; 
        rdfs:comment "Average number of fumbles lost per game."@en ; 
        rdfs:domain [fill in] ; 
        rdfs:range xsd:integer ; 
        rdf:isDefinedBy <https://sportschema.org/ontologies/american-football-statistics> . 
        
	spamfstat:fumblesYardsGained rdf:type rdf:Property ; 
        rdfs:label "fumblesYardsGained"@en ; 
        rdfs:comment "The number of yards gained as a result of
                fumbles."@en ; 
        rdfs:domain [fill in] ; 
        rdfs:range xsd:integer ; 
        rdf:isDefinedBy <https://sportschema.org/ontologies/american-football-statistics> . 
        
	spamfstat:fumblesOwnCommitted rdf:type rdf:Property ; 
        rdfs:label "fumblesOwnCommitted"@en ; 
        rdfs:comment "The number of fumbles committed by this team."@en ; 
        rdfs:domain [fill in] ; 
        rdfs:range xsd:integer ; 
        rdf:isDefinedBy <https://sportschema.org/ontologies/american-football-statistics> . 
        
	spamfstat:fumblesOwnRecovered rdf:type rdf:Property ; 
        rdfs:label "fumblesOwnRecovered"@en ; 
        rdfs:comment "The number of fumbles committed by this team that were then
                also recovered by this team."@en ; 
        rdfs:domain [fill in] ; 
        rdfs:range xsd:integer ; 
        rdf:isDefinedBy <https://sportschema.org/ontologies/american-football-statistics> . 
        
	spamfstat:fumblesOwnLost rdf:type rdf:Property ; 
        rdfs:label "fumblesOwnLost"@en ; 
        rdfs:comment "The number of fumbles committed by this team but recovered
                by the other team. A subset of turnovers. Also referred to as a
                giveaway."@en ; 
        rdfs:domain [fill in] ; 
        rdfs:range xsd:integer ; 
        rdf:isDefinedBy <https://sportschema.org/ontologies/american-football-statistics> . 
        
	spamfstat:fumblesOwnYardsGained rdf:type rdf:Property ; 
        rdfs:label "fumblesOwnYardsGained"@en ; 
        rdfs:comment "The number of yards gained as a result of fumbles by this
                team."@en ; 
        rdfs:domain [fill in] ; 
        rdfs:range xsd:integer ; 
        rdf:isDefinedBy <https://sportschema.org/ontologies/american-football-statistics> . 
        
	spamfstat:fumblesOwnTouchdowns rdf:type rdf:Property ; 
        rdfs:label "fumblesOwnTouchdowns"@en ; 
        rdfs:comment "The number of touchdowns earned after a team recovers its
                own fumbles."@en ; 
        rdfs:domain [fill in] ; 
        rdfs:range xsd:integer ; 
        rdf:isDefinedBy <https://sportschema.org/ontologies/american-football-statistics> . 
        
	spamfstat:fumblesOpposingCommitted rdf:type rdf:Property ; 
        rdfs:label "fumblesOpposingCommitted"@en ; 
        rdfs:comment "The number of fumbles committed by the opposing
                team."@en ; 
        rdfs:domain [fill in] ; 
        rdfs:range xsd:integer ; 
        rdf:isDefinedBy <https://sportschema.org/ontologies/american-football-statistics> . 
        
	spamfstat:fumblesOpposingRecovered rdf:type rdf:Property ; 
        rdfs:label "fumblesOpposingRecovered"@en ; 
        rdfs:comment "The number of fumbles committed by the opposing but
                recovered by this team. A subset of turnovers. Also referred to a
                takeaway."@en ; 
        rdfs:domain [fill in] ; 
        rdfs:range xsd:integer ; 
        rdf:isDefinedBy <https://sportschema.org/ontologies/american-football-statistics> . 
        
	spamfstat:fumblesOpposingRecoveredAveragePerGame rdf:type rdf:Property ; 
        rdfs:label "fumblesOpposingRecoveredAveragePerGame"@en ; 
        rdfs:comment "Average number of opposing team's fumbles recovered per
                game."@en ; 
        rdfs:domain [fill in] ; 
        rdfs:range xsd:integer ; 
        rdf:isDefinedBy <https://sportschema.org/ontologies/american-football-statistics> . 
        
	spamfstat:fumblesOpposingLost rdf:type rdf:Property ; 
        rdfs:label "fumblesOpposingLost"@en ; 
        rdfs:comment "The number of fumbles committed by the opposing team that
                were subsequently lost to the opposing team."@en ; 
        rdfs:domain [fill in] ; 
        rdfs:range xsd:integer ; 
        rdf:isDefinedBy <https://sportschema.org/ontologies/american-football-statistics> . 
        
	spamfstat:fumblesOpposingYardsGained rdf:type rdf:Property ; 
        rdfs:label "fumblesOpposingYardsGained"@en ; 
        rdfs:comment "The number of yards gained as a result of fumbles by the
                opposing team."@en ; 
        rdfs:domain [fill in] ; 
        rdfs:range xsd:integer ; 
        rdf:isDefinedBy <https://sportschema.org/ontologies/american-football-statistics> . 
        
	spamfstat:fumblesOpposingTouchdowns rdf:type rdf:Property ; 
        rdfs:label "fumblesOpposingTouchdowns"@en ; 
        rdfs:comment "The number of touchdowns scored as a result of fumbles by
                the opposing team.."@en ; 
        rdfs:domain [fill in] ; 
        rdfs:range xsd:integer ; 
        rdf:isDefinedBy <https://sportschema.org/ontologies/american-football-statistics> . 
        
	spamfstat:fumblesCommittedDefense rdf:type rdf:Property ; 
        rdfs:label "fumblesCommittedDefense"@en ; 
        rdfs:comment "The number of fumbles committed by a player or team on
                defense."@en ; 
        rdfs:domain [fill in] ; 
        rdfs:range xsd:integer ; 
        rdf:isDefinedBy <https://sportschema.org/ontologies/american-football-statistics> . 
        
	spamfstat:fumblesLostDefense rdf:type rdf:Property ; 
        rdfs:label "fumblesLostDefense"@en ; 
        rdfs:comment "The number of fumbles lost by a player or team on
                defense."@en ; 
        rdfs:domain [fill in] ; 
        rdfs:range xsd:integer ; 
        rdf:isDefinedBy <https://sportschema.org/ontologies/american-football-statistics> . 
        
	spamfstat:fumblesForcedDefense rdf:type rdf:Property ; 
        rdfs:label "fumblesForcedDefense"@en ; 
        rdfs:comment "The number of fumbles forced by a player or team on
                defense."@en ; 
        rdfs:domain [fill in] ; 
        rdfs:range xsd:integer ; 
        rdf:isDefinedBy <https://sportschema.org/ontologies/american-football-statistics> . 
        
	spamfstat:fumblesRecoveredDefense rdf:type rdf:Property ; 
        rdfs:label "fumblesRecoveredDefense"@en ; 
        rdfs:comment "The number of fumbles recovered by a player or team on
                defense."@en ; 
        rdfs:domain [fill in] ; 
        rdfs:range xsd:integer ; 
        rdf:isDefinedBy <https://sportschema.org/ontologies/american-football-statistics> . 
        
	spamfstat:fumblesRecoveredYardsDefense rdf:type rdf:Property ; 
        rdfs:label "fumblesRecoveredYardsDefense"@en ; 
        rdfs:comment "The number of yards gained on fumbles recovered by a player
                or team on defense."@en ; 
        rdfs:domain [fill in] ; 
        rdfs:range xsd:integer ; 
        rdf:isDefinedBy <https://sportschema.org/ontologies/american-football-statistics> . 
        
	spamfstat:fumblesCommittedSpecialTeams rdf:type rdf:Property ; 
        rdfs:label "fumblesCommittedSpecialTeams"@en ; 
        rdfs:comment "The number of fumbles committed by a player or team on
                special-teams."@en ; 
        rdfs:domain [fill in] ; 
        rdfs:range xsd:integer ; 
        rdf:isDefinedBy <https://sportschema.org/ontologies/american-football-statistics> . 
        
	spamfstat:fumblesLostSpecialTeams rdf:type rdf:Property ; 
        rdfs:label "fumblesLostSpecialTeams"@en ; 
        rdfs:comment "The number of fumbles lost by a player or team on
                special-teams."@en ; 
        rdfs:domain [fill in] ; 
        rdfs:range xsd:integer ; 
        rdf:isDefinedBy <https://sportschema.org/ontologies/american-football-statistics> . 
        
	spamfstat:fumblesForcedSpecialTeams rdf:type rdf:Property ; 
        rdfs:label "fumblesForcedSpecialTeams"@en ; 
        rdfs:comment "The number of fumbles forced by a player or team on
                special-teams."@en ; 
        rdfs:domain [fill in] ; 
        rdfs:range xsd:integer ; 
        rdf:isDefinedBy <https://sportschema.org/ontologies/american-football-statistics> . 
        
	spamfstat:fumblesRecoveredSpecialTeams rdf:type rdf:Property ; 
        rdfs:label "fumblesRecoveredSpecialTeams"@en ; 
        rdfs:comment "The number of fumbles recovered by a player or team on
                special-teams."@en ; 
        rdfs:domain [fill in] ; 
        rdfs:range xsd:integer ; 
        rdf:isDefinedBy <https://sportschema.org/ontologies/american-football-statistics> . 
        
	spamfstat:fumblesRecoveredYardsSpecialTeams rdf:type rdf:Property ; 
        rdfs:label "fumblesRecoveredYardsSpecialTeams"@en ; 
        rdfs:comment "The number of yards gained on fumbles recovered by a player
                or team on special-teams."@en ; 
        rdfs:domain [fill in] ; 
        rdfs:range xsd:integer ; 
        rdf:isDefinedBy <https://sportschema.org/ontologies/american-football-statistics> . 
        
	spamfstat:fumblesCommittedOther rdf:type rdf:Property ; 
        rdfs:label "fumblesCommittedOther"@en ; 
        rdfs:comment "The number of fumbles committed by a player or team on
                neither defense or special teams."@en ; 
        rdfs:domain [fill in] ; 
        rdfs:range xsd:integer ; 
        rdf:isDefinedBy <https://sportschema.org/ontologies/american-football-statistics> . 
        
	spamfstat:fumblesLostOther rdf:type rdf:Property ; 
        rdfs:label "fumblesLostOther"@en ; 
        rdfs:comment "The number of fumbles lost by a player or team on neither
                defense or special teams."@en ; 
        rdfs:domain [fill in] ; 
        rdfs:range xsd:integer ; 
        rdf:isDefinedBy <https://sportschema.org/ontologies/american-football-statistics> . 
        
	spamfstat:fumblesForcedOther rdf:type rdf:Property ; 
        rdfs:label "fumblesForcedOther"@en ; 
        rdfs:comment "The number of fumbles forced by a player or team on neither
                defense or special teams."@en ; 
        rdfs:domain [fill in] ; 
        rdfs:range xsd:integer ; 
        rdf:isDefinedBy <https://sportschema.org/ontologies/american-football-statistics> . 
        
	spamfstat:fumblesRecoveredOther rdf:type rdf:Property ; 
        rdfs:label "fumblesRecoveredOther"@en ; 
        rdfs:comment "The number of fumbles recovered by a player or team on
                neither defense or special teams."@en ; 
        rdfs:domain [fill in] ; 
        rdfs:range xsd:integer ; 
        rdf:isDefinedBy <https://sportschema.org/ontologies/american-football-statistics> . 
        
	spamfstat:fumblesRecoveredYardsOther rdf:type rdf:Property ; 
        rdfs:label "fumblesRecoveredYardsOther"@en ; 
        rdfs:comment "The number of yards gained on fumbles recovered by a player
                or team on neither defense or special teams."@en ; 
        rdfs:domain [fill in] ; 
        rdfs:range xsd:integer ; 
        rdf:isDefinedBy <https://sportschema.org/ontologies/american-football-statistics> . 
        
	spamfstat:touchbacksFumbles rdf:type rdf:Property ; 
        rdfs:label "touchbacksFumbles"@en ; 
        rdfs:comment "The number of fumbles into the end zone that are not
                brought out."@en ; 
        rdfs:domain [fill in] ; 
        rdfs:range xsd:integer ; 
        rdf:isDefinedBy <https://sportschema.org/ontologies/american-football-statistics> . 
        
	spamfstat:touchbacksFumblesPercentage rdf:type rdf:Property ; 
        rdfs:label "touchbacksFumblesPercentage"@en ; 
        rdfs:comment "The percentage of fumbles that resulted in
                touchbacks."@en ; 
        rdfs:domain [fill in] ; 
        rdfs:range xsd:integer ; 
        rdf:isDefinedBy <https://sportschema.org/ontologies/american-football-statistics> . 
        
	spamfstat:penaltiesTotal rdf:type rdf:Property ; 
        rdfs:label "penaltiesTotal"@en ; 
        rdfs:comment "The number of penalties."@en ; 
        rdfs:domain [fill in] ; 
        rdfs:range xsd:integer ; 
        rdf:isDefinedBy <https://sportschema.org/ontologies/american-football-statistics> . 
        
	spamfstat:penaltyYards rdf:type rdf:Property ; 
        rdfs:label "penaltyYards"@en ; 
        rdfs:comment "The yards gained as a result of penalties."@en ; 
        rdfs:domain [fill in] ; 
        rdfs:range xsd:integer ; 
        rdf:isDefinedBy <https://sportschema.org/ontologies/american-football-statistics> . 
        
	spamfstat:penaltyFirstDowns rdf:type rdf:Property ; 
        rdfs:label "penaltyFirstDowns"@en ; 
        rdfs:comment "The number of first downs gained as a result of
                penalties."@en ; 
        rdfs:domain [fill in] ; 
        rdfs:range xsd:integer ; 
        rdf:isDefinedBy <https://sportschema.org/ontologies/american-football-statistics> . 
        
	spamfstat:penaltyOpponentYards rdf:type rdf:Property ; 
        rdfs:label "penaltyOpponentYards"@en ; 
        rdfs:comment "Yards opponents gain as a result of penalties."@en ; 
        rdfs:domain [fill in] ; 
        rdfs:range xsd:integer ; 
        rdf:isDefinedBy <https://sportschema.org/ontologies/american-football-statistics> . 
        
	spamfstat:penaltiesOpponentTotal rdf:type rdf:Property ; 
        rdfs:label "penaltiesOpponentTotal"@en ; 
        rdfs:comment "Total of penalties by opposing team."@en ; 
        rdfs:domain [fill in] ; 
        rdfs:range xsd:integer ; 
        rdf:isDefinedBy <https://sportschema.org/ontologies/american-football-statistics> . 
        
	spamfstat:penaltiesChallenged rdf:type rdf:Property ; 
        rdfs:label "penaltiesChallenged"@en ; 
        rdfs:comment "Includes penalty challenges that were both won and
                lost."@en ; 
        rdfs:domain [fill in] ; 
        rdfs:range xsd:integer ; 
        rdf:isDefinedBy <https://sportschema.org/ontologies/american-football-statistics> . 
        
	spamfstat:penaltiesReviewed rdf:type rdf:Property ; 
        rdfs:label "penaltiesReviewed"@en ; 
        rdfs:comment "Includes both coach challenges and booth challenges (by the
                replay assistant in the NFL)."@en ; 
        rdfs:domain [fill in] ; 
        rdfs:range xsd:integer ; 
        rdf:isDefinedBy <https://sportschema.org/ontologies/american-football-statistics> . 
        
	spamfstat:penaltiesOverturned rdf:type rdf:Property ; 
        rdfs:label "penaltiesOverturned"@en ; 
        rdfs:comment "The number of successful penalty challenges by a team,
                leading to the overturning of the original call."@en ; 
        rdfs:domain [fill in] ; 
        rdfs:range xsd:integer ; 
        rdf:isDefinedBy <https://sportschema.org/ontologies/american-football-statistics> . 
        
	